<?xml version="1.0"?>
<rdf:RDF xmlns="https://w3id.org/def/vaeontology#"
     xml:base="https://w3id.org/def/vaeontology"
     xmlns:dc="http://purl.org/dc/elements/1.1/"
     xmlns:bhv="https://w3id.org/spice/SON/SchwartzValues#"
     xmlns:dul="http://www.ontologydesignpatterns.org/ont/dul/DUL.owl#"
     xmlns:mod="https://w3id.org/mod#"
     xmlns:owl="http://www.w3.org/2002/07/owl#"
     xmlns:rdf="http://www.w3.org/1999/02/22-rdf-syntax-ns#"
     xmlns:vae="https://w3id.org/def/vaeontology#"
     xmlns:xml="http://www.w3.org/XML/1998/namespace"
     xmlns:xsd="http://www.w3.org/2001/XMLSchema#"
     xmlns:odrl="http://www.w3.org/ns/odrl/2/"
     xmlns:rdfs="http://www.w3.org/2000/01/rdf-schema#"
     xmlns:skos="http://www.w3.org/2004/02/skos/core#"
     xmlns:vann="http://purl.org/vocab/vann/"
     xmlns:vcvf="http://www.ontologydesignpatterns.org/ont/values/valuecore_with_value_frames.owl#"
     xmlns:terms="http://purl.org/dc/terms/"
     xmlns:schema="https://w3id.org/framester/schema/"
     xmlns:fschema="https://w3id.org/framester/schema#"
     xmlns:schema1="https://w3id.org/framester/metanet/schema/"
     xmlns:cpannotationschema="http://www.ontologydesignpatterns.org/schemas/cpannotationschema.owl#">
    <owl:Ontology rdf:about="https://w3id.org/def/vaeontology">
        <owl:versionIRI rdf:resource="https://w3id.org/def/vaeontology/1.0.1"/>
        <dc:created rdf:datatype="http://www.w3.org/2001/XMLSchema#date">2023-11-14</dc:created>
        <dc:creator>Andrés Holgado Sánchez - https://orcid.org/my-orcid?orcid=0000-0001-8853-1022</dc:creator>
        <dc:description xml:lang="en">Ontology for Value Awareness Engineering: representation and reasoning with human values.</dc:description>
        <dc:title xml:lang="en">VAE Ontology</dc:title>
        <terms:license rdf:resource="https://creativecommons.org/licenses/by/4.0/"/>
        <vann:preferredNamespacePrefix>vae</vann:preferredNamespacePrefix>
        <vann:preferredNamespaceUri rdf:resource="https://w3id.org/def/vaeontology#"/>
        <owl:versionInfo>1.0.1</owl:versionInfo>
        <mod:createdWith rdf:resource="https://chowlk.linkeddata.es"/>
    </owl:Ontology>
    


    <!-- 
    ///////////////////////////////////////////////////////////////////////////////////////
    //
    // Annotation properties
    //
    ///////////////////////////////////////////////////////////////////////////////////////
     -->

    


    <!-- http://purl.org/dc/elements/1.1/created -->

    <owl:AnnotationProperty rdf:about="http://purl.org/dc/elements/1.1/created"/>
    


    <!-- http://purl.org/dc/elements/1.1/creator -->

    <owl:AnnotationProperty rdf:about="http://purl.org/dc/elements/1.1/creator"/>
    


    <!-- http://purl.org/dc/elements/1.1/description -->

    <owl:AnnotationProperty rdf:about="http://purl.org/dc/elements/1.1/description"/>
    


    <!-- http://purl.org/dc/elements/1.1/license -->

    <owl:AnnotationProperty rdf:about="http://purl.org/dc/elements/1.1/license"/>
    


    <!-- http://purl.org/dc/elements/1.1/title -->

    <owl:AnnotationProperty rdf:about="http://purl.org/dc/elements/1.1/title"/>
    


    <!-- http://purl.org/dc/terms/license -->

    <owl:AnnotationProperty rdf:about="http://purl.org/dc/terms/license">
        <rdfs:subPropertyOf rdf:resource="http://purl.org/dc/terms/license"/>
    </owl:AnnotationProperty>
    


    <!-- http://purl.org/vocab/vann/preferredNamespacePrefix -->

    <owl:AnnotationProperty rdf:about="http://purl.org/vocab/vann/preferredNamespacePrefix"/>
    


    <!-- http://purl.org/vocab/vann/preferredNamespaceUri -->

    <owl:AnnotationProperty rdf:about="http://purl.org/vocab/vann/preferredNamespaceUri"/>
    


    <!-- http://www.ontologydesignpatterns.org/ont/dul/DUL.owl#defines -->

    <owl:AnnotationProperty rdf:about="http://www.ontologydesignpatterns.org/ont/dul/DUL.owl#defines"/>
    


    <!-- http://www.ontologydesignpatterns.org/ont/values/valuecore_with_value_frames.owl#commitsTo -->

    <owl:AnnotationProperty rdf:about="http://www.ontologydesignpatterns.org/ont/values/valuecore_with_value_frames.owl#commitsTo"/>
    


    <!-- http://www.w3.org/2000/01/rdf-schema#comment -->

    <owl:AnnotationProperty rdf:about="http://www.w3.org/2000/01/rdf-schema#comment">
        <rdfs:range rdf:resource="http://www.w3.org/2001/XMLSchema#String"/>
        <rdfs:range rdf:resource="http://www.w3.org/2001/XMLSchema#string"/>
    </owl:AnnotationProperty>
    


    <!-- http://www.w3.org/2002/07/owl#priorVersion -->

    <owl:AnnotationProperty rdf:about="http://www.w3.org/2002/07/owl#priorVersion"/>
    


    <!-- http://www.w3.org/2002/07/owl#versionIRI -->

    <owl:AnnotationProperty rdf:about="http://www.w3.org/2002/07/owl#versionIRI"/>
    


    <!-- http://www.w3.org/2002/07/owl#versionInfo -->

    <owl:AnnotationProperty rdf:about="http://www.w3.org/2002/07/owl#versionInfo"/>
    


    <!-- http://www.w3.org/2004/02/skos/core#definition -->

    <owl:AnnotationProperty rdf:about="http://www.w3.org/2004/02/skos/core#definition"/>
    


    <!-- http://www.w3.org/2004/02/skos/core#note -->

    <owl:AnnotationProperty rdf:about="http://www.w3.org/2004/02/skos/core#note"/>
    


    <!-- http://www.w3.org/2004/02/skos/core#scopeNote -->

    <owl:AnnotationProperty rdf:about="http://www.w3.org/2004/02/skos/core#scopeNote"/>
    


    <!-- https://w3id.org/def/vaeontology#directlyGeneralizes -->

    <owl:AnnotationProperty rdf:about="https://w3id.org/def/vaeontology#directlyGeneralizes"/>
    


    <!-- https://w3id.org/mod#createdWith -->

    <owl:AnnotationProperty rdf:about="https://w3id.org/mod#createdWith"/>
    


    <!-- https://w3id.org/spice/SON/SchwartzValues#bibRef -->

    <owl:AnnotationProperty rdf:about="https://w3id.org/spice/SON/SchwartzValues#bibRef"/>
    


    <!-- 
    ///////////////////////////////////////////////////////////////////////////////////////
    //
    // Datatypes
    //
    ///////////////////////////////////////////////////////////////////////////////////////
     -->

    


    <!-- http://www.w3.org/2001/XMLSchema#date -->

    <rdfs:Datatype rdf:about="http://www.w3.org/2001/XMLSchema#date"/>
    


    <!-- 
    ///////////////////////////////////////////////////////////////////////////////////////
    //
    // Object Properties
    //
    ///////////////////////////////////////////////////////////////////////////////////////
     -->

    


    <!-- http://www.ontologydesignpatterns.org/ont/dul/DUL.owl#associatedWith -->

    <owl:ObjectProperty rdf:about="http://www.ontologydesignpatterns.org/ont/dul/DUL.owl#associatedWith"/>
    


    <!-- http://www.ontologydesignpatterns.org/ont/dul/DUL.owl#conceptualizes -->

    <owl:ObjectProperty rdf:about="http://www.ontologydesignpatterns.org/ont/dul/DUL.owl#conceptualizes">
        <rdfs:subPropertyOf rdf:resource="http://www.ontologydesignpatterns.org/ont/dul/DUL.owl#associatedWith"/>
        <owl:inverseOf rdf:resource="http://www.ontologydesignpatterns.org/ont/dul/DUL.owl#isConceptualizedBy"/>
        <rdfs:domain rdf:resource="http://www.ontologydesignpatterns.org/ont/dul/DUL.owl#Agent"/>
        <rdfs:range rdf:resource="http://www.ontologydesignpatterns.org/ont/dul/DUL.owl#SocialObject"/>
        <rdfs:comment>A relation stating that an Agent is internally representing a SocialObject: situations, descriptions, concepts, etc. E.g., &apos;John believes in the conspiracy theory&apos;; &apos;Niels Bohr created the solar-system metaphor for the atomic theory&apos;; &apos;Jacques assumes all swans are white&apos;; &apos;the task force members share the attack plan&apos;.
Conceptualizations can be distinguished into different forms, primarily based on the type of SocialObject that is conceptualized. Descriptions and concepts can be &apos;assumed&apos;, situations can be &apos;believed&apos; or &apos;known&apos;, plans can be &apos;adopted&apos;, etc. (see ontology: http://www.ontologydesignpatterns.org/ont/dul/Conceptualization.owl.</rdfs:comment>
        <rdfs:isDefinedBy rdf:resource="http://www.ontologydesignpatterns.org/ont/dul/DUL.owl"/>
        <rdfs:label>conceptualizes</rdfs:label>
        <rdfs:label xml:lang="en">conceptualizes</rdfs:label>
        <rdfs:label xml:lang="it">concettualizza</rdfs:label>
    </owl:ObjectProperty>
    


    <!-- http://www.ontologydesignpatterns.org/ont/dul/DUL.owl#describes -->

    <owl:ObjectProperty rdf:about="http://www.ontologydesignpatterns.org/ont/dul/DUL.owl#describes">
        <rdfs:subPropertyOf rdf:resource="http://www.ontologydesignpatterns.org/ont/dul/DUL.owl#associatedWith"/>
        <owl:inverseOf rdf:resource="http://www.ontologydesignpatterns.org/ont/dul/DUL.owl#isDescribedBy"/>
        <rdfs:domain rdf:resource="http://www.ontologydesignpatterns.org/ont/dul/DUL.owl#Description"/>
        <rdfs:range rdf:resource="http://www.ontologydesignpatterns.org/ont/dul/DUL.owl#Entity"/>
        <rdfs:comment>The relation between a Description and an Entity : a Description gives a unity to a Collection of parts (the components), or constituents, by assigning a Role to each of them in the context of a whole Object (the system).
A same Entity can be given different descriptions, for example, an old cradle can be given a unifying Description based on the original aesthetic design, the functionality it was built for, or a new aesthetic functionality in which it can be used as a flower pot.</rdfs:comment>
        <rdfs:isDefinedBy rdf:resource="http://www.ontologydesignpatterns.org/ont/dul/DUL.owl"/>
        <rdfs:label xml:lang="en">describes</rdfs:label>
        <rdfs:label xml:lang="it">descrive</rdfs:label>
    </owl:ObjectProperty>
    


    <!-- http://www.ontologydesignpatterns.org/ont/dul/DUL.owl#directlyFollows -->

    <owl:ObjectProperty rdf:about="http://www.ontologydesignpatterns.org/ont/dul/DUL.owl#directlyFollows">
        <rdfs:subPropertyOf rdf:resource="http://www.ontologydesignpatterns.org/ont/dul/DUL.owl#follows"/>
        <owl:inverseOf rdf:resource="http://www.ontologydesignpatterns.org/ont/dul/DUL.owl#directlyPrecedes"/>
        <rdfs:domain rdf:resource="http://www.ontologydesignpatterns.org/ont/dul/DUL.owl#Entity"/>
        <rdfs:range rdf:resource="http://www.ontologydesignpatterns.org/ont/dul/DUL.owl#Entity"/>
        <rdfs:comment>The intransitive follows relation. For example, Wednesday directly precedes Thursday. Directness of precedence depends on the designer conceptualization.</rdfs:comment>
        <rdfs:isDefinedBy rdf:resource="http://www.ontologydesignpatterns.org/ont/dul/DUL.owl"/>
        <rdfs:label xml:lang="en">directly follows</rdfs:label>
        <rdfs:label xml:lang="it">segue direttamente</rdfs:label>
    </owl:ObjectProperty>
    


    <!-- http://www.ontologydesignpatterns.org/ont/dul/DUL.owl#directlyPrecedes -->

    <owl:ObjectProperty rdf:about="http://www.ontologydesignpatterns.org/ont/dul/DUL.owl#directlyPrecedes">
        <rdfs:subPropertyOf rdf:resource="http://www.ontologydesignpatterns.org/ont/dul/DUL.owl#precedes"/>
        <rdfs:domain rdf:resource="http://www.ontologydesignpatterns.org/ont/dul/DUL.owl#Entity"/>
        <rdfs:range rdf:resource="http://www.ontologydesignpatterns.org/ont/dul/DUL.owl#Entity"/>
        <rdfs:comment>The intransitive precedes relation. For example, Monday directly precedes Tuesday. Directness of precedence depends on the designer conceptualization.</rdfs:comment>
        <rdfs:isDefinedBy rdf:resource="http://www.ontologydesignpatterns.org/ont/dul/DUL.owl"/>
        <rdfs:label xml:lang="en">directly precedes</rdfs:label>
        <rdfs:label xml:lang="it">precede direttamente</rdfs:label>
    </owl:ObjectProperty>
    


    <!-- http://www.ontologydesignpatterns.org/ont/dul/DUL.owl#executesTask -->

    <owl:ObjectProperty rdf:about="http://www.ontologydesignpatterns.org/ont/dul/DUL.owl#executesTask"/>
    


    <!-- http://www.ontologydesignpatterns.org/ont/dul/DUL.owl#follows -->

    <owl:ObjectProperty rdf:about="http://www.ontologydesignpatterns.org/ont/dul/DUL.owl#follows">
        <rdfs:subPropertyOf rdf:resource="http://www.ontologydesignpatterns.org/ont/dul/DUL.owl#associatedWith"/>
        <owl:inverseOf rdf:resource="http://www.ontologydesignpatterns.org/ont/dul/DUL.owl#precedes"/>
        <rdf:type rdf:resource="http://www.w3.org/2002/07/owl#TransitiveProperty"/>
        <rdfs:domain rdf:resource="http://www.ontologydesignpatterns.org/ont/dul/DUL.owl#Entity"/>
        <rdfs:range rdf:resource="http://www.ontologydesignpatterns.org/ont/dul/DUL.owl#Entity"/>
        <rdfs:comment>A relation between entities, expressing a &apos;sequence&apos; schema. 
E.g. &apos;year 2000 follows 1999&apos;, &apos;preparing coffee&apos; follows &apos;deciding what coffee to use&apos;, &apos;II World War follows I World War&apos;, etc. 
It can be used between tasks, processes or time intervals, and subproperties would fit best in order to distinguish the different uses.</rdfs:comment>
        <rdfs:isDefinedBy rdf:resource="http://www.ontologydesignpatterns.org/ont/dul/DUL.owl"/>
        <rdfs:label xml:lang="en">follows</rdfs:label>
        <rdfs:label xml:lang="it">segue</rdfs:label>
    </owl:ObjectProperty>
    


    <!-- http://www.ontologydesignpatterns.org/ont/dul/DUL.owl#hasComponent -->

    <owl:ObjectProperty rdf:about="http://www.ontologydesignpatterns.org/ont/dul/DUL.owl#hasComponent">
        <rdfs:subPropertyOf rdf:resource="http://www.ontologydesignpatterns.org/ont/dul/DUL.owl#hasProperPart"/>
        <owl:inverseOf rdf:resource="http://www.ontologydesignpatterns.org/ont/dul/DUL.owl#isComponentOf"/>
        <rdf:type rdf:resource="http://www.w3.org/2002/07/owl#AsymmetricProperty"/>
        <rdfs:domain rdf:resource="http://www.ontologydesignpatterns.org/ont/dul/DUL.owl#Entity"/>
        <rdfs:range rdf:resource="http://www.ontologydesignpatterns.org/ont/dul/DUL.owl#Entity"/>
        <rdfs:comment>The hasProperPart relation without transitivity, holding between an Object (the system) and another (the component), and assuming a Design that structures the Object.</rdfs:comment>
        <rdfs:isDefinedBy rdf:resource="http://www.ontologydesignpatterns.org/ont/dul/DUL.owl"/>
        <rdfs:label xml:lang="it">ha componente</rdfs:label>
        <rdfs:label xml:lang="en">has component</rdfs:label>
    </owl:ObjectProperty>
    


    <!-- http://www.ontologydesignpatterns.org/ont/dul/DUL.owl#hasConstituent -->

    <owl:ObjectProperty rdf:about="http://www.ontologydesignpatterns.org/ont/dul/DUL.owl#hasConstituent">
        <rdfs:subPropertyOf rdf:resource="http://www.ontologydesignpatterns.org/ont/dul/DUL.owl#associatedWith"/>
        <owl:inverseOf rdf:resource="http://www.ontologydesignpatterns.org/ont/dul/DUL.owl#isConstituentOf"/>
        <rdfs:domain rdf:resource="http://www.ontologydesignpatterns.org/ont/dul/DUL.owl#Entity"/>
        <rdfs:range rdf:resource="http://www.ontologydesignpatterns.org/ont/dul/DUL.owl#Entity"/>
        <rdfs:comment>&apos;Constituency&apos; depends on some layering of  the world described by the ontology. For example, scientific granularities (e.g. body-organ-tissue-cell) or ontological &apos;strata&apos; (e.g. social-mental-biological-physical) are  typical layerings. 
Intuitively, a constituent is a part belonging to a lower layer. Since layering is actually a partition of the world described by the ontology, constituents are not properly classified as parts, although this kinship can be intuitive for common sense.
A desirable advantage of this distinction is that we are able to talk e.g. of physical constituents of non-physical objects (e.g. systems), while this is not possible in terms of parts.
Example of are the persons constituting a social system, the molecules constituting a person, the atoms constituting a river, etc. 
In all these examples, we notice a typical discontinuity between the constituted and the constituent object: e.g. a social system is conceptualized at a different layer from the persons that constitute it, a person is conceptualized at a different layer from the molecules that constitute them, and a river is conceptualized at a different layer from the atoms that constitute it.</rdfs:comment>
        <rdfs:isDefinedBy rdf:resource="http://www.ontologydesignpatterns.org/ont/dul/DUL.owl"/>
        <rdfs:label xml:lang="it">ha costituente</rdfs:label>
        <rdfs:label xml:lang="en">has constituent</rdfs:label>
    </owl:ObjectProperty>
    


    <!-- http://www.ontologydesignpatterns.org/ont/dul/DUL.owl#hasLocation -->

    <owl:ObjectProperty rdf:about="http://www.ontologydesignpatterns.org/ont/dul/DUL.owl#hasLocation">
        <rdfs:subPropertyOf rdf:resource="http://www.ontologydesignpatterns.org/ont/dul/DUL.owl#associatedWith"/>
        <rdfs:domain rdf:resource="http://www.ontologydesignpatterns.org/ont/dul/DUL.owl#Entity"/>
        <rdfs:range rdf:resource="http://www.ontologydesignpatterns.org/ont/dul/DUL.owl#Entity"/>
        <rdfs:comment>A generic, relative spatial location, holding between any entities. E.g. &apos;the cat is on the mat&apos;, &apos;Omar is in Samarcanda&apos;, &apos;the wound is close to the femural artery&apos;.
For &apos;absolute&apos; locations, see SpaceRegion</rdfs:comment>
        <rdfs:isDefinedBy rdf:resource="http://www.ontologydesignpatterns.org/ont/dul/DUL.owl"/>
        <rdfs:label xml:lang="it">ha localizzazione</rdfs:label>
        <rdfs:label xml:lang="en">has location</rdfs:label>
    </owl:ObjectProperty>
    


    <!-- http://www.ontologydesignpatterns.org/ont/dul/DUL.owl#hasMember -->

    <owl:ObjectProperty rdf:about="http://www.ontologydesignpatterns.org/ont/dul/DUL.owl#hasMember">
        <rdfs:subPropertyOf rdf:resource="http://www.ontologydesignpatterns.org/ont/dul/DUL.owl#associatedWith"/>
        <owl:inverseOf rdf:resource="http://www.ontologydesignpatterns.org/ont/dul/DUL.owl#isMemberOf"/>
        <rdfs:domain rdf:resource="http://www.ontologydesignpatterns.org/ont/dul/DUL.owl#Collection"/>
        <rdfs:range rdf:resource="http://www.ontologydesignpatterns.org/ont/dul/DUL.owl#Entity"/>
        <rdfs:comment>A relation between collections and entities, e.g. &apos;my collection of saxophones includes an old Adolphe Sax original alto&apos; (i.e. my collection has member an Adolphe Sax alto).</rdfs:comment>
        <rdfs:isDefinedBy rdf:resource="http://www.ontologydesignpatterns.org/ont/dul/DUL.owl"/>
        <rdfs:label xml:lang="it">ha membro</rdfs:label>
        <rdfs:label xml:lang="en">has member</rdfs:label>
    </owl:ObjectProperty>
    


    <!-- http://www.ontologydesignpatterns.org/ont/dul/DUL.owl#hasPart -->

    <owl:ObjectProperty rdf:about="http://www.ontologydesignpatterns.org/ont/dul/DUL.owl#hasPart">
        <rdfs:subPropertyOf rdf:resource="http://www.ontologydesignpatterns.org/ont/dul/DUL.owl#associatedWith"/>
        <owl:inverseOf rdf:resource="http://www.ontologydesignpatterns.org/ont/dul/DUL.owl#isPartOf"/>
        <rdf:type rdf:resource="http://www.w3.org/2002/07/owl#TransitiveProperty"/>
        <rdfs:domain rdf:resource="http://www.ontologydesignpatterns.org/ont/dul/DUL.owl#Entity"/>
        <rdfs:range rdf:resource="http://www.ontologydesignpatterns.org/ont/dul/DUL.owl#Entity"/>
        <rdfs:comment>A schematic relation between any entities, e.g. &apos;the human body has a brain as part&apos;, &apos;20th century contains year 1923&apos;, &apos;World War II includes the Pearl Harbour event&apos;.

Parthood should assume the basic properties of mereology: transitivity, antisymmetry, and reflexivity (propert Parthood of course misses reflexivity). 
However, antisymmetry is not supported in OWL2 explicitly, therefore DUL has to adopt one of two patterns:
1) dropping asymmetry axioms, while granting reflexivity: this means that symmetry is not enforced, but permitted for the case of reflexivity. Of course, in this way we cannot prevent symmetric usages of hasPart;
2) dropping the reflexivity axiom, and enforce asymmetry: in this case, we would prevent all symmetric usages, but we loose the possibility of enforcing reflexivity, which is commonsensical in parthood.
In DUL, we adopt pattern #1 for partOf, and pattern #2 for properPartOf, which seems a good approximation: due to the lack of inheritance of property characteristics, each asymmetric hasPropertPart assertion would also be a reflexive hasPart assertion (reflexive reduction design pattern).

Subproperties and restrictions can be used to specialize hasPart for objects, events, etc.</rdfs:comment>
        <rdfs:isDefinedBy rdf:resource="http://www.ontologydesignpatterns.org/ont/dul/DUL.owl"/>
        <rdfs:label xml:lang="it">ha parte</rdfs:label>
        <rdfs:label xml:lang="en">has part</rdfs:label>
    </owl:ObjectProperty>
    


    <!-- http://www.ontologydesignpatterns.org/ont/dul/DUL.owl#hasParticipant -->

    <owl:ObjectProperty rdf:about="http://www.ontologydesignpatterns.org/ont/dul/DUL.owl#hasParticipant">
        <rdfs:subPropertyOf rdf:resource="http://www.ontologydesignpatterns.org/ont/dul/DUL.owl#associatedWith"/>
        <owl:inverseOf rdf:resource="http://www.ontologydesignpatterns.org/ont/dul/DUL.owl#isParticipantIn"/>
        <rdfs:domain rdf:resource="http://www.ontologydesignpatterns.org/ont/dul/DUL.owl#Event"/>
        <rdfs:range rdf:resource="http://www.ontologydesignpatterns.org/ont/dul/DUL.owl#Object"/>
        <rdfs:comment>A relation between an object and a process, e.g. &apos;John took part in the discussion&apos;, &apos;a large mass of snow fell during the avalanche&apos;, or &apos;a cook, some sugar, flour, etc. are all present in the cooking of a cake&apos;.</rdfs:comment>
        <rdfs:isDefinedBy rdf:resource="http://www.ontologydesignpatterns.org/ont/dul/DUL.owl"/>
        <rdfs:label xml:lang="it">ha come partecipante</rdfs:label>
        <rdfs:label xml:lang="en">has participant</rdfs:label>
    </owl:ObjectProperty>
    


    <!-- http://www.ontologydesignpatterns.org/ont/dul/DUL.owl#hasPostcondition -->

    <owl:ObjectProperty rdf:about="http://www.ontologydesignpatterns.org/ont/dul/DUL.owl#hasPostcondition">
        <rdfs:subPropertyOf rdf:resource="http://www.ontologydesignpatterns.org/ont/dul/DUL.owl#directlyPrecedes"/>
        <owl:inverseOf rdf:resource="http://www.ontologydesignpatterns.org/ont/dul/DUL.owl#isPostconditionOf"/>
        <rdfs:domain>
            <owl:Class>
                <owl:unionOf rdf:parseType="Collection">
                    <rdf:Description rdf:about="http://www.ontologydesignpatterns.org/ont/dul/DUL.owl#Event"/>
                    <rdf:Description rdf:about="http://www.ontologydesignpatterns.org/ont/dul/DUL.owl#Situation"/>
                </owl:unionOf>
            </owl:Class>
        </rdfs:domain>
        <rdfs:range>
            <owl:Class>
                <owl:unionOf rdf:parseType="Collection">
                    <rdf:Description rdf:about="http://www.ontologydesignpatterns.org/ont/dul/DUL.owl#Event"/>
                    <rdf:Description rdf:about="http://www.ontologydesignpatterns.org/ont/dul/DUL.owl#Situation"/>
                </owl:unionOf>
            </owl:Class>
        </rdfs:range>
        <rdfs:comment>Direct succession applied to situations. 
E.g., &apos;A postcondition of our Plan is to have things settled&apos;.</rdfs:comment>
        <rdfs:isDefinedBy rdf:resource="http://www.ontologydesignpatterns.org/ont/dul/DUL.owl"/>
        <rdfs:label xml:lang="it">ha postcondizione</rdfs:label>
        <rdfs:label xml:lang="en">has postcondition</rdfs:label>
    </owl:ObjectProperty>
    


    <!-- http://www.ontologydesignpatterns.org/ont/dul/DUL.owl#hasPrecondition -->

    <owl:ObjectProperty rdf:about="http://www.ontologydesignpatterns.org/ont/dul/DUL.owl#hasPrecondition">
        <rdfs:subPropertyOf rdf:resource="http://www.ontologydesignpatterns.org/ont/dul/DUL.owl#directlyFollows"/>
        <owl:inverseOf rdf:resource="http://www.ontologydesignpatterns.org/ont/dul/DUL.owl#isPreconditionOf"/>
        <rdfs:domain>
            <owl:Class>
                <owl:unionOf rdf:parseType="Collection">
                    <rdf:Description rdf:about="http://www.ontologydesignpatterns.org/ont/dul/DUL.owl#Event"/>
                    <rdf:Description rdf:about="http://www.ontologydesignpatterns.org/ont/dul/DUL.owl#Situation"/>
                </owl:unionOf>
            </owl:Class>
        </rdfs:domain>
        <rdfs:range>
            <owl:Class>
                <owl:unionOf rdf:parseType="Collection">
                    <rdf:Description rdf:about="http://www.ontologydesignpatterns.org/ont/dul/DUL.owl#Event"/>
                    <rdf:Description rdf:about="http://www.ontologydesignpatterns.org/ont/dul/DUL.owl#Situation"/>
                </owl:unionOf>
            </owl:Class>
        </rdfs:range>
        <rdfs:comment>Direct precedence applied to situations. 
E.g., &apos;A precondition to declare war against a foreign country is claiming to find nuclear weapons in it&apos;.</rdfs:comment>
        <rdfs:isDefinedBy rdf:resource="http://www.ontologydesignpatterns.org/ont/dul/DUL.owl"/>
        <rdfs:label xml:lang="it">ha precondizione</rdfs:label>
        <rdfs:label xml:lang="en">has precondition</rdfs:label>
    </owl:ObjectProperty>
    


    <!-- http://www.ontologydesignpatterns.org/ont/dul/DUL.owl#hasProperPart -->

    <owl:ObjectProperty rdf:about="http://www.ontologydesignpatterns.org/ont/dul/DUL.owl#hasProperPart">
        <rdfs:subPropertyOf rdf:resource="http://www.ontologydesignpatterns.org/ont/dul/DUL.owl#hasPart"/>
        <owl:inverseOf rdf:resource="http://www.ontologydesignpatterns.org/ont/dul/DUL.owl#isPropertPartOf"/>
        <rdf:type rdf:resource="http://www.w3.org/2002/07/owl#TransitiveProperty"/>
        <rdfs:comment>Asymmetric (so including irreflexive) parthood.</rdfs:comment>
        <rdfs:label>has proper part</rdfs:label>
        <rdfs:label xml:lang="en">has proper part</rdfs:label>
    </owl:ObjectProperty>
    


    <!-- http://www.ontologydesignpatterns.org/ont/dul/DUL.owl#hasRegion -->

    <owl:ObjectProperty rdf:about="http://www.ontologydesignpatterns.org/ont/dul/DUL.owl#hasRegion">
        <rdfs:subPropertyOf rdf:resource="http://www.ontologydesignpatterns.org/ont/dul/DUL.owl#associatedWith"/>
        <owl:inverseOf rdf:resource="http://www.ontologydesignpatterns.org/ont/dul/DUL.owl#isRegionFor"/>
        <rdfs:domain rdf:resource="http://www.ontologydesignpatterns.org/ont/dul/DUL.owl#Entity"/>
        <rdfs:range rdf:resource="http://www.ontologydesignpatterns.org/ont/dul/DUL.owl#Region"/>
        <rdfs:comment>A relation between entities and regions, e.g. &apos;the number of wheels of that truck is 12&apos;, &apos;the time of the experiment is August 9th, 2004&apos;, &apos;the whale has been localized at 34 degrees E, 20 degrees S&apos;.</rdfs:comment>
        <rdfs:isDefinedBy rdf:resource="http://www.ontologydesignpatterns.org/ont/dul/DUL.owl"/>
        <rdfs:label xml:lang="it">ha attributo</rdfs:label>
        <rdfs:label>has region</rdfs:label>
        <rdfs:label xml:lang="en">has region</rdfs:label>
    </owl:ObjectProperty>
    


    <!-- http://www.ontologydesignpatterns.org/ont/dul/DUL.owl#hasSetting -->

    <owl:ObjectProperty rdf:about="http://www.ontologydesignpatterns.org/ont/dul/DUL.owl#hasSetting">
        <rdfs:subPropertyOf rdf:resource="http://www.ontologydesignpatterns.org/ont/dul/DUL.owl#associatedWith"/>
        <owl:inverseOf rdf:resource="http://www.ontologydesignpatterns.org/ont/dul/DUL.owl#isSettingFor"/>
        <rdfs:domain rdf:resource="http://www.ontologydesignpatterns.org/ont/dul/DUL.owl#Entity"/>
        <rdfs:range rdf:resource="http://www.ontologydesignpatterns.org/ont/dul/DUL.owl#Situation"/>
        <rdfs:comment>A relation between entities and situations, e.g. &apos;this morning I&apos;ve prepared my coffee with a new fantastic Arabica&apos;, i.e.: (an amount of) a new fantastic Arabica hasSetting the preparation of my coffee this morning.</rdfs:comment>
        <rdfs:isDefinedBy rdf:resource="http://www.ontologydesignpatterns.org/ont/dul/DUL.owl"/>
        <rdfs:label>has setting</rdfs:label>
        <rdfs:label xml:lang="en">has setting</rdfs:label>
        <rdfs:label xml:lang="it">è nel contesto di</rdfs:label>
    </owl:ObjectProperty>
    


    <!-- http://www.ontologydesignpatterns.org/ont/dul/DUL.owl#hasTimeInterval -->

    <owl:ObjectProperty rdf:about="http://www.ontologydesignpatterns.org/ont/dul/DUL.owl#hasTimeInterval">
        <rdfs:subPropertyOf rdf:resource="http://www.ontologydesignpatterns.org/ont/dul/DUL.owl#hasRegion"/>
        <owl:inverseOf rdf:resource="http://www.ontologydesignpatterns.org/ont/dul/DUL.owl#isTimeIntervalOf"/>
        <rdfs:domain rdf:resource="http://www.ontologydesignpatterns.org/ont/dul/DUL.owl#Event"/>
        <rdfs:range rdf:resource="http://www.ontologydesignpatterns.org/ont/dul/DUL.owl#TimeInterval"/>
        <rdfs:comment xml:lang="en">The generic relation between events and time intervals.</rdfs:comment>
        <rdfs:isDefinedBy rdf:resource="http://www.ontologydesignpatterns.org/ont/dul/DUL.owl"/>
        <rdfs:label xml:lang="it">ha intervallo temporale</rdfs:label>
        <rdfs:label xml:lang="en">has time interval</rdfs:label>
    </owl:ObjectProperty>
    


    <!-- http://www.ontologydesignpatterns.org/ont/dul/DUL.owl#involvesAgent -->

    <owl:ObjectProperty rdf:about="http://www.ontologydesignpatterns.org/ont/dul/DUL.owl#involvesAgent">
        <rdfs:subPropertyOf rdf:resource="http://www.ontologydesignpatterns.org/ont/dul/DUL.owl#hasParticipant"/>
        <owl:inverseOf rdf:resource="http://www.ontologydesignpatterns.org/ont/dul/DUL.owl#isAgentInvolvedIn"/>
        <rdfs:domain rdf:resource="http://www.ontologydesignpatterns.org/ont/dul/DUL.owl#Event"/>
        <rdfs:range rdf:resource="http://www.ontologydesignpatterns.org/ont/dul/DUL.owl#Agent"/>
        <rdfs:comment>Agent participation.</rdfs:comment>
        <rdfs:isDefinedBy rdf:resource="http://www.ontologydesignpatterns.org/ont/dul/DUL.owl"/>
        <rdfs:label xml:lang="it">coinvolge agente</rdfs:label>
        <rdfs:label xml:lang="en">involves agent</rdfs:label>
    </owl:ObjectProperty>
    


    <!-- http://www.ontologydesignpatterns.org/ont/dul/DUL.owl#isAgentInvolvedIn -->

    <owl:ObjectProperty rdf:about="http://www.ontologydesignpatterns.org/ont/dul/DUL.owl#isAgentInvolvedIn">
        <rdfs:subPropertyOf rdf:resource="http://www.ontologydesignpatterns.org/ont/dul/DUL.owl#isParticipantIn"/>
        <rdfs:domain rdf:resource="http://www.ontologydesignpatterns.org/ont/dul/DUL.owl#Agent"/>
        <rdfs:range rdf:resource="http://www.ontologydesignpatterns.org/ont/dul/DUL.owl#Event"/>
        <rdfs:comment>Agent participation.</rdfs:comment>
        <rdfs:isDefinedBy rdf:resource="http://www.ontologydesignpatterns.org/ont/dul/DUL.owl"/>
        <rdfs:label xml:lang="en">is agent involved in</rdfs:label>
        <rdfs:label xml:lang="it">è un agente coinvolto in</rdfs:label>
    </owl:ObjectProperty>
    


    <!-- http://www.ontologydesignpatterns.org/ont/dul/DUL.owl#isComponentOf -->

    <owl:ObjectProperty rdf:about="http://www.ontologydesignpatterns.org/ont/dul/DUL.owl#isComponentOf">
        <rdfs:subPropertyOf rdf:resource="http://www.ontologydesignpatterns.org/ont/dul/DUL.owl#isPropertPartOf"/>
        <rdf:type rdf:resource="http://www.w3.org/2002/07/owl#AsymmetricProperty"/>
        <rdfs:domain rdf:resource="http://www.ontologydesignpatterns.org/ont/dul/DUL.owl#Entity"/>
        <rdfs:range rdf:resource="http://www.ontologydesignpatterns.org/ont/dul/DUL.owl#Entity"/>
        <rdfs:comment>The asymmetric isProperPartOf relation without transitivity, holding between an Object (the system) and another (the component), and assuming a Design that structures the Object.</rdfs:comment>
        <rdfs:isDefinedBy rdf:resource="http://www.ontologydesignpatterns.org/ont/dul/DUL.owl"/>
        <rdfs:label xml:lang="en">is component of</rdfs:label>
        <rdfs:label xml:lang="it">è componente di</rdfs:label>
    </owl:ObjectProperty>
    


    <!-- http://www.ontologydesignpatterns.org/ont/dul/DUL.owl#isConceptualizedBy -->

    <owl:ObjectProperty rdf:about="http://www.ontologydesignpatterns.org/ont/dul/DUL.owl#isConceptualizedBy">
        <rdfs:subPropertyOf rdf:resource="http://www.ontologydesignpatterns.org/ont/dul/DUL.owl#associatedWith"/>
        <rdfs:domain rdf:resource="http://www.ontologydesignpatterns.org/ont/dul/DUL.owl#SocialObject"/>
        <rdfs:range rdf:resource="http://www.ontologydesignpatterns.org/ont/dul/DUL.owl#Agent"/>
        <rdfs:comment>A relation stating that an Agent is internally representing a Description . E.g., &apos;John believes in the conspiracy theory&apos;; &apos;Niels Bohr created a solar-system metaphor for his atomic theory&apos;; &apos;Jacques assumes all swans are white&apos;; &apos;the task force shares the attack plan&apos;.</rdfs:comment>
        <rdfs:isDefinedBy rdf:resource="http://www.ontologydesignpatterns.org/ont/dul/DUL.owl"/>
        <rdfs:label xml:lang="en">is conceptualized by</rdfs:label>
        <rdfs:label xml:lang="it">è concettualizzato da</rdfs:label>
    </owl:ObjectProperty>
    


    <!-- http://www.ontologydesignpatterns.org/ont/dul/DUL.owl#isConstituentOf -->

    <owl:ObjectProperty rdf:about="http://www.ontologydesignpatterns.org/ont/dul/DUL.owl#isConstituentOf">
        <rdfs:subPropertyOf rdf:resource="http://www.ontologydesignpatterns.org/ont/dul/DUL.owl#associatedWith"/>
        <rdfs:domain rdf:resource="http://www.ontologydesignpatterns.org/ont/dul/DUL.owl#Entity"/>
        <rdfs:range rdf:resource="http://www.ontologydesignpatterns.org/ont/dul/DUL.owl#Entity"/>
        <rdfs:comment>&apos;Constituency&apos; depends on some layering of  the world described by the ontology. For example, scientific granularities (e.g. body-organ-tissue-cell) or ontological &apos;strata&apos; (e.g. social-mental-biological-physical) are  typical layerings. 
Intuitively, a constituent is a part belonging to a lower layer. Since layering is actually a partition of the world described by the ontology, constituents are not properly classified as parts, although this kinship can be intuitive for common sense.
A desirable advantage of this distinction is that we are able to talk e.g. of physical constituents of non-physical objects (e.g. systems), while this is not possible in terms of parts.
Example of are the persons constituting a social system, the molecules constituting a person, the atoms constituting a river, etc. 
In all these examples, we notice a typical discontinuity between the constituted and the constituent object: e.g. a social system is conceptualized at a different layer from the persons that constitute it, a person is conceptualized at a different layer from the molecules that constitute them, and a river is conceptualized at a different layer from the atoms that constitute it.</rdfs:comment>
        <rdfs:isDefinedBy rdf:resource="http://www.ontologydesignpatterns.org/ont/dul/DUL.owl"/>
        <rdfs:label xml:lang="en">is constituent of</rdfs:label>
        <rdfs:label xml:lang="it">è costituente di</rdfs:label>
    </owl:ObjectProperty>
    


    <!-- http://www.ontologydesignpatterns.org/ont/dul/DUL.owl#isDescribedBy -->

    <owl:ObjectProperty rdf:about="http://www.ontologydesignpatterns.org/ont/dul/DUL.owl#isDescribedBy">
        <rdfs:subPropertyOf rdf:resource="http://www.ontologydesignpatterns.org/ont/dul/DUL.owl#associatedWith"/>
        <rdfs:domain rdf:resource="http://www.ontologydesignpatterns.org/ont/dul/DUL.owl#Entity"/>
        <rdfs:range rdf:resource="http://www.ontologydesignpatterns.org/ont/dul/DUL.owl#Description"/>
        <rdfs:comment>The relation between an Entity and a Description: a Description gives a unity to a Collection of parts (the components), or constituents, by assigning a Role to each of them in the context of a whole Object (the system).
A same Entity can be given different descriptions, for example, an old cradle can be given a unifying Description based on the original aesthetic design, the functionality it was built for, or a new aesthetic functionality in which it can be used as a flower pot.</rdfs:comment>
        <rdfs:isDefinedBy rdf:resource="http://www.ontologydesignpatterns.org/ont/dul/DUL.owl"/>
        <rdfs:label xml:lang="en">is described by</rdfs:label>
        <rdfs:label xml:lang="it">è descritto da</rdfs:label>
    </owl:ObjectProperty>
    


    <!-- http://www.ontologydesignpatterns.org/ont/dul/DUL.owl#isMemberOf -->

    <owl:ObjectProperty rdf:about="http://www.ontologydesignpatterns.org/ont/dul/DUL.owl#isMemberOf">
        <rdfs:subPropertyOf rdf:resource="http://www.ontologydesignpatterns.org/ont/dul/DUL.owl#associatedWith"/>
        <rdfs:domain rdf:resource="http://www.ontologydesignpatterns.org/ont/dul/DUL.owl#Entity"/>
        <rdfs:range rdf:resource="http://www.ontologydesignpatterns.org/ont/dul/DUL.owl#Collection"/>
        <rdfs:comment>A relation between collections and entities, e.g. &apos;the Night Watch by Rembrandt is in the Rijksmuseum collection&apos;; &apos;Davide is member of the Pen Club&apos;, &apos;Igor is one the subjects chosen for the experiment&apos;.</rdfs:comment>
        <rdfs:isDefinedBy rdf:resource="http://www.ontologydesignpatterns.org/ont/dul/DUL.owl"/>
        <rdfs:label xml:lang="en">is member of</rdfs:label>
        <rdfs:label xml:lang="it">è membro di</rdfs:label>
    </owl:ObjectProperty>
    


    <!-- http://www.ontologydesignpatterns.org/ont/dul/DUL.owl#isObservableAt -->

    <owl:ObjectProperty rdf:about="http://www.ontologydesignpatterns.org/ont/dul/DUL.owl#isObservableAt">
        <rdfs:subPropertyOf rdf:resource="http://www.ontologydesignpatterns.org/ont/dul/DUL.owl#hasRegion"/>
        <owl:inverseOf rdf:resource="http://www.ontologydesignpatterns.org/ont/dul/DUL.owl#isTimeOfObservationOf"/>
        <rdfs:domain rdf:resource="http://www.ontologydesignpatterns.org/ont/dul/DUL.owl#Entity"/>
        <rdfs:range rdf:resource="http://www.ontologydesignpatterns.org/ont/dul/DUL.owl#TimeInterval"/>
        <rdfs:comment>A relation to represent a (past, present or future) TimeInterval at which an Entity is observable.
In order to encode a specific time, a data value should be related to the TimeInterval. 
An alternative way of representing time is the datatype property: hasIntervalDate</rdfs:comment>
        <rdfs:isDefinedBy rdf:resource="http://www.ontologydesignpatterns.org/ont/dul/DUL.owl"/>
        <rdfs:label xml:lang="en">is observable at</rdfs:label>
        <rdfs:label xml:lang="it">è osservabile a</rdfs:label>
    </owl:ObjectProperty>
    


    <!-- http://www.ontologydesignpatterns.org/ont/dul/DUL.owl#isPartOf -->

    <owl:ObjectProperty rdf:about="http://www.ontologydesignpatterns.org/ont/dul/DUL.owl#isPartOf">
        <rdfs:subPropertyOf rdf:resource="http://www.ontologydesignpatterns.org/ont/dul/DUL.owl#associatedWith"/>
        <rdf:type rdf:resource="http://www.w3.org/2002/07/owl#TransitiveProperty"/>
        <rdfs:domain rdf:resource="http://www.ontologydesignpatterns.org/ont/dul/DUL.owl#Entity"/>
        <rdfs:range rdf:resource="http://www.ontologydesignpatterns.org/ont/dul/DUL.owl#Entity"/>
        <rdfs:comment>A relation between any entities, e.g. &apos;brain is a part of the human body&apos;. See dul:hasPart for additional documentation.</rdfs:comment>
        <rdfs:isDefinedBy rdf:resource="http://www.ontologydesignpatterns.org/ont/dul/DUL.owl"/>
        <rdfs:label xml:lang="en">is part of</rdfs:label>
        <rdfs:label xml:lang="it">è parte di</rdfs:label>
    </owl:ObjectProperty>
    


    <!-- http://www.ontologydesignpatterns.org/ont/dul/DUL.owl#isParticipantIn -->

    <owl:ObjectProperty rdf:about="http://www.ontologydesignpatterns.org/ont/dul/DUL.owl#isParticipantIn">
        <rdfs:subPropertyOf rdf:resource="http://www.ontologydesignpatterns.org/ont/dul/DUL.owl#associatedWith"/>
        <rdfs:domain rdf:resource="http://www.ontologydesignpatterns.org/ont/dul/DUL.owl#Object"/>
        <rdfs:range rdf:resource="http://www.ontologydesignpatterns.org/ont/dul/DUL.owl#Event"/>
        <rdfs:comment>A relation between an object and a process, e.g. &apos;John took part in the discussion&apos;, &apos;a large mass of snow fell during the avalanche&apos;, or &apos;a cook, some sugar, flour, etc. are all present in the cooking of a cake&apos;.</rdfs:comment>
        <rdfs:isDefinedBy rdf:resource="http://www.ontologydesignpatterns.org/ont/dul/DUL.owl"/>
        <rdfs:label>is participant in</rdfs:label>
        <rdfs:label xml:lang="en">is participant in</rdfs:label>
        <rdfs:label xml:lang="it">è un partecipante a</rdfs:label>
    </owl:ObjectProperty>
    


    <!-- http://www.ontologydesignpatterns.org/ont/dul/DUL.owl#isPostconditionOf -->

    <owl:ObjectProperty rdf:about="http://www.ontologydesignpatterns.org/ont/dul/DUL.owl#isPostconditionOf">
        <rdfs:subPropertyOf rdf:resource="http://www.ontologydesignpatterns.org/ont/dul/DUL.owl#directlyFollows"/>
        <rdfs:domain>
            <owl:Class>
                <owl:unionOf rdf:parseType="Collection">
                    <rdf:Description rdf:about="http://www.ontologydesignpatterns.org/ont/dul/DUL.owl#Event"/>
                    <rdf:Description rdf:about="http://www.ontologydesignpatterns.org/ont/dul/DUL.owl#Situation"/>
                </owl:unionOf>
            </owl:Class>
        </rdfs:domain>
        <rdfs:range>
            <owl:Class>
                <owl:unionOf rdf:parseType="Collection">
                    <rdf:Description rdf:about="http://www.ontologydesignpatterns.org/ont/dul/DUL.owl#Event"/>
                    <rdf:Description rdf:about="http://www.ontologydesignpatterns.org/ont/dul/DUL.owl#Situation"/>
                </owl:unionOf>
            </owl:Class>
        </rdfs:range>
        <rdfs:comment>Direct succession applied to situations. 
E.g., &apos;Taking some rest is a postcondition of my search for a hotel&apos;.</rdfs:comment>
        <rdfs:isDefinedBy rdf:resource="http://www.ontologydesignpatterns.org/ont/dul/DUL.owl"/>
        <rdfs:label xml:lang="en">is postcondition of</rdfs:label>
        <rdfs:label xml:lang="it">è postcondizione di</rdfs:label>
    </owl:ObjectProperty>
    


    <!-- http://www.ontologydesignpatterns.org/ont/dul/DUL.owl#isPreconditionOf -->

    <owl:ObjectProperty rdf:about="http://www.ontologydesignpatterns.org/ont/dul/DUL.owl#isPreconditionOf">
        <rdfs:subPropertyOf rdf:resource="http://www.ontologydesignpatterns.org/ont/dul/DUL.owl#directlyPrecedes"/>
        <rdfs:domain>
            <owl:Class>
                <owl:unionOf rdf:parseType="Collection">
                    <rdf:Description rdf:about="http://www.ontologydesignpatterns.org/ont/dul/DUL.owl#Event"/>
                    <rdf:Description rdf:about="http://www.ontologydesignpatterns.org/ont/dul/DUL.owl#Situation"/>
                </owl:unionOf>
            </owl:Class>
        </rdfs:domain>
        <rdfs:range>
            <owl:Class>
                <owl:unionOf rdf:parseType="Collection">
                    <rdf:Description rdf:about="http://www.ontologydesignpatterns.org/ont/dul/DUL.owl#Event"/>
                    <rdf:Description rdf:about="http://www.ontologydesignpatterns.org/ont/dul/DUL.owl#Situation"/>
                </owl:unionOf>
            </owl:Class>
        </rdfs:range>
        <rdfs:comment>Direct precedence applied to situations. 
E.g., &apos;claiming to find nuclear weapons in a foreign country is a precondition to declare war against it&apos;.</rdfs:comment>
        <rdfs:isDefinedBy rdf:resource="http://www.ontologydesignpatterns.org/ont/dul/DUL.owl"/>
        <rdfs:label xml:lang="en">is precondition of</rdfs:label>
        <rdfs:label xml:lang="it">è precondizione di</rdfs:label>
    </owl:ObjectProperty>
    


    <!-- http://www.ontologydesignpatterns.org/ont/dul/DUL.owl#isPropertPartOf -->

    <owl:ObjectProperty rdf:about="http://www.ontologydesignpatterns.org/ont/dul/DUL.owl#isPropertPartOf">
        <rdfs:subPropertyOf rdf:resource="http://www.ontologydesignpatterns.org/ont/dul/DUL.owl#isPartOf"/>
        <rdf:type rdf:resource="http://www.w3.org/2002/07/owl#TransitiveProperty"/>
        <rdfs:comment xml:lang="en">See dul:hasProperPart for additional documentation.</rdfs:comment>
        <rdfs:label xml:lang="en">is propert part of</rdfs:label>
    </owl:ObjectProperty>
    


    <!-- http://www.ontologydesignpatterns.org/ont/dul/DUL.owl#isRegionFor -->

    <owl:ObjectProperty rdf:about="http://www.ontologydesignpatterns.org/ont/dul/DUL.owl#isRegionFor">
        <rdfs:subPropertyOf rdf:resource="http://www.ontologydesignpatterns.org/ont/dul/DUL.owl#associatedWith"/>
        <rdfs:domain rdf:resource="http://www.ontologydesignpatterns.org/ont/dul/DUL.owl#Region"/>
        <rdfs:range rdf:resource="http://www.ontologydesignpatterns.org/ont/dul/DUL.owl#Entity"/>
        <rdfs:comment>A relation between entities and regions, e.g. &apos;the color of my car is red&apos;.</rdfs:comment>
        <rdfs:isDefinedBy rdf:resource="http://www.ontologydesignpatterns.org/ont/dul/DUL.owl"/>
        <rdfs:label xml:lang="en">is region for</rdfs:label>
        <rdfs:label xml:lang="it">è una regione di</rdfs:label>
    </owl:ObjectProperty>
    


    <!-- http://www.ontologydesignpatterns.org/ont/dul/DUL.owl#isSatisfiedBy -->

    <owl:ObjectProperty rdf:about="http://www.ontologydesignpatterns.org/ont/dul/DUL.owl#isSatisfiedBy">
        <rdfs:subPropertyOf rdf:resource="http://www.ontologydesignpatterns.org/ont/dul/DUL.owl#associatedWith"/>
        <owl:inverseOf rdf:resource="http://www.ontologydesignpatterns.org/ont/dul/DUL.owl#satisfies"/>
        <rdfs:domain rdf:resource="http://www.ontologydesignpatterns.org/ont/dul/DUL.owl#Description"/>
        <rdfs:range rdf:resource="http://www.ontologydesignpatterns.org/ont/dul/DUL.owl#Situation"/>
        <rdfs:comment>A relation between a Situation and a Description, e.g. the execution of a Plan satisfies that plan.</rdfs:comment>
        <rdfs:isDefinedBy rdf:resource="http://www.ontologydesignpatterns.org/ont/dul/DUL.owl"/>
        <rdfs:label xml:lang="en">is satisfied by</rdfs:label>
        <rdfs:label xml:lang="it">è soddisfatta da</rdfs:label>
    </owl:ObjectProperty>
    


    <!-- http://www.ontologydesignpatterns.org/ont/dul/DUL.owl#isSettingFor -->

    <owl:ObjectProperty rdf:about="http://www.ontologydesignpatterns.org/ont/dul/DUL.owl#isSettingFor">
        <rdfs:subPropertyOf rdf:resource="http://www.ontologydesignpatterns.org/ont/dul/DUL.owl#associatedWith"/>
        <rdfs:domain rdf:resource="http://www.ontologydesignpatterns.org/ont/dul/DUL.owl#Situation"/>
        <rdfs:range rdf:resource="http://www.ontologydesignpatterns.org/ont/dul/DUL.owl#Entity"/>
        <rdfs:comment>A relation between situations and entities, e.g. &apos;this morning I&apos;ve prepared my coffee with a new fantastic Arabica&apos;, i.e.: the preparation of my coffee this morning is the setting for (an amount of) a new fantastic Arabica.</rdfs:comment>
        <rdfs:isDefinedBy rdf:resource="http://www.ontologydesignpatterns.org/ont/dul/DUL.owl"/>
        <rdfs:label xml:lang="it">include</rdfs:label>
        <rdfs:label xml:lang="en">is setting for</rdfs:label>
    </owl:ObjectProperty>
    


    <!-- http://www.ontologydesignpatterns.org/ont/dul/DUL.owl#isSubordinatedTo -->

    <owl:ObjectProperty rdf:about="http://www.ontologydesignpatterns.org/ont/dul/DUL.owl#isSubordinatedTo">
        <rdfs:subPropertyOf rdf:resource="http://www.ontologydesignpatterns.org/ont/dul/DUL.owl#directlyFollows"/>
    </owl:ObjectProperty>
    


    <!-- http://www.ontologydesignpatterns.org/ont/dul/DUL.owl#isSuperordinatedTo -->

    <owl:ObjectProperty rdf:about="http://www.ontologydesignpatterns.org/ont/dul/DUL.owl#isSuperordinatedTo">
        <rdfs:subPropertyOf rdf:resource="http://www.ontologydesignpatterns.org/ont/dul/DUL.owl#directlyPrecedes"/>
    </owl:ObjectProperty>
    


    <!-- http://www.ontologydesignpatterns.org/ont/dul/DUL.owl#isTimeIntervalOf -->

    <owl:ObjectProperty rdf:about="http://www.ontologydesignpatterns.org/ont/dul/DUL.owl#isTimeIntervalOf">
        <rdfs:subPropertyOf rdf:resource="http://www.ontologydesignpatterns.org/ont/dul/DUL.owl#isRegionFor"/>
        <rdfs:domain rdf:resource="http://www.ontologydesignpatterns.org/ont/dul/DUL.owl#TimeInterval"/>
        <rdfs:range rdf:resource="http://www.ontologydesignpatterns.org/ont/dul/DUL.owl#Event"/>
        <rdfs:comment xml:lang="en">The generic relation between time intervals and events.</rdfs:comment>
        <rdfs:isDefinedBy rdf:resource="http://www.ontologydesignpatterns.org/ont/dul/DUL.owl"/>
        <rdfs:label xml:lang="it">intervallo temporale di</rdfs:label>
        <rdfs:label xml:lang="en">is time interval of</rdfs:label>
    </owl:ObjectProperty>
    


    <!-- http://www.ontologydesignpatterns.org/ont/dul/DUL.owl#isTimeOfObservationOf -->

    <owl:ObjectProperty rdf:about="http://www.ontologydesignpatterns.org/ont/dul/DUL.owl#isTimeOfObservationOf">
        <rdfs:subPropertyOf rdf:resource="http://www.ontologydesignpatterns.org/ont/dul/DUL.owl#isRegionFor"/>
        <rdfs:domain rdf:resource="http://www.ontologydesignpatterns.org/ont/dul/DUL.owl#TimeInterval"/>
        <rdfs:range rdf:resource="http://www.ontologydesignpatterns.org/ont/dul/DUL.owl#Entity"/>
        <rdfs:comment>A relation to represent a (past, present or future) TimeInterval at which an Entity is observable.
In order to encode a specific time, a data value should be related to the TimeInterval. 
An alternative way of representing time is the datatype property: hasIntervalDate</rdfs:comment>
        <rdfs:isDefinedBy rdf:resource="http://www.ontologydesignpatterns.org/ont/dul/DUL.owl"/>
        <rdfs:label xml:lang="en">is time of observation of</rdfs:label>
        <rdfs:label xml:lang="it">è il tempo di osservazione di</rdfs:label>
    </owl:ObjectProperty>
    


    <!-- http://www.ontologydesignpatterns.org/ont/dul/DUL.owl#precedes -->

    <owl:ObjectProperty rdf:about="http://www.ontologydesignpatterns.org/ont/dul/DUL.owl#precedes">
        <rdfs:subPropertyOf rdf:resource="http://www.ontologydesignpatterns.org/ont/dul/DUL.owl#associatedWith"/>
        <rdf:type rdf:resource="http://www.w3.org/2002/07/owl#TransitiveProperty"/>
        <rdfs:domain rdf:resource="http://www.ontologydesignpatterns.org/ont/dul/DUL.owl#Entity"/>
        <rdfs:range rdf:resource="http://www.ontologydesignpatterns.org/ont/dul/DUL.owl#Entity"/>
        <rdfs:comment>A relation between entities, expressing a &apos;sequence&apos; schema. 
E.g. &apos;year 1999 precedes 2000&apos;, &apos;deciding what coffee to use&apos; precedes &apos;preparing coffee&apos;, &apos;World War II follows World War I&apos;, &apos;in the Milan to Rome autoroute, Bologna precedes Florence&apos;, etc.
It can then be used between tasks, processes, time intervals, spatially locate objects, situations, etc. 
Subproperties can be defined in order to distinguish the different uses.</rdfs:comment>
        <rdfs:isDefinedBy rdf:resource="http://www.ontologydesignpatterns.org/ont/dul/DUL.owl"/>
        <rdfs:label xml:lang="it">precede</rdfs:label>
        <rdfs:label xml:lang="en">precedes</rdfs:label>
    </owl:ObjectProperty>
    


    <!-- http://www.ontologydesignpatterns.org/ont/dul/DUL.owl#satisfies -->

    <owl:ObjectProperty rdf:about="http://www.ontologydesignpatterns.org/ont/dul/DUL.owl#satisfies">
        <rdfs:subPropertyOf rdf:resource="http://www.ontologydesignpatterns.org/ont/dul/DUL.owl#associatedWith"/>
        <rdfs:domain rdf:resource="http://www.ontologydesignpatterns.org/ont/dul/DUL.owl#Situation"/>
        <rdfs:range rdf:resource="http://www.ontologydesignpatterns.org/ont/dul/DUL.owl#Description"/>
        <rdfs:comment>A relation between a Situation and a Description, e.g. the execution of a Plan satisfies that plan.</rdfs:comment>
        <rdfs:isDefinedBy rdf:resource="http://www.ontologydesignpatterns.org/ont/dul/DUL.owl"/>
        <rdfs:label>satisfies</rdfs:label>
        <rdfs:label xml:lang="en">satisfies</rdfs:label>
        <rdfs:label xml:lang="it">soddisfa</rdfs:label>
    </owl:ObjectProperty>
    


    <!-- http://www.w3.org/ns/odrl/2/action -->

    <owl:ObjectProperty rdf:about="http://www.w3.org/ns/odrl/2/action">
        <rdfs:domain>
            <owl:Class>
                <owl:unionOf rdf:parseType="Collection">
                    <rdf:Description rdf:about="http://www.w3.org/ns/odrl/2/Policy"/>
                    <rdf:Description rdf:about="http://www.w3.org/ns/odrl/2/Rule"/>
                </owl:unionOf>
            </owl:Class>
        </rdfs:domain>
        <rdfs:range rdf:resource="http://www.w3.org/ns/odrl/2/Action"/>
        <rdfs:isDefinedBy rdf:resource="http://www.w3.org/ns/odrl/2/"/>
        <rdfs:label xml:lang="en">Has Action</rdfs:label>
        <rdfs:label>action</rdfs:label>
        <skos:definition xml:lang="en">The operation relating to the Asset for which the Rule is being subjected.</skos:definition>
    </owl:ObjectProperty>
    


    <!-- http://www.w3.org/ns/odrl/2/assignee -->

    <owl:ObjectProperty rdf:about="http://www.w3.org/ns/odrl/2/assignee">
        <rdfs:subPropertyOf rdf:resource="http://www.w3.org/ns/odrl/2/function"/>
        <rdfs:domain>
            <owl:Class>
                <owl:unionOf rdf:parseType="Collection">
                    <rdf:Description rdf:about="http://www.w3.org/ns/odrl/2/Policy"/>
                    <rdf:Description rdf:about="http://www.w3.org/ns/odrl/2/Rule"/>
                </owl:unionOf>
            </owl:Class>
        </rdfs:domain>
        <rdfs:range rdf:resource="http://www.w3.org/ns/odrl/2/Party"/>
        <rdfs:isDefinedBy rdf:resource="http://www.w3.org/ns/odrl/2/"/>
        <rdfs:label xml:lang="en">Assignee</rdfs:label>
        <rdfs:label>asignee</rdfs:label>
        <skos:definition xml:lang="en">The Party is the recipient of the Rule.</skos:definition>
    </owl:ObjectProperty>
    


    <!-- http://www.w3.org/ns/odrl/2/assigneeOf -->

    <owl:ObjectProperty rdf:about="http://www.w3.org/ns/odrl/2/assigneeOf">
        <rdfs:domain rdf:resource="http://www.w3.org/ns/odrl/2/Party"/>
        <rdfs:range rdf:resource="http://www.w3.org/ns/odrl/2/Policy"/>
        <rdfs:isDefinedBy rdf:resource="http://www.w3.org/ns/odrl/2/"/>
        <rdfs:label xml:lang="en">Assignee Of</rdfs:label>
        <skos:definition xml:lang="en">Identifies an ODRL Policy for which the identified Party undertakes the assignee functional role.</skos:definition>
        <skos:note xml:lang="en">When assigneeOf has been asserted between a metadata expression and an ODRL Policy, the Party being identified MUST be inferred to undertake the assignee functional role of all the Rules of that Policy.</skos:note>
    </owl:ObjectProperty>
    


    <!-- http://www.w3.org/ns/odrl/2/assigner -->

    <owl:ObjectProperty rdf:about="http://www.w3.org/ns/odrl/2/assigner">
        <rdfs:subPropertyOf rdf:resource="http://www.w3.org/ns/odrl/2/function"/>
        <rdfs:domain>
            <owl:Class>
                <owl:unionOf rdf:parseType="Collection">
                    <rdf:Description rdf:about="http://www.w3.org/ns/odrl/2/Policy"/>
                    <rdf:Description rdf:about="http://www.w3.org/ns/odrl/2/Rule"/>
                </owl:unionOf>
            </owl:Class>
        </rdfs:domain>
        <rdfs:range rdf:resource="http://www.w3.org/ns/odrl/2/Party"/>
        <rdfs:isDefinedBy rdf:resource="http://www.w3.org/ns/odrl/2/"/>
        <rdfs:label xml:lang="en">Assigner</rdfs:label>
        <rdfs:label>asigner</rdfs:label>
        <skos:definition xml:lang="en">The Party is the issuer of the Rule.</skos:definition>
    </owl:ObjectProperty>
    


    <!-- http://www.w3.org/ns/odrl/2/assignerOf -->

    <owl:ObjectProperty rdf:about="http://www.w3.org/ns/odrl/2/assignerOf">
        <rdfs:domain rdf:resource="http://www.w3.org/ns/odrl/2/Party"/>
        <rdfs:range rdf:resource="http://www.w3.org/ns/odrl/2/Policy"/>
        <rdfs:isDefinedBy rdf:resource="http://www.w3.org/ns/odrl/2/"/>
        <rdfs:label xml:lang="en">Assigner Of</rdfs:label>
        <skos:definition xml:lang="en">Identifies an ODRL Policy for which the identified Party undertakes the assigner functional role.</skos:definition>
        <skos:note xml:lang="en">When assignerOf has been asserted between a metadata expression and an ODRL Policy, the Party being identified MUST be inferred to undertake the assigner functional role of all the Rules of that Policy.</skos:note>
    </owl:ObjectProperty>
    


    <!-- http://www.w3.org/ns/odrl/2/constraint -->

    <owl:ObjectProperty rdf:about="http://www.w3.org/ns/odrl/2/constraint">
        <rdfs:domain>
            <owl:Class>
                <owl:unionOf rdf:parseType="Collection">
                    <rdf:Description rdf:about="http://www.w3.org/ns/odrl/2/Policy"/>
                    <rdf:Description rdf:about="http://www.w3.org/ns/odrl/2/Rule"/>
                </owl:unionOf>
            </owl:Class>
        </rdfs:domain>
        <rdfs:range>
            <owl:Class>
                <owl:unionOf rdf:parseType="Collection">
                    <rdf:Description rdf:about="http://www.w3.org/ns/odrl/2/Constraint"/>
                    <rdf:Description rdf:about="http://www.w3.org/ns/odrl/2/LogicalConstraint"/>
                </owl:unionOf>
            </owl:Class>
        </rdfs:range>
        <rdfs:isDefinedBy rdf:resource="http://www.w3.org/ns/odrl/2/"/>
        <rdfs:label xml:lang="en">Has Constraint</rdfs:label>
        <rdfs:label>constraint</rdfs:label>
        <skos:definition xml:lang="en">Constraint applied to a Rule</skos:definition>
        <skos:note xml:lang="en">Constraints on Rules are used to determine if a rule is Active or not. Example: the Permission rule is only active during the year 2018.</skos:note>
    </owl:ObjectProperty>
    


    <!-- http://www.w3.org/ns/odrl/2/function -->

    <owl:ObjectProperty rdf:about="http://www.w3.org/ns/odrl/2/function">
        <rdfs:domain>
            <owl:Class>
                <owl:unionOf rdf:parseType="Collection">
                    <rdf:Description rdf:about="http://www.w3.org/ns/odrl/2/Policy"/>
                    <rdf:Description rdf:about="http://www.w3.org/ns/odrl/2/Rule"/>
                </owl:unionOf>
            </owl:Class>
        </rdfs:domain>
        <rdfs:range rdf:resource="http://www.w3.org/ns/odrl/2/Party"/>
        <rdfs:isDefinedBy rdf:resource="http://www.w3.org/ns/odrl/2/"/>
        <rdfs:label xml:lang="en">Function</rdfs:label>
        <skos:definition xml:lang="en">Function is an abstract property whose sub-properties define the functional roles which may be fulfilled by a party in relation to a Rule.</skos:definition>
    </owl:ObjectProperty>
    


    <!-- http://www.w3.org/ns/odrl/2/hasPolicy -->

    <owl:ObjectProperty rdf:about="http://www.w3.org/ns/odrl/2/hasPolicy">
        <rdfs:domain rdf:resource="http://www.w3.org/ns/odrl/2/Asset"/>
        <rdfs:range rdf:resource="http://www.w3.org/ns/odrl/2/Policy"/>
        <rdfs:isDefinedBy rdf:resource="http://www.w3.org/ns/odrl/2/"/>
        <rdfs:label xml:lang="en">Target Policy</rdfs:label>
        <skos:definition xml:lang="en">Identifies an ODRL Policy for which the identified Asset is the target Asset to all the Rules.</skos:definition>
        <skos:note xml:lang="en">The Asset being identified MUST be inferred to be the target Asset of all of the Rules of the Policy.</skos:note>
    </owl:ObjectProperty>
    


    <!-- http://www.w3.org/ns/odrl/2/leftOperand -->

    <owl:ObjectProperty rdf:about="http://www.w3.org/ns/odrl/2/leftOperand">
        <rdfs:domain rdf:resource="http://www.w3.org/ns/odrl/2/Constraint"/>
        <rdfs:isDefinedBy rdf:resource="http://www.w3.org/ns/odrl/2/"/>
        <rdfs:label xml:lang="en">Has Left Operand</rdfs:label>
        <rdfs:label>left operand</rdfs:label>
        <skos:definition xml:lang="en">The left operand in a constraint expression.</skos:definition>
    </owl:ObjectProperty>
    


    <!-- http://www.w3.org/ns/odrl/2/operator -->

    <owl:ObjectProperty rdf:about="http://www.w3.org/ns/odrl/2/operator">
        <rdfs:domain rdf:resource="http://www.w3.org/ns/odrl/2/Constraint"/>
        <rdfs:range rdf:resource="http://www.w3.org/ns/odrl/2/Operator"/>
        <rdfs:isDefinedBy rdf:resource="http://www.w3.org/ns/odrl/2/"/>
        <rdfs:label xml:lang="en">Has Operator</rdfs:label>
        <rdfs:label>operator</rdfs:label>
        <skos:definition xml:lang="en">The operator function applied to operands of a Constraint</skos:definition>
    </owl:ObjectProperty>
    


    <!-- http://www.w3.org/ns/odrl/2/relation -->

    <owl:ObjectProperty rdf:about="http://www.w3.org/ns/odrl/2/relation">
        <rdfs:domain>
            <owl:Class>
                <owl:unionOf rdf:parseType="Collection">
                    <rdf:Description rdf:about="http://www.w3.org/ns/odrl/2/Policy"/>
                    <rdf:Description rdf:about="http://www.w3.org/ns/odrl/2/Rule"/>
                </owl:unionOf>
            </owl:Class>
        </rdfs:domain>
        <rdfs:range rdf:resource="http://www.w3.org/ns/odrl/2/Asset"/>
        <rdfs:isDefinedBy rdf:resource="http://www.w3.org/ns/odrl/2/"/>
        <rdfs:label xml:lang="en">Relation</rdfs:label>
        <skos:definition xml:lang="en">Relation is an abstract property which creates an explicit link between an Action and an Asset.</skos:definition>
        <skos:note xml:lang="en">Sub-properties of relation are used to define the nature of that link.</skos:note>
    </owl:ObjectProperty>
    


    <!-- http://www.w3.org/ns/odrl/2/rightOperand -->

    <owl:ObjectProperty rdf:about="http://www.w3.org/ns/odrl/2/rightOperand">
        <rdfs:domain rdf:resource="http://www.w3.org/ns/odrl/2/Constraint"/>
        <rdfs:isDefinedBy rdf:resource="http://www.w3.org/ns/odrl/2/"/>
        <rdfs:label xml:lang="en">Has Right Operand</rdfs:label>
        <rdfs:label>right operand</rdfs:label>
        <skos:definition xml:lang="en">The value of the right operand in a constraint expression.</skos:definition>
        <skos:note xml:lang="en">When used with set-based operators, a list of values may be used.</skos:note>
    </owl:ObjectProperty>
    


    <!-- http://www.w3.org/ns/odrl/2/target -->

    <owl:ObjectProperty rdf:about="http://www.w3.org/ns/odrl/2/target">
        <rdfs:subPropertyOf rdf:resource="http://www.w3.org/ns/odrl/2/relation"/>
        <rdfs:domain>
            <owl:Class>
                <owl:unionOf rdf:parseType="Collection">
                    <rdf:Description rdf:about="http://www.w3.org/ns/odrl/2/Policy"/>
                    <rdf:Description rdf:about="http://www.w3.org/ns/odrl/2/Rule"/>
                </owl:unionOf>
            </owl:Class>
        </rdfs:domain>
        <rdfs:range rdf:resource="http://www.w3.org/ns/odrl/2/Asset"/>
        <rdfs:isDefinedBy rdf:resource="http://www.w3.org/ns/odrl/2/"/>
        <rdfs:label xml:lang="en">Target</rdfs:label>
        <rdfs:label>target</rdfs:label>
        <skos:definition xml:lang="en">The target property indicates the Asset that is the primary subject to which the Rule action directly applies.</skos:definition>
    </owl:ObjectProperty>
    


    <!-- https://w3id.org/def/vaeontology#abidesByValue -->

    <owl:ObjectProperty rdf:about="https://w3id.org/def/vaeontology#abidesByValue">
        <owl:inverseOf rdf:resource="https://w3id.org/def/vaeontology#constrainsOutcome"/>
        <rdfs:domain rdf:resource="https://w3id.org/def/vaeontology#Outcome"/>
        <rdfs:range rdf:resource="https://w3id.org/def/vaeontology#ValueConcept"/>
        <rdfs:comment>Said of an outcome abiding by a ValueConcept</rdfs:comment>
        <rdfs:label>abides by value</rdfs:label>
    </owl:ObjectProperty>
    


    <!-- https://w3id.org/def/vaeontology#comparisonHasInferior -->

    <owl:ObjectProperty rdf:about="https://w3id.org/def/vaeontology#comparisonHasInferior">
        <rdfs:subPropertyOf rdf:resource="https://w3id.org/def/vaeontology#interpretationOn"/>
        <owl:inverseOf rdf:resource="https://w3id.org/def/vaeontology#inferiorInComparison"/>
        <rdfs:domain rdf:resource="https://w3id.org/def/vaeontology#ValueComparisonStatement"/>
        <rdfs:range rdf:resource="https://w3id.org/def/vaeontology#ValueConcept"/>
        <rdfs:comment>Indicates in the ValueComparisonStatement the ValueConcept that is inferior to some other superior one (that is to be supplied in the same ValueComparisonStatement).</rdfs:comment>
        <rdfs:label>comparison has inferior</rdfs:label>
    </owl:ObjectProperty>
    


    <!-- https://w3id.org/def/vaeontology#comparisonHasSuperior -->

    <owl:ObjectProperty rdf:about="https://w3id.org/def/vaeontology#comparisonHasSuperior">
        <rdfs:subPropertyOf rdf:resource="https://w3id.org/def/vaeontology#interpretationOn"/>
        <owl:inverseOf rdf:resource="https://w3id.org/def/vaeontology#superiorInComparison"/>
        <rdfs:domain rdf:resource="https://w3id.org/def/vaeontology#ValueComparisonStatement"/>
        <rdfs:range rdf:resource="https://w3id.org/def/vaeontology#ValueConcept"/>
        <rdfs:comment>Indicates in the ValueComparisonStatement the ValueConcept that is superior to some other inferior one (that is to be supplied in the same ValueComparisonStatement).</rdfs:comment>
        <rdfs:label>comparison has superior</rdfs:label>
    </owl:ObjectProperty>
    


    <!-- https://w3id.org/def/vaeontology#composedBySequence -->

    <owl:ObjectProperty rdf:about="https://w3id.org/def/vaeontology#composedBySequence">
        <rdfs:subPropertyOf rdf:resource="http://www.ontologydesignpatterns.org/ont/dul/DUL.owl#hasComponent"/>
        <owl:inverseOf rdf:resource="https://w3id.org/def/vaeontology#composesComplexOutcome"/>
        <rdfs:domain rdf:resource="https://w3id.org/def/vaeontology#Outcome"/>
        <rdfs:range rdf:resource="https://w3id.org/def/vaeontology#Sequence"/>
        <rdfs:comment>Indicates that the Outcome is composed by a Sequence of other outcomes.</rdfs:comment>
        <rdfs:label>composed by sequence</rdfs:label>
    </owl:ObjectProperty>
    


    <!-- https://w3id.org/def/vaeontology#composesComplexOutcome -->

    <owl:ObjectProperty rdf:about="https://w3id.org/def/vaeontology#composesComplexOutcome">
        <rdfs:subPropertyOf rdf:resource="http://www.ontologydesignpatterns.org/ont/dul/DUL.owl#isComponentOf"/>
        <rdfs:domain rdf:resource="https://w3id.org/def/vaeontology#Sequence"/>
        <rdfs:range rdf:resource="https://w3id.org/def/vaeontology#Outcome"/>
        <rdfs:comment>Indicates that the Sequence is a sequence of outcomes that composes a more complex Outcome.</rdfs:comment>
        <rdfs:label>composes complex outcome</rdfs:label>
    </owl:ObjectProperty>
    


    <!-- https://w3id.org/def/vaeontology#conditionsActionIn -->

    <owl:ObjectProperty rdf:about="https://w3id.org/def/vaeontology#conditionsActionIn">
        <rdfs:subPropertyOf rdf:resource="http://www.ontologydesignpatterns.org/ont/dul/DUL.owl#isPreconditionOf"/>
        <owl:inverseOf rdf:resource="https://w3id.org/def/vaeontology#onState"/>
        <rdfs:domain rdf:resource="https://w3id.org/def/vaeontology#State"/>
        <rdfs:range rdf:resource="https://w3id.org/def/vaeontology#ActionOnState"/>
        <rdfs:comment>Indicates that the vae:State is in some relation (vae:ActionOnState) from a vae:Strategy, an such, some vae:Action should be made by the Agent holding the vae:Strategy on the vae:State.</rdfs:comment>
        <rdfs:label>conditions action in</rdfs:label>
    </owl:ObjectProperty>
    


    <!-- https://w3id.org/def/vaeontology#constrainsOutcome -->

    <owl:ObjectProperty rdf:about="https://w3id.org/def/vaeontology#constrainsOutcome">
        <rdfs:domain rdf:resource="https://w3id.org/def/vaeontology#ValueConcept"/>
        <rdfs:range rdf:resource="https://w3id.org/def/vaeontology#Outcome"/>
        <rdfs:comment>Said of an ValueConcept constraining an Outcome.</rdfs:comment>
        <rdfs:label>constrains outcome</rdfs:label>
    </owl:ObjectProperty>
    


    <!-- https://w3id.org/def/vaeontology#describesVaeStatementEntity -->

    <owl:ObjectProperty rdf:about="https://w3id.org/def/vaeontology#describesVaeStatementEntity">
        <rdfs:subPropertyOf rdf:resource="http://www.ontologydesignpatterns.org/ont/dul/DUL.owl#describes"/>
        <owl:inverseOf rdf:resource="https://w3id.org/def/vaeontology#isPresentInStatement"/>
        <rdfs:domain rdf:resource="https://w3id.org/def/vaeontology#AgentStatement"/>
        <rdfs:range rdf:resource="https://w3id.org/def/vaeontology#VaeStatementEntity"/>
        <rdfs:comment>Indicates that the AgentStatement covers some Vae abstraction (Agent or Norm or Outcome or VaeProperty or ValeuConcept) in an undetermined way.</rdfs:comment>
        <rdfs:label>covers item</rdfs:label>
    </owl:ObjectProperty>
    


    <!-- https://w3id.org/def/vaeontology#directlyGeneralizesNode -->

    <owl:ObjectProperty rdf:about="https://w3id.org/def/vaeontology#directlyGeneralizesNode">
        <rdfs:subPropertyOf rdf:resource="https://w3id.org/def/vaeontology#generalizesNode"/>
        <owl:inverseOf rdf:resource="https://w3id.org/def/vaeontology#directlyParticularizesNode"/>
        <rdfs:domain rdf:resource="https://w3id.org/def/vaeontology#ConceptNode"/>
        <rdfs:range>
            <owl:Class>
                <owl:unionOf rdf:parseType="Collection">
                    <rdf:Description rdf:about="https://w3id.org/def/vaeontology#ConceptNode"/>
                    <rdf:Description rdf:about="https://w3id.org/def/vaeontology#PropertyNode"/>
                </owl:unionOf>
            </owl:Class>
        </rdfs:range>
        <rdfs:comment>Indicates that the ConceptNode directly generalizes the ConceptNode or PropertyNode specified (they are linked directly in the ValueTaxonomy).</rdfs:comment>
        <rdfs:label>directly generalizes</rdfs:label>
    </owl:ObjectProperty>
    


    <!-- https://w3id.org/def/vaeontology#directlyParticularizesNode -->

    <owl:ObjectProperty rdf:about="https://w3id.org/def/vaeontology#directlyParticularizesNode">
        <rdfs:subPropertyOf rdf:resource="https://w3id.org/def/vaeontology#particularizesNode"/>
        <rdfs:domain>
            <owl:Class>
                <owl:unionOf rdf:parseType="Collection">
                    <rdf:Description rdf:about="https://w3id.org/def/vaeontology#ConceptNode"/>
                    <rdf:Description rdf:about="https://w3id.org/def/vaeontology#PropertyNode"/>
                </owl:unionOf>
            </owl:Class>
        </rdfs:domain>
        <rdfs:range rdf:resource="https://w3id.org/def/vaeontology#ConceptNode"/>
        <rdfs:comment>Indicates that the ConceptNode or PropertyNode directly particularizes the ConceptNode specified (they are linked directly in the ValueTaxonomy).</rdfs:comment>
        <rdfs:label>directly particularizes</rdfs:label>
    </owl:ObjectProperty>
    


    <!-- https://w3id.org/def/vaeontology#expressesProperty -->

    <owl:ObjectProperty rdf:about="https://w3id.org/def/vaeontology#expressesProperty">
        <rdfs:subPropertyOf rdf:resource="https://w3id.org/def/vaeontology#describesVaeStatementEntity"/>
        <owl:inverseOf rdf:resource="https://w3id.org/def/vaeontology#propertyExpressedAt"/>
        <rdfs:domain rdf:resource="https://w3id.org/def/vaeontology#AgentStatement"/>
        <rdfs:range rdf:resource="https://w3id.org/def/vaeontology#VaeProperty"/>
        <rdfs:comment>Indicates that the VaePropertyStatement expresses some VaeProperty</rdfs:comment>
        <rdfs:label>presents property</rdfs:label>
    </owl:ObjectProperty>
    


    <!-- https://w3id.org/def/vaeontology#followsStrategy -->

    <owl:ObjectProperty rdf:about="https://w3id.org/def/vaeontology#followsStrategy">
        <rdfs:subPropertyOf rdf:resource="http://www.ontologydesignpatterns.org/ont/dul/DUL.owl#isParticipantIn"/>
        <owl:inverseOf rdf:resource="https://w3id.org/def/vaeontology#isFollowedByAgent"/>
        <rdfs:domain rdf:resource="https://w3id.org/def/vaeontology#ActingAgent"/>
        <rdfs:range rdf:resource="https://w3id.org/def/vaeontology#Strategy"/>
        <rdfs:comment>Indicates that the Strategy is followed by some ActingAgent.</rdfs:comment>
        <rdfs:label>follows strategy</rdfs:label>
    </owl:ObjectProperty>
    


    <!-- https://w3id.org/def/vaeontology#generalizesNode -->

    <owl:ObjectProperty rdf:about="https://w3id.org/def/vaeontology#generalizesNode">
        <rdfs:subPropertyOf rdf:resource="https://w3id.org/framester/schema/subsumes"/>
        <owl:inverseOf rdf:resource="https://w3id.org/def/vaeontology#particularizesNode"/>
        <rdf:type rdf:resource="http://www.w3.org/2002/07/owl#TransitiveProperty"/>
        <rdfs:domain rdf:resource="https://w3id.org/def/vaeontology#ConceptNode"/>
        <rdfs:range>
            <owl:Class>
                <owl:unionOf rdf:parseType="Collection">
                    <rdf:Description rdf:about="https://w3id.org/def/vaeontology#ConceptNode"/>
                    <rdf:Description rdf:about="https://w3id.org/def/vaeontology#PropertyNode"/>
                </owl:unionOf>
            </owl:Class>
        </rdfs:range>
        <rdfs:comment>Indicates that the ConceptNode generalizes the ConceptNode or PropertyNode specified.</rdfs:comment>
        <rdfs:label>generalizes</rdfs:label>
    </owl:ObjectProperty>
    


    <!-- https://w3id.org/def/vaeontology#hasActionOnState -->

    <owl:ObjectProperty rdf:about="https://w3id.org/def/vaeontology#hasActionOnState">
        <rdfs:subPropertyOf rdf:resource="http://www.ontologydesignpatterns.org/ont/dul/DUL.owl#hasComponent"/>
        <owl:inverseOf rdf:resource="https://w3id.org/def/vaeontology#isActionOnStateOfStrategy"/>
        <rdfs:domain rdf:resource="https://w3id.org/def/vaeontology#Strategy"/>
        <rdfs:range rdf:resource="https://w3id.org/def/vaeontology#ActionOnState"/>
        <rdfs:comment>Indicates the Strategy has the ActionOnState relation specified.</rdfs:comment>
        <rdfs:label>has action on state</rdfs:label>
    </owl:ObjectProperty>
    


    <!-- https://w3id.org/def/vaeontology#hasAgent -->

    <owl:ObjectProperty rdf:about="https://w3id.org/def/vaeontology#hasAgent">
        <rdfs:subPropertyOf rdf:resource="http://www.ontologydesignpatterns.org/ont/dul/DUL.owl#hasMember"/>
        <owl:inverseOf rdf:resource="https://w3id.org/def/vaeontology#isAgentOfSystem"/>
        <rdfs:domain rdf:resource="https://w3id.org/def/vaeontology#System"/>
        <rdfs:range rdf:resource="https://w3id.org/def/vaeontology#Agent"/>
        <rdfs:comment>Indicates that the System has the Agent specified.</rdfs:comment>
        <rdfs:label>has agent</rdfs:label>
    </owl:ObjectProperty>
    


    <!-- https://w3id.org/def/vaeontology#hasClaim -->

    <owl:ObjectProperty rdf:about="https://w3id.org/def/vaeontology#hasClaim">
        <rdfs:subPropertyOf rdf:resource="http://www.ontologydesignpatterns.org/ont/dul/DUL.owl#hasConstituent"/>
        <owl:inverseOf rdf:resource="https://w3id.org/def/vaeontology#isClaimOf"/>
        <rdfs:domain rdf:resource="https://w3id.org/def/vaeontology#ArgumentStatement"/>
        <rdfs:range rdf:resource="https://w3id.org/def/vaeontology#VaeStatement"/>
        <rdfs:comment>Indicates that the Argument has the VaeStaement specified as a claim.</rdfs:comment>
        <rdfs:label>has claim</rdfs:label>
    </owl:ObjectProperty>
    


    <!-- https://w3id.org/def/vaeontology#hasConceptNode -->

    <owl:ObjectProperty rdf:about="https://w3id.org/def/vaeontology#hasConceptNode">
        <rdfs:subPropertyOf rdf:resource="https://w3id.org/def/vaeontology#hasTaxonomyNode"/>
        <owl:inverseOf rdf:resource="https://w3id.org/def/vaeontology#isConceptNodeOf"/>
        <rdfs:domain rdf:resource="https://w3id.org/def/vaeontology#ValueTaxonomyStatement"/>
        <rdfs:range rdf:resource="https://w3id.org/def/vaeontology#ConceptNode"/>
        <rdfs:comment>Indicates that the ValueTaxonomy has the ConceptNode specified.</rdfs:comment>
        <rdfs:label>has concept node</rdfs:label>
    </owl:ObjectProperty>
    


    <!-- https://w3id.org/def/vaeontology#hasImportance -->

    <owl:ObjectProperty rdf:about="https://w3id.org/def/vaeontology#hasImportance">
        <rdfs:subPropertyOf rdf:resource="https://w3id.org/def/vaeontology#expressesProperty"/>
        <owl:inverseOf rdf:resource="https://w3id.org/def/vaeontology#isImportanceOf"/>
        <rdfs:domain>
            <owl:Class>
                <owl:unionOf rdf:parseType="Collection">
                    <rdf:Description rdf:about="https://w3id.org/def/vaeontology#ConceptNode"/>
                    <rdf:Description rdf:about="https://w3id.org/def/vaeontology#PropertyNode"/>
                </owl:unionOf>
            </owl:Class>
        </rdfs:domain>
        <rdfs:range rdf:resource="https://w3id.org/def/vaeontology#NodeImportance"/>
        <rdfs:comment>Indicates that the ConceptNode has a NodeImportance.</rdfs:comment>
        <rdfs:label>has importance</rdfs:label>
    </owl:ObjectProperty>
    


    <!-- https://w3id.org/def/vaeontology#hasInput -->

    <owl:ObjectProperty rdf:about="https://w3id.org/def/vaeontology#hasInput">
        <rdfs:subPropertyOf rdf:resource="http://www.ontologydesignpatterns.org/ont/dul/DUL.owl#hasConstituent"/>
        <owl:inverseOf rdf:resource="https://w3id.org/def/vaeontology#isInputOf"/>
        <rdfs:domain rdf:resource="https://w3id.org/def/vaeontology#MultiInputOutcome"/>
        <rdfs:range rdf:resource="http://www.ontologydesignpatterns.org/ont/dul/DUL.owl#Event"/>
        <rdfs:comment>Indicates that the MultiInputOutcome has some Event as its input, that conditions its outcome.</rdfs:comment>
        <rdfs:label>has input</rdfs:label>
    </owl:ObjectProperty>
    


    <!-- https://w3id.org/def/vaeontology#hasInputOutcome -->

    <owl:ObjectProperty rdf:about="https://w3id.org/def/vaeontology#hasInputOutcome">
        <rdfs:subPropertyOf rdf:resource="http://www.ontologydesignpatterns.org/ont/dul/DUL.owl#hasConstituent"/>
        <owl:inverseOf rdf:resource="https://w3id.org/def/vaeontology#isInputOutcomeOf"/>
        <rdfs:domain rdf:resource="https://w3id.org/def/vaeontology#Sequence"/>
        <rdfs:range rdf:resource="https://w3id.org/def/vaeontology#MultiInputOutcome"/>
        <rdfs:comment>Indicates that a vae:Sequence contains some vae:InputOutcome relation.</rdfs:comment>
        <rdfs:label>has input outcome</rdfs:label>
    </owl:ObjectProperty>
    


    <!-- https://w3id.org/def/vaeontology#hasInterpretation -->

    <owl:ObjectProperty rdf:about="https://w3id.org/def/vaeontology#hasInterpretation">
        <rdfs:subPropertyOf rdf:resource="https://w3id.org/def/vaeontology#isPresentInStatement"/>
        <owl:inverseOf rdf:resource="https://w3id.org/def/vaeontology#interpretationOn"/>
        <rdfs:domain rdf:resource="https://w3id.org/def/vaeontology#VaeConditioningEntity"/>
        <rdfs:range rdf:resource="https://w3id.org/def/vaeontology#AgentStatement"/>
    </owl:ObjectProperty>
    


    <!-- https://w3id.org/def/vaeontology#hasOutcome -->

    <owl:ObjectProperty rdf:about="https://w3id.org/def/vaeontology#hasOutcome">
        <rdfs:subPropertyOf rdf:resource="http://www.ontologydesignpatterns.org/ont/dul/DUL.owl#hasConstituent"/>
        <owl:inverseOf rdf:resource="https://w3id.org/def/vaeontology#isOutcomeOf"/>
        <rdfs:domain rdf:resource="https://w3id.org/def/vaeontology#MultiInputOutcome"/>
        <rdfs:range rdf:resource="https://w3id.org/def/vaeontology#Outcome"/>
        <rdfs:comment>Indicates that the MultiInputOutcome relation has some Outcome, that might be conditioned on some input.</rdfs:comment>
        <rdfs:label>has outcome</rdfs:label>
    </owl:ObjectProperty>
    


    <!-- https://w3id.org/def/vaeontology#hasPremise -->

    <owl:ObjectProperty rdf:about="https://w3id.org/def/vaeontology#hasPremise">
        <rdfs:subPropertyOf rdf:resource="http://www.ontologydesignpatterns.org/ont/dul/DUL.owl#hasConstituent"/>
        <owl:inverseOf rdf:resource="https://w3id.org/def/vaeontology#isPremiseOf"/>
        <rdfs:domain rdf:resource="https://w3id.org/def/vaeontology#ArgumentStatement"/>
        <rdfs:range rdf:resource="https://w3id.org/def/vaeontology#VaeStatement"/>
        <rdfs:comment>Indicates that the Argument has the VaeStaement specified as a premise.</rdfs:comment>
        <rdfs:label>has premise</rdfs:label>
    </owl:ObjectProperty>
    


    <!-- https://w3id.org/def/vaeontology#hasPropertyNode -->

    <owl:ObjectProperty rdf:about="https://w3id.org/def/vaeontology#hasPropertyNode">
        <rdfs:subPropertyOf rdf:resource="http://www.ontologydesignpatterns.org/ont/dul/DUL.owl#hasComponent"/>
        <rdfs:subPropertyOf rdf:resource="https://w3id.org/def/vaeontology#hasTaxonomyNode"/>
        <owl:inverseOf rdf:resource="https://w3id.org/def/vaeontology#isPropertyNodeOf"/>
        <rdfs:domain rdf:resource="https://w3id.org/def/vaeontology#ValueTaxonomyStatement"/>
        <rdfs:range rdf:resource="https://w3id.org/def/vaeontology#PropertyNode"/>
        <rdfs:comment>Indicates that the ValueTaxonomy has the PropertyNode specified.</rdfs:comment>
        <rdfs:label>has PropertyNode</rdfs:label>
    </owl:ObjectProperty>
    


    <!-- https://w3id.org/def/vaeontology#hasPropertyOfInferior -->

    <owl:ObjectProperty rdf:about="https://w3id.org/def/vaeontology#hasPropertyOfInferior">
        <rdfs:subPropertyOf rdf:resource="https://w3id.org/def/vaeontology#expressesProperty"/>
        <owl:inverseOf rdf:resource="https://w3id.org/def/vaeontology#isPropertyOfInferiorOf"/>
        <rdfs:domain rdf:resource="https://w3id.org/def/vaeontology#ValueComparisonStatement"/>
        <rdfs:range rdf:resource="https://w3id.org/def/vaeontology#ValueProperty"/>
        <rdfs:comment>Indicates that the ValueComparisonStatement has a ValueProperty characterizing why the inferior of the comparison is, in fact, inferior of the relation.</rdfs:comment>
        <rdfs:label>has property of inferior</rdfs:label>
    </owl:ObjectProperty>
    


    <!-- https://w3id.org/def/vaeontology#hasPropertyOfSuperior -->

    <owl:ObjectProperty rdf:about="https://w3id.org/def/vaeontology#hasPropertyOfSuperior">
        <rdfs:subPropertyOf rdf:resource="https://w3id.org/def/vaeontology#expressesProperty"/>
        <owl:inverseOf rdf:resource="https://w3id.org/def/vaeontology#isPropertyOfSuperiorOf"/>
        <rdfs:domain rdf:resource="https://w3id.org/def/vaeontology#ValueComparisonStatement"/>
        <rdfs:range rdf:resource="https://w3id.org/def/vaeontology#ValueProperty"/>
        <rdfs:comment>Indicates that the ValueComparisonStatement has a ValueProperty characterizing why the superior of the comparison is, in fact, superior of the relation.</rdfs:comment>
        <rdfs:label>has property of superior</rdfs:label>
    </owl:ObjectProperty>
    


    <!-- https://w3id.org/def/vaeontology#hasPropertyTaxonomy -->

    <owl:ObjectProperty rdf:about="https://w3id.org/def/vaeontology#hasPropertyTaxonomy">
        <rdfs:subPropertyOf rdf:resource="https://w3id.org/def/vaeontology#expressesProperty"/>
        <owl:inverseOf rdf:resource="https://w3id.org/def/vaeontology#isTaxonomyPropertyOf"/>
        <rdfs:domain rdf:resource="https://w3id.org/def/vaeontology#PropertyNode"/>
        <rdfs:range rdf:resource="https://w3id.org/def/vaeontology#TaxonomyProperty"/>
        <rdfs:comment>Indicates that the PropertyNode has a PropertyTaxonomy (a ValueProperty informing of the degree of satisfaction of the taxonomy property).</rdfs:comment>
        <rdfs:label>has Property Taxonomy</rdfs:label>
    </owl:ObjectProperty>
    


    <!-- https://w3id.org/def/vaeontology#hasRelationWithProperty -->

    <owl:ObjectProperty rdf:about="https://w3id.org/def/vaeontology#hasRelationWithProperty">
        <rdfs:subPropertyOf rdf:resource="https://w3id.org/framester/schema/hasPerspective"/>
        <owl:inverseOf rdf:resource="https://w3id.org/def/vaeontology#relationWith"/>
        <rdfs:domain rdf:resource="https://w3id.org/def/vaeontology#VaeConditioningEntity"/>
        <rdfs:range rdf:resource="https://w3id.org/def/vaeontology#VaeProperty"/>
    </owl:ObjectProperty>
    


    <!-- https://w3id.org/def/vaeontology#hasRootNode -->

    <owl:ObjectProperty rdf:about="https://w3id.org/def/vaeontology#hasRootNode">
        <rdfs:subPropertyOf rdf:resource="https://w3id.org/def/vaeontology#hasConceptNode"/>
        <owl:inverseOf rdf:resource="https://w3id.org/def/vaeontology#isRootNodeOf"/>
        <rdfs:domain rdf:resource="https://w3id.org/def/vaeontology#ValueTaxonomyStatement"/>
        <rdfs:range>
            <owl:Class>
                <owl:intersectionOf rdf:parseType="Collection">
                    <rdf:Description rdf:about="https://w3id.org/def/vaeontology#ConceptNode"/>
                    <owl:Class>
                        <owl:complementOf>
                            <owl:Restriction>
                                <owl:onProperty rdf:resource="https://w3id.org/def/vaeontology#particularizesNode"/>
                                <owl:someValuesFrom rdf:resource="https://w3id.org/def/vaeontology#ConceptNode"/>
                            </owl:Restriction>
                        </owl:complementOf>
                    </owl:Class>
                </owl:intersectionOf>
            </owl:Class>
        </rdfs:range>
        <rdfs:comment>Indicates that the ValueTaxonomy has the RootNode specified (a ConceptNode which is not generalized by any other).</rdfs:comment>
        <rdfs:label>has root node</rdfs:label>
    </owl:ObjectProperty>
    


    <!-- https://w3id.org/def/vaeontology#hasState -->

    <owl:ObjectProperty rdf:about="https://w3id.org/def/vaeontology#hasState">
        <rdfs:subPropertyOf rdf:resource="http://www.ontologydesignpatterns.org/ont/dul/DUL.owl#isAgentInvolvedIn"/>
        <owl:inverseOf rdf:resource="https://w3id.org/def/vaeontology#isStateOfAgent"/>
        <rdfs:domain rdf:resource="https://w3id.org/def/vaeontology#Agent"/>
        <rdfs:range rdf:resource="https://w3id.org/def/vaeontology#State"/>
        <rdfs:comment>Indicates that the Agent is represented by some State.</rdfs:comment>
        <rdfs:label>has state</rdfs:label>
    </owl:ObjectProperty>
    


    <!-- https://w3id.org/def/vaeontology#hasTaxonomyAlignment -->

    <owl:ObjectProperty rdf:about="https://w3id.org/def/vaeontology#hasTaxonomyAlignment">
        <rdfs:subPropertyOf rdf:resource="https://w3id.org/def/vaeontology#expressesProperty"/>
        <owl:inverseOf rdf:resource="https://w3id.org/def/vaeontology#isAlignmentOfTaxonomy"/>
        <rdfs:domain rdf:resource="https://w3id.org/def/vaeontology#ValueTaxonomyStatement"/>
        <rdfs:range rdf:resource="https://w3id.org/def/vaeontology#TaxonomyAlignment"/>
        <rdfs:comment>Indicates the ValueTaxonomy has a TaxonomyAlignment (a ValueProperty indicating the degree of alignment of an outcome considering the ValueTaxonomy).</rdfs:comment>
        <rdfs:label>has taxonomy alignment</rdfs:label>
    </owl:ObjectProperty>
    


    <!-- https://w3id.org/def/vaeontology#hasTaxonomyNode -->

    <owl:ObjectProperty rdf:about="https://w3id.org/def/vaeontology#hasTaxonomyNode">
        <rdfs:subPropertyOf rdf:resource="http://www.ontologydesignpatterns.org/ont/dul/DUL.owl#hasComponent"/>
        <owl:inverseOf rdf:resource="https://w3id.org/def/vaeontology#isTaxonomyNodeOf"/>
        <rdfs:domain rdf:resource="https://w3id.org/def/vaeontology#ValueTaxonomyStatement"/>
        <rdfs:range>
            <owl:Class>
                <owl:unionOf rdf:parseType="Collection">
                    <rdf:Description rdf:about="https://w3id.org/def/vaeontology#ConceptNode"/>
                    <rdf:Description rdf:about="https://w3id.org/def/vaeontology#PropertyNode"/>
                </owl:unionOf>
            </owl:Class>
        </rdfs:range>
        <rdfs:comment>Indicates that the ValueTaxonomy containts the ConceptNode or PropertyNode specified.</rdfs:comment>
        <rdfs:label>has TaxonomyNode</rdfs:label>
    </owl:ObjectProperty>
    


    <!-- https://w3id.org/def/vaeontology#hasTrace -->

    <owl:ObjectProperty rdf:about="https://w3id.org/def/vaeontology#hasTrace">
        <rdfs:subPropertyOf rdf:resource="http://www.ontologydesignpatterns.org/ont/dul/DUL.owl#isAgentInvolvedIn"/>
        <owl:inverseOf rdf:resource="https://w3id.org/def/vaeontology#isTraceOfSystem"/>
        <rdfs:domain rdf:resource="https://w3id.org/def/vaeontology#System"/>
        <rdfs:range rdf:resource="https://w3id.org/def/vaeontology#Sequence"/>
        <rdfs:comment>Indicates that the System has a Sequence representing its trace.</rdfs:comment>
        <rdfs:label>has trace</rdfs:label>
    </owl:ObjectProperty>
    


    <!-- https://w3id.org/def/vaeontology#hasUser -->

    <owl:ObjectProperty rdf:about="https://w3id.org/def/vaeontology#hasUser">
        <rdfs:subPropertyOf rdf:resource="https://w3id.org/def/vaeontology#hasAgent"/>
        <owl:inverseOf rdf:resource="https://w3id.org/def/vaeontology#isUserOfSystem"/>
        <rdfs:domain rdf:resource="https://w3id.org/def/vaeontology#System"/>
        <rdfs:range rdf:resource="https://w3id.org/def/vaeontology#User"/>
        <rdfs:comment>Indicates that the System has the User specified.</rdfs:comment>
        <rdfs:label>has user</rdfs:label>
    </owl:ObjectProperty>
    


    <!-- https://w3id.org/def/vaeontology#inferiorInComparison -->

    <owl:ObjectProperty rdf:about="https://w3id.org/def/vaeontology#inferiorInComparison">
        <rdfs:subPropertyOf rdf:resource="https://w3id.org/def/vaeontology#hasInterpretation"/>
        <rdfs:domain rdf:resource="https://w3id.org/def/vaeontology#ValueConcept"/>
        <rdfs:range rdf:resource="https://w3id.org/def/vaeontology#ValueComparisonStatement"/>
        <rdfs:comment>Indicates in the ValueComparisonStatement the ValueConcept that is inferior to some other superior one (that is to be supplied in the same ValueComparisonStatement).</rdfs:comment>
        <rdfs:label>inferior in comparison</rdfs:label>
    </owl:ObjectProperty>
    


    <!-- https://w3id.org/def/vaeontology#influencesOutcome -->

    <owl:ObjectProperty rdf:about="https://w3id.org/def/vaeontology#influencesOutcome">
        <owl:inverseOf rdf:resource="https://w3id.org/def/vaeontology#satisfiesNorm"/>
        <rdfs:domain rdf:resource="https://w3id.org/def/vaeontology#Norm"/>
        <rdfs:range rdf:resource="https://w3id.org/def/vaeontology#Outcome"/>
        <rdfs:comment>Said of an Norm influencing an Outcome.</rdfs:comment>
        <rdfs:label>influences outcome</rdfs:label>
    </owl:ObjectProperty>
    


    <!-- https://w3id.org/def/vaeontology#interpretationOn -->

    <owl:ObjectProperty rdf:about="https://w3id.org/def/vaeontology#interpretationOn">
        <rdfs:subPropertyOf rdf:resource="https://w3id.org/def/vaeontology#describesVaeStatementEntity"/>
        <rdfs:domain rdf:resource="https://w3id.org/def/vaeontology#AgentStatement"/>
        <rdfs:range rdf:resource="https://w3id.org/def/vaeontology#VaeConditioningEntity"/>
    </owl:ObjectProperty>
    


    <!-- https://w3id.org/def/vaeontology#isActionOnStateOfStrategy -->

    <owl:ObjectProperty rdf:about="https://w3id.org/def/vaeontology#isActionOnStateOfStrategy">
        <rdfs:subPropertyOf rdf:resource="http://www.ontologydesignpatterns.org/ont/dul/DUL.owl#isComponentOf"/>
        <rdfs:domain rdf:resource="https://w3id.org/def/vaeontology#ActionOnState"/>
        <rdfs:range rdf:resource="https://w3id.org/def/vaeontology#Strategy"/>
        <rdfs:comment>Indicates the ActionOnState relation is part of the Strategy specified.</rdfs:comment>
        <rdfs:label>is ActionOnState of Strategy</rdfs:label>
    </owl:ObjectProperty>
    


    <!-- https://w3id.org/def/vaeontology#isAgentOfSystem -->

    <owl:ObjectProperty rdf:about="https://w3id.org/def/vaeontology#isAgentOfSystem">
        <rdfs:subPropertyOf rdf:resource="http://www.ontologydesignpatterns.org/ont/dul/DUL.owl#isMemberOf"/>
        <rdfs:domain rdf:resource="https://w3id.org/def/vaeontology#Agent"/>
        <rdfs:range rdf:resource="https://w3id.org/def/vaeontology#System"/>
        <rdfs:comment>Indicates that the Agent belongs to the System specified.</rdfs:comment>
        <rdfs:label>is agent of system</rdfs:label>
    </owl:ObjectProperty>
    


    <!-- https://w3id.org/def/vaeontology#isAlignmentOfTaxonomy -->

    <owl:ObjectProperty rdf:about="https://w3id.org/def/vaeontology#isAlignmentOfTaxonomy">
        <rdfs:subPropertyOf rdf:resource="https://w3id.org/def/vaeontology#propertyExpressedAt"/>
        <rdfs:domain rdf:resource="https://w3id.org/def/vaeontology#TaxonomyAlignment"/>
        <rdfs:range rdf:resource="https://w3id.org/def/vaeontology#ValueTaxonomyStatement"/>
        <rdfs:comment>Indicates the ValueTaxonomy has a TaxonomyAlignment (a ValueProperty indicating the degree of alignment of an outcome considering the ValueTaxonomy).</rdfs:comment>
        <rdfs:label>is alignment of taxonomy</rdfs:label>
    </owl:ObjectProperty>
    


    <!-- https://w3id.org/def/vaeontology#isBasedOnCriterion -->

    <owl:ObjectProperty rdf:about="https://w3id.org/def/vaeontology#isBasedOnCriterion">
        <rdfs:subPropertyOf rdf:resource="http://www.ontologydesignpatterns.org/ont/dul/DUL.owl#hasConstituent"/>
        <owl:inverseOf rdf:resource="https://w3id.org/def/vaeontology#isCriterionOfArgument"/>
        <rdfs:domain rdf:resource="https://w3id.org/def/vaeontology#ArgumentStatement"/>
        <rdfs:range rdf:resource="https://w3id.org/def/vaeontology#Criterion"/>
        <rdfs:comment>Indicates that the vae:ArgumentStatement is based on some vae:Criterion as the theory of the Explanation ODP.</rdfs:comment>
        <rdfs:label>is based on criterion</rdfs:label>
    </owl:ObjectProperty>
    


    <!-- https://w3id.org/def/vaeontology#isClaimOf -->

    <owl:ObjectProperty rdf:about="https://w3id.org/def/vaeontology#isClaimOf">
        <rdfs:subPropertyOf rdf:resource="http://www.ontologydesignpatterns.org/ont/dul/DUL.owl#isConstituentOf"/>
        <rdfs:domain rdf:resource="https://w3id.org/def/vaeontology#VaeStatement"/>
        <rdfs:range rdf:resource="https://w3id.org/def/vaeontology#ArgumentStatement"/>
        <rdfs:comment>Indicates that the VaeStatement functions as a claim for the ArgumentStatement supplied.</rdfs:comment>
        <rdfs:label>is claim of</rdfs:label>
    </owl:ObjectProperty>
    


    <!-- https://w3id.org/def/vaeontology#isConceptNodeOf -->

    <owl:ObjectProperty rdf:about="https://w3id.org/def/vaeontology#isConceptNodeOf">
        <rdfs:subPropertyOf rdf:resource="https://w3id.org/def/vaeontology#isTaxonomyNodeOf"/>
        <rdfs:domain rdf:resource="https://w3id.org/def/vaeontology#ConceptNode"/>
        <rdfs:range rdf:resource="https://w3id.org/def/vaeontology#ValueTaxonomyStatement"/>
        <rdfs:comment>Indicates that the ConceptNode is part of a ValueTaxonomy.</rdfs:comment>
        <rdfs:label>is ConceptNode of</rdfs:label>
    </owl:ObjectProperty>
    


    <!-- https://w3id.org/def/vaeontology#isCriterionOfArgument -->

    <owl:ObjectProperty rdf:about="https://w3id.org/def/vaeontology#isCriterionOfArgument">
        <rdfs:subPropertyOf rdf:resource="http://www.ontologydesignpatterns.org/ont/dul/DUL.owl#isConstituentOf"/>
        <rdfs:domain rdf:resource="https://w3id.org/def/vaeontology#Criterion"/>
        <rdfs:range rdf:resource="https://w3id.org/def/vaeontology#ArgumentStatement"/>
        <rdfs:comment>Indicates that the vae:ArgumentStatement is based on some vae:Criterion as the theory of the Explanation ODP.</rdfs:comment>
        <rdfs:label>is Criterion Of Argument</rdfs:label>
    </owl:ObjectProperty>
    


    <!-- https://w3id.org/def/vaeontology#isEntityOf -->

    <owl:ObjectProperty rdf:about="https://w3id.org/def/vaeontology#isEntityOf">
        <rdfs:subPropertyOf rdf:resource="https://w3id.org/def/vaeontology#isPresentInStatement"/>
        <owl:inverseOf rdf:resource="https://w3id.org/def/vaeontology#onEntity"/>
        <rdfs:domain rdf:resource="https://w3id.org/def/vaeontology#VaeConditionedEntity"/>
        <rdfs:range rdf:resource="https://w3id.org/def/vaeontology#AgentStatement"/>
        <rdfs:comment>Indicates that an Agent or Outcome or Norm is being used in a VaeStatement as an entity subject of evaluation for some characteristic, e.g. for an vae:AwarenessStatement: &quot;The vae:Agent payerAgent is aware of the vae:Norm [norm]&quot;, the entity of the statement is the vae:Agent payerAgent.</rdfs:comment>
        <rdfs:label xml:lang="en">Is Entity Of</rdfs:label>
    </owl:ObjectProperty>
    


    <!-- https://w3id.org/def/vaeontology#isFollowedByAgent -->

    <owl:ObjectProperty rdf:about="https://w3id.org/def/vaeontology#isFollowedByAgent">
        <rdfs:subPropertyOf rdf:resource="http://www.ontologydesignpatterns.org/ont/dul/DUL.owl#hasParticipant"/>
        <rdfs:domain rdf:resource="https://w3id.org/def/vaeontology#Strategy"/>
        <rdfs:range rdf:resource="https://w3id.org/def/vaeontology#ActingAgent"/>
        <rdfs:comment>Indicates that the Strategy is followed by some ActingAgent.</rdfs:comment>
        <rdfs:label>followed by agent</rdfs:label>
    </owl:ObjectProperty>
    


    <!-- https://w3id.org/def/vaeontology#isImportanceOf -->

    <owl:ObjectProperty rdf:about="https://w3id.org/def/vaeontology#isImportanceOf">
        <rdfs:subPropertyOf rdf:resource="https://w3id.org/def/vaeontology#propertyExpressedAt"/>
        <rdfs:domain rdf:resource="https://w3id.org/def/vaeontology#NodeImportance"/>
        <rdfs:range>
            <owl:Class>
                <owl:unionOf rdf:parseType="Collection">
                    <rdf:Description rdf:about="https://w3id.org/def/vaeontology#ConceptNode"/>
                    <rdf:Description rdf:about="https://w3id.org/def/vaeontology#PropertyNode"/>
                </owl:unionOf>
            </owl:Class>
        </rdfs:range>
        <rdfs:comment>Indicates that the ConceptNode has a NodeImportance.</rdfs:comment>
        <rdfs:label>is importance of</rdfs:label>
    </owl:ObjectProperty>
    


    <!-- https://w3id.org/def/vaeontology#isInputOf -->

    <owl:ObjectProperty rdf:about="https://w3id.org/def/vaeontology#isInputOf">
        <rdfs:subPropertyOf rdf:resource="http://www.ontologydesignpatterns.org/ont/dul/DUL.owl#isConstituentOf"/>
        <rdfs:domain rdf:resource="http://www.ontologydesignpatterns.org/ont/dul/DUL.owl#Event"/>
        <rdfs:range rdf:resource="https://w3id.org/def/vaeontology#MultiInputOutcome"/>
        <rdfs:comment>Indicates that the Event is input of a MultiInputOutcome relation, so it conditions some outcome.</rdfs:comment>
        <rdfs:label>is input of sequence</rdfs:label>
    </owl:ObjectProperty>
    


    <!-- https://w3id.org/def/vaeontology#isInputOutcomeOf -->

    <owl:ObjectProperty rdf:about="https://w3id.org/def/vaeontology#isInputOutcomeOf">
        <rdfs:subPropertyOf rdf:resource="http://www.ontologydesignpatterns.org/ont/dul/DUL.owl#isConstituentOf"/>
        <rdfs:domain rdf:resource="https://w3id.org/def/vaeontology#MultiInputOutcome"/>
        <rdfs:range rdf:resource="https://w3id.org/def/vaeontology#Sequence"/>
        <rdfs:comment>Indicates the MultiInputOutcome is part of some Sequence</rdfs:comment>
        <rdfs:label>is InputOutcome of</rdfs:label>
    </owl:ObjectProperty>
    


    <!-- https://w3id.org/def/vaeontology#isOptimizationOfProperty -->

    <owl:ObjectProperty rdf:about="https://w3id.org/def/vaeontology#isOptimizationOfProperty">
        <rdfs:subPropertyOf rdf:resource="http://www.ontologydesignpatterns.org/ont/dul/DUL.owl#describes"/>
        <owl:inverseOf rdf:resource="https://w3id.org/def/vaeontology#propertyOptimizedAt"/>
        <rdfs:domain rdf:resource="https://w3id.org/def/vaeontology#OptimizedProperty"/>
        <rdfs:range rdf:resource="https://w3id.org/def/vaeontology#VaeProperty"/>
        <rdfs:comment>Indicates the VaeProperty that is being optimized in some OptimizedProperty assertion.</rdfs:comment>
        <rdfs:label>is optimization of property</rdfs:label>
    </owl:ObjectProperty>
    


    <!-- https://w3id.org/def/vaeontology#isOutcomeOf -->

    <owl:ObjectProperty rdf:about="https://w3id.org/def/vaeontology#isOutcomeOf">
        <rdfs:subPropertyOf rdf:resource="http://www.ontologydesignpatterns.org/ont/dul/DUL.owl#isConstituentOf"/>
        <rdfs:domain rdf:resource="https://w3id.org/def/vaeontology#Outcome"/>
        <rdfs:range rdf:resource="https://w3id.org/def/vaeontology#MultiInputOutcome"/>
        <rdfs:comment>Indicates that the Outcome is present at a MultiInputOutcome relation, being part of some Sequence.</rdfs:comment>
        <rdfs:label>is outcome of sequence</rdfs:label>
    </owl:ObjectProperty>
    


    <!-- https://w3id.org/def/vaeontology#isPremiseOf -->

    <owl:ObjectProperty rdf:about="https://w3id.org/def/vaeontology#isPremiseOf">
        <rdfs:subPropertyOf rdf:resource="http://www.ontologydesignpatterns.org/ont/dul/DUL.owl#isConstituentOf"/>
        <rdfs:domain rdf:resource="https://w3id.org/def/vaeontology#VaeStatement"/>
        <rdfs:range rdf:resource="https://w3id.org/def/vaeontology#ArgumentStatement"/>
        <rdfs:comment>Indicates that the VaeStatement functions as a premise for the ArgumentStatement supplied.</rdfs:comment>
        <rdfs:label>is premise of</rdfs:label>
    </owl:ObjectProperty>
    


    <!-- https://w3id.org/def/vaeontology#isPresentInStatement -->

    <owl:ObjectProperty rdf:about="https://w3id.org/def/vaeontology#isPresentInStatement">
        <rdfs:subPropertyOf rdf:resource="http://www.ontologydesignpatterns.org/ont/dul/DUL.owl#isDescribedBy"/>
        <rdfs:domain rdf:resource="https://w3id.org/def/vaeontology#VaeStatementEntity"/>
        <rdfs:range rdf:resource="https://w3id.org/def/vaeontology#AgentStatement"/>
        <rdfs:comment>Indicates some Vae abstraction (Agent or Norm or Outcome or VaeProperty or ValueConcept) is present (referenced) in an AgentStatement.</rdfs:comment>
        <rdfs:label>is present in statement</rdfs:label>
    </owl:ObjectProperty>
    


    <!-- https://w3id.org/def/vaeontology#isPropertyNodeOf -->

    <owl:ObjectProperty rdf:about="https://w3id.org/def/vaeontology#isPropertyNodeOf">
        <rdfs:subPropertyOf rdf:resource="http://www.ontologydesignpatterns.org/ont/dul/DUL.owl#isComponentOf"/>
        <rdfs:subPropertyOf rdf:resource="https://w3id.org/def/vaeontology#isTaxonomyNodeOf"/>
        <rdfs:domain rdf:resource="https://w3id.org/def/vaeontology#PropertyNode"/>
        <rdfs:range rdf:resource="https://w3id.org/def/vaeontology#ValueTaxonomyStatement"/>
        <rdfs:comment>Indicates that the PropertyNode is part of the ValueTaxonomy specified.</rdfs:comment>
        <rdfs:label>is PropertyNode of</rdfs:label>
    </owl:ObjectProperty>
    


    <!-- https://w3id.org/def/vaeontology#isPropertyOfInferiorOf -->

    <owl:ObjectProperty rdf:about="https://w3id.org/def/vaeontology#isPropertyOfInferiorOf">
        <rdfs:subPropertyOf rdf:resource="http://www.ontologydesignpatterns.org/ont/dul/DUL.owl#isConstituentOf"/>
        <rdfs:subPropertyOf rdf:resource="https://w3id.org/def/vaeontology#propertyExpressedAt"/>
        <rdfs:domain rdf:resource="https://w3id.org/def/vaeontology#ValueProperty"/>
        <rdfs:range rdf:resource="https://w3id.org/def/vaeontology#ValueComparisonStatement"/>
        <rdfs:comment>Indicates that the ValueComparisonStatement has a ValueProperty characterizing why the inferior of the comparison is, in fact, inferior of the relation.</rdfs:comment>
        <rdfs:label>is property of inferior of</rdfs:label>
    </owl:ObjectProperty>
    


    <!-- https://w3id.org/def/vaeontology#isPropertyOfSuperiorOf -->

    <owl:ObjectProperty rdf:about="https://w3id.org/def/vaeontology#isPropertyOfSuperiorOf">
        <rdfs:subPropertyOf rdf:resource="http://www.ontologydesignpatterns.org/ont/dul/DUL.owl#isConstituentOf"/>
        <rdfs:subPropertyOf rdf:resource="https://w3id.org/def/vaeontology#propertyExpressedAt"/>
        <rdfs:domain rdf:resource="https://w3id.org/def/vaeontology#ValueProperty"/>
        <rdfs:range rdf:resource="https://w3id.org/def/vaeontology#ValueComparisonStatement"/>
        <rdfs:comment>Indicates that the ValueComparisonStatement has a ValueProperty characterizing why the superior of the comparison is, in fact, superior of the relation.</rdfs:comment>
        <rdfs:label>Is property of superior of</rdfs:label>
    </owl:ObjectProperty>
    


    <!-- https://w3id.org/def/vaeontology#isProposedByAgent -->

    <owl:ObjectProperty rdf:about="https://w3id.org/def/vaeontology#isProposedByAgent">
        <rdfs:subPropertyOf rdf:resource="http://www.ontologydesignpatterns.org/ont/dul/DUL.owl#isConceptualizedBy"/>
        <owl:inverseOf rdf:resource="https://w3id.org/def/vaeontology#proposesStatement"/>
        <rdfs:domain rdf:resource="https://w3id.org/def/vaeontology#AgentStatement"/>
        <rdfs:range rdf:resource="https://w3id.org/def/vaeontology#Agent"/>
        <rdfs:comment>Indicates that the AgentStatement about the world was proposed by some Agent.</rdfs:comment>
        <rdfs:label>is expressed by agent</rdfs:label>
    </owl:ObjectProperty>
    


    <!-- https://w3id.org/def/vaeontology#isRootNodeOf -->

    <owl:ObjectProperty rdf:about="https://w3id.org/def/vaeontology#isRootNodeOf">
        <rdfs:subPropertyOf rdf:resource="https://w3id.org/def/vaeontology#isConceptNodeOf"/>
        <rdfs:domain>
            <owl:Class>
                <owl:intersectionOf rdf:parseType="Collection">
                    <rdf:Description rdf:about="https://w3id.org/def/vaeontology#ConceptNode"/>
                    <owl:Class>
                        <owl:complementOf>
                            <owl:Restriction>
                                <owl:onProperty rdf:resource="https://w3id.org/def/vaeontology#particularizesNode"/>
                                <owl:someValuesFrom rdf:resource="https://w3id.org/def/vaeontology#ConceptNode"/>
                            </owl:Restriction>
                        </owl:complementOf>
                    </owl:Class>
                </owl:intersectionOf>
            </owl:Class>
        </rdfs:domain>
        <rdfs:range rdf:resource="https://w3id.org/def/vaeontology#ValueTaxonomyStatement"/>
        <rdfs:comment>Indicates that the ConceptNode is a root of the ValueTaxonomy (is generalized by none other ConceptNode).</rdfs:comment>
        <rdfs:label>is root node of</rdfs:label>
    </owl:ObjectProperty>
    


    <!-- https://w3id.org/def/vaeontology#isStartOfSequence -->

    <owl:ObjectProperty rdf:about="https://w3id.org/def/vaeontology#isStartOfSequence">
        <rdfs:subPropertyOf rdf:resource="http://www.ontologydesignpatterns.org/ont/dul/DUL.owl#isPropertPartOf"/>
        <rdfs:subPropertyOf rdf:resource="https://w3id.org/def/vaeontology#isInputOutcomeOf"/>
        <owl:inverseOf rdf:resource="https://w3id.org/def/vaeontology#startsWithInputOutcome"/>
        <rdfs:domain rdf:resource="https://w3id.org/def/vaeontology#MultiInputOutcome"/>
        <rdfs:range rdf:resource="https://w3id.org/def/vaeontology#Sequence"/>
        <rdfs:comment>Indicates that the MultiInputOutcome relation is the starting point of some Sequence.</rdfs:comment>
        <rdfs:label>is start of sequence</rdfs:label>
    </owl:ObjectProperty>
    


    <!-- https://w3id.org/def/vaeontology#isStateOfAgent -->

    <owl:ObjectProperty rdf:about="https://w3id.org/def/vaeontology#isStateOfAgent">
        <rdfs:subPropertyOf rdf:resource="http://www.ontologydesignpatterns.org/ont/dul/DUL.owl#involvesAgent"/>
        <rdfs:domain rdf:resource="https://w3id.org/def/vaeontology#State"/>
        <rdfs:range rdf:resource="https://w3id.org/def/vaeontology#Agent"/>
        <rdfs:comment>Indicates that the State represents the Agent supplied.</rdfs:comment>
        <rdfs:label>is state of agent</rdfs:label>
    </owl:ObjectProperty>
    


    <!-- https://w3id.org/def/vaeontology#isTaxonomyNodeOf -->

    <owl:ObjectProperty rdf:about="https://w3id.org/def/vaeontology#isTaxonomyNodeOf">
        <rdfs:subPropertyOf rdf:resource="http://www.ontologydesignpatterns.org/ont/dul/DUL.owl#isComponentOf"/>
        <rdfs:domain>
            <owl:Class>
                <owl:unionOf rdf:parseType="Collection">
                    <rdf:Description rdf:about="https://w3id.org/def/vaeontology#ConceptNode"/>
                    <rdf:Description rdf:about="https://w3id.org/def/vaeontology#PropertyNode"/>
                </owl:unionOf>
            </owl:Class>
        </rdfs:domain>
        <rdfs:range rdf:resource="https://w3id.org/def/vaeontology#ValueTaxonomyStatement"/>
        <rdfs:comment>Indicates that the Node (Concept or Property nodes) are part of a ValueTaxonomy.</rdfs:comment>
        <rdfs:label>is Taxonomy Node Of</rdfs:label>
    </owl:ObjectProperty>
    


    <!-- https://w3id.org/def/vaeontology#isTaxonomyPropertyOf -->

    <owl:ObjectProperty rdf:about="https://w3id.org/def/vaeontology#isTaxonomyPropertyOf">
        <rdfs:subPropertyOf rdf:resource="https://w3id.org/def/vaeontology#propertyExpressedAt"/>
        <rdfs:domain rdf:resource="https://w3id.org/def/vaeontology#TaxonomyProperty"/>
        <rdfs:range rdf:resource="https://w3id.org/def/vaeontology#PropertyNode"/>
        <rdfs:comment>Indicates that the PropertyNode has a Taxonomy Property (a ValueProperty informing of the degree of satisfaction of the taxonomy property).</rdfs:comment>
        <rdfs:label>is PropertyTaxonomy of PropertyNode</rdfs:label>
    </owl:ObjectProperty>
    


    <!-- https://w3id.org/def/vaeontology#isTestedInStatement -->

    <owl:ObjectProperty rdf:about="https://w3id.org/def/vaeontology#isTestedInStatement">
        <rdfs:subPropertyOf rdf:resource="https://w3id.org/def/vaeontology#hasInterpretation"/>
        <owl:inverseOf rdf:resource="https://w3id.org/def/vaeontology#withNorm"/>
        <rdfs:domain rdf:resource="https://w3id.org/def/vaeontology#Norm"/>
        <rdfs:range rdf:resource="https://w3id.org/def/vaeontology#VaeStatement"/>
        <rdfs:comment>Indicates that the norm is being used in a VaeStatement as the evaluated characteristic, e.g. for an AwarenessStatement: &quot;The vae:Agent payerAgent is aware of the vae:Norm [norm]&quot;.</rdfs:comment>
        <rdfs:label>Is Tested in Statement</rdfs:label>
    </owl:ObjectProperty>
    


    <!-- https://w3id.org/def/vaeontology#isTraceOfSystem -->

    <owl:ObjectProperty rdf:about="https://w3id.org/def/vaeontology#isTraceOfSystem">
        <rdfs:subPropertyOf rdf:resource="http://www.ontologydesignpatterns.org/ont/dul/DUL.owl#involvesAgent"/>
        <rdfs:domain rdf:resource="https://w3id.org/def/vaeontology#Sequence"/>
        <rdfs:range rdf:resource="https://w3id.org/def/vaeontology#System"/>
        <rdfs:comment>Indicates that the Sequence is the trace of a System supplied.</rdfs:comment>
        <rdfs:label>is trace of system</rdfs:label>
    </owl:ObjectProperty>
    


    <!-- https://w3id.org/def/vaeontology#isUserOfSystem -->

    <owl:ObjectProperty rdf:about="https://w3id.org/def/vaeontology#isUserOfSystem">
        <rdfs:subPropertyOf rdf:resource="https://w3id.org/def/vaeontology#isAgentOfSystem"/>
        <rdfs:domain rdf:resource="https://w3id.org/def/vaeontology#User"/>
        <rdfs:range rdf:resource="https://w3id.org/def/vaeontology#System"/>
        <rdfs:comment>Indicates that the User is in some System.</rdfs:comment>
        <rdfs:label>is user of system</rdfs:label>
    </owl:ObjectProperty>
    


    <!-- https://w3id.org/def/vaeontology#isValuedInStatement -->

    <owl:ObjectProperty rdf:about="https://w3id.org/def/vaeontology#isValuedInStatement">
        <rdfs:subPropertyOf rdf:resource="https://w3id.org/def/vaeontology#hasInterpretation"/>
        <owl:inverseOf rdf:resource="https://w3id.org/def/vaeontology#withValue"/>
        <rdfs:domain rdf:resource="https://w3id.org/def/vaeontology#ValueConcept"/>
        <rdfs:range rdf:resource="https://w3id.org/def/vaeontology#VaeStatement"/>
        <rdfs:comment>Indicates that the value concept is being used in a VaeStatement as the evaluated characteristic, e.g. for an AlignmentStatement: &quot;The vae:Outcome actOfPayingTaxes is aligned with the vae:ValueConcept [value concept] with a vae:GiniIndex of 0.9&quot;.</rdfs:comment>
        <rdfs:label>is valued in statement</rdfs:label>
    </owl:ObjectProperty>
    


    <!-- https://w3id.org/def/vaeontology#madeByAgent -->

    <owl:ObjectProperty rdf:about="https://w3id.org/def/vaeontology#madeByAgent">
        <rdfs:subPropertyOf rdf:resource="http://www.ontologydesignpatterns.org/ont/dul/DUL.owl#involvesAgent"/>
        <owl:inverseOf rdf:resource="https://w3id.org/def/vaeontology#makesAction"/>
        <rdfs:domain rdf:resource="https://w3id.org/def/vaeontology#Action"/>
        <rdfs:range rdf:resource="https://w3id.org/def/vaeontology#ActingAgent"/>
        <rdfs:comment>Indicates that the Action was made by some ActingAgent.</rdfs:comment>
        <rdfs:label>made by agent</rdfs:label>
    </owl:ObjectProperty>
    


    <!-- https://w3id.org/def/vaeontology#makesAction -->

    <owl:ObjectProperty rdf:about="https://w3id.org/def/vaeontology#makesAction">
        <rdfs:subPropertyOf rdf:resource="http://www.ontologydesignpatterns.org/ont/dul/DUL.owl#isAgentInvolvedIn"/>
        <rdfs:domain rdf:resource="https://w3id.org/def/vaeontology#ActingAgent"/>
        <rdfs:range rdf:resource="https://w3id.org/def/vaeontology#Action"/>
        <rdfs:comment>Indicates that the ActingAgent makes some Action.</rdfs:comment>
        <rdfs:label>makes action</rdfs:label>
    </owl:ObjectProperty>
    


    <!-- https://w3id.org/def/vaeontology#measuredOnOutcome -->

    <owl:ObjectProperty rdf:about="https://w3id.org/def/vaeontology#measuredOnOutcome">
        <rdfs:subPropertyOf rdf:resource="http://www.ontologydesignpatterns.org/ont/dul/DUL.owl#describes"/>
        <rdfs:subPropertyOf rdf:resource="http://www.ontologydesignpatterns.org/ont/dul/DUL.owl#isParticipantIn"/>
        <owl:inverseOf rdf:resource="https://w3id.org/def/vaeontology#satisfiesProperty"/>
        <rdfs:domain rdf:resource="https://w3id.org/def/vaeontology#VaeProperty"/>
        <rdfs:range rdf:resource="https://w3id.org/def/vaeontology#Outcome"/>
        <rdfs:comment>Indicates that the VaeProperty was satisfied (measured) in some Outcome.</rdfs:comment>
        <rdfs:label>measured on outcome</rdfs:label>
    </owl:ObjectProperty>
    


    <!-- https://w3id.org/def/vaeontology#nextInputOutcome -->

    <owl:ObjectProperty rdf:about="https://w3id.org/def/vaeontology#nextInputOutcome">
        <rdfs:subPropertyOf rdf:resource="http://www.ontologydesignpatterns.org/ont/dul/DUL.owl#directlyPrecedes"/>
        <rdfs:subPropertyOf rdf:resource="http://www.ontologydesignpatterns.org/ont/dul/DUL.owl#isConstituentOf"/>
        <owl:inverseOf rdf:resource="https://w3id.org/def/vaeontology#previousInputOutcome"/>
        <rdfs:domain rdf:resource="https://w3id.org/def/vaeontology#MultiInputOutcome"/>
        <rdfs:range rdf:resource="https://w3id.org/def/vaeontology#MultiInputOutcome"/>
        <rdfs:comment>Indicates a next MultiInputOutcome relation in a Sequence.</rdfs:comment>
        <rdfs:label>next input outcome</rdfs:label>
    </owl:ObjectProperty>
    


    <!-- https://w3id.org/def/vaeontology#onEntity -->

    <owl:ObjectProperty rdf:about="https://w3id.org/def/vaeontology#onEntity">
        <rdfs:subPropertyOf rdf:resource="https://w3id.org/def/vaeontology#describesVaeStatementEntity"/>
        <rdfs:domain rdf:resource="https://w3id.org/def/vaeontology#AgentStatement"/>
        <rdfs:range rdf:resource="https://w3id.org/def/vaeontology#VaeConditionedEntity"/>
        <rdfs:comment>Indicates that an Agent or Outcome or Norm is being used in a VaeStatement as an entity subject of evaluation for some characteristic, e.g. for an vae:AwarenessStatement: &quot;The vae:Agent payerAgent is aware of the vae:Norm [norm]&quot;, the entity of the statement is the vae:Agent payerAgent.</rdfs:comment>
        <rdfs:label>on entity</rdfs:label>
    </owl:ObjectProperty>
    


    <!-- https://w3id.org/def/vaeontology#onState -->

    <owl:ObjectProperty rdf:about="https://w3id.org/def/vaeontology#onState">
        <rdfs:subPropertyOf rdf:resource="http://www.ontologydesignpatterns.org/ont/dul/DUL.owl#hasPrecondition"/>
        <rdfs:domain rdf:resource="https://w3id.org/def/vaeontology#ActionOnState"/>
        <rdfs:range rdf:resource="https://w3id.org/def/vaeontology#State"/>
        <rdfs:comment>On a state to action relation (vae:ActionOnState) from a vae:Strategy, indicates the vae:State where some vae:Action should be made by the Agent holding the vae:Strategy.</rdfs:comment>
        <rdfs:label>on state</rdfs:label>
    </owl:ObjectProperty>
    


    <!-- https://w3id.org/def/vaeontology#particularizesNode -->

    <owl:ObjectProperty rdf:about="https://w3id.org/def/vaeontology#particularizesNode">
        <rdfs:subPropertyOf rdf:resource="https://w3id.org/framester/schema/subsumedUnder"/>
        <rdf:type rdf:resource="http://www.w3.org/2002/07/owl#TransitiveProperty"/>
        <rdfs:domain>
            <owl:Class>
                <owl:unionOf rdf:parseType="Collection">
                    <rdf:Description rdf:about="https://w3id.org/def/vaeontology#ConceptNode"/>
                    <rdf:Description rdf:about="https://w3id.org/def/vaeontology#PropertyNode"/>
                </owl:unionOf>
            </owl:Class>
        </rdfs:domain>
        <rdfs:range rdf:resource="https://w3id.org/def/vaeontology#ConceptNode"/>
        <rdfs:comment>Indicates that the ConceptNode or PropertyNode particularizes the ConceptNode  specified (the object ConceptNode generalizes the subject).</rdfs:comment>
        <rdfs:label>particularizes</rdfs:label>
    </owl:ObjectProperty>
    


    <!-- https://w3id.org/def/vaeontology#perform -->

    <owl:ObjectProperty rdf:about="https://w3id.org/def/vaeontology#perform">
        <rdfs:subPropertyOf rdf:resource="http://www.ontologydesignpatterns.org/ont/dul/DUL.owl#hasPostcondition"/>
        <owl:inverseOf rdf:resource="https://w3id.org/def/vaeontology#performedOnStateIn"/>
        <rdfs:domain rdf:resource="https://w3id.org/def/vaeontology#ActionOnState"/>
        <rdfs:range>
            <owl:Class>
                <owl:unionOf rdf:parseType="Collection">
                    <rdf:Description rdf:about="https://w3id.org/def/vaeontology#Action"/>
                    <rdf:Description rdf:about="https://w3id.org/def/vaeontology#Strategy"/>
                </owl:unionOf>
            </owl:Class>
        </rdfs:range>
        <rdfs:comment>Indicates the Action to be performed when an State is given, represented in a ActionOnState relation, which are components of some Strategy.</rdfs:comment>
        <rdfs:label>perform</rdfs:label>
    </owl:ObjectProperty>
    


    <!-- https://w3id.org/def/vaeontology#performedOnStateIn -->

    <owl:ObjectProperty rdf:about="https://w3id.org/def/vaeontology#performedOnStateIn">
        <rdfs:subPropertyOf rdf:resource="http://www.ontologydesignpatterns.org/ont/dul/DUL.owl#isPostconditionOf"/>
        <rdfs:domain>
            <owl:Class>
                <owl:unionOf rdf:parseType="Collection">
                    <rdf:Description rdf:about="https://w3id.org/def/vaeontology#Action"/>
                    <rdf:Description rdf:about="https://w3id.org/def/vaeontology#Strategy"/>
                </owl:unionOf>
            </owl:Class>
        </rdfs:domain>
        <rdfs:range rdf:resource="https://w3id.org/def/vaeontology#ActionOnState"/>
        <rdfs:comment>Indicates the Action to be performed when an State is given, represented in a ActionOnState relation, which are components of some Strategy.</rdfs:comment>
        <rdfs:label>performed on state in</rdfs:label>
    </owl:ObjectProperty>
    


    <!-- https://w3id.org/def/vaeontology#previousInputOutcome -->

    <owl:ObjectProperty rdf:about="https://w3id.org/def/vaeontology#previousInputOutcome">
        <rdfs:subPropertyOf rdf:resource="http://www.ontologydesignpatterns.org/ont/dul/DUL.owl#directlyFollows"/>
        <rdfs:subPropertyOf rdf:resource="http://www.ontologydesignpatterns.org/ont/dul/DUL.owl#isConstituentOf"/>
        <rdfs:domain rdf:resource="https://w3id.org/def/vaeontology#MultiInputOutcome"/>
        <rdfs:range rdf:resource="https://w3id.org/def/vaeontology#MultiInputOutcome"/>
        <rdfs:comment>Indicates a previous MultiInputOutcome relation in a Sequence.</rdfs:comment>
        <rdfs:label>previous input outcome</rdfs:label>
    </owl:ObjectProperty>
    


    <!-- https://w3id.org/def/vaeontology#propertyExpressedAt -->

    <owl:ObjectProperty rdf:about="https://w3id.org/def/vaeontology#propertyExpressedAt">
        <rdfs:subPropertyOf rdf:resource="https://w3id.org/def/vaeontology#isPresentInStatement"/>
        <rdfs:domain rdf:resource="https://w3id.org/def/vaeontology#VaeProperty"/>
        <rdfs:range rdf:resource="https://w3id.org/def/vaeontology#AgentStatement"/>
        <rdfs:comment>Indicates that the VaeProperty is expressed at some VaePropertyStatement.</rdfs:comment>
        <rdfs:label>property expressed at</rdfs:label>
    </owl:ObjectProperty>
    


    <!-- https://w3id.org/def/vaeontology#propertyOptimizedAt -->

    <owl:ObjectProperty rdf:about="https://w3id.org/def/vaeontology#propertyOptimizedAt">
        <rdfs:subPropertyOf rdf:resource="http://www.ontologydesignpatterns.org/ont/dul/DUL.owl#isDescribedBy"/>
        <rdfs:domain rdf:resource="https://w3id.org/def/vaeontology#VaeProperty"/>
        <rdfs:range rdf:resource="https://w3id.org/def/vaeontology#OptimizedProperty"/>
        <rdfs:comment>Indicates that the VaeProperty that is being optimized in the OptimizedProperty assertion.</rdfs:comment>
        <rdfs:label>property optimzed at</rdfs:label>
    </owl:ObjectProperty>
    


    <!-- https://w3id.org/def/vaeontology#proposesStatement -->

    <owl:ObjectProperty rdf:about="https://w3id.org/def/vaeontology#proposesStatement">
        <rdfs:subPropertyOf rdf:resource="http://www.ontologydesignpatterns.org/ont/dul/DUL.owl#conceptualizes"/>
        <rdfs:domain rdf:resource="https://w3id.org/def/vaeontology#Agent"/>
        <rdfs:range rdf:resource="https://w3id.org/def/vaeontology#AgentStatement"/>
        <rdfs:comment>Indicates that the Agent proposes an AgentStatement about the world.</rdfs:comment>
        <rdfs:label>proposes statement</rdfs:label>
    </owl:ObjectProperty>
    


    <!-- https://w3id.org/def/vaeontology#reflectsValue -->

    <owl:ObjectProperty rdf:about="https://w3id.org/def/vaeontology#reflectsValue">
        <owl:inverseOf rdf:resource="https://w3id.org/def/vaeontology#shapesNorm"/>
        <rdfs:domain rdf:resource="https://w3id.org/def/vaeontology#Norm"/>
        <rdfs:range rdf:resource="https://w3id.org/def/vaeontology#ValueConcept"/>
        <rdfs:comment>Said of an Norm reflecting a ValueConcept.</rdfs:comment>
        <rdfs:label>reflects value</rdfs:label>
    </owl:ObjectProperty>
    


    <!-- https://w3id.org/def/vaeontology#relationWith -->

    <owl:ObjectProperty rdf:about="https://w3id.org/def/vaeontology#relationWith">
        <rdfs:subPropertyOf rdf:resource="https://w3id.org/framester/schema/perspectiveOn"/>
        <rdfs:domain rdf:resource="https://w3id.org/def/vaeontology#VaeProperty"/>
        <rdfs:range rdf:resource="https://w3id.org/def/vaeontology#VaeConditioningEntity"/>
    </owl:ObjectProperty>
    


    <!-- https://w3id.org/def/vaeontology#satisfiesNorm -->

    <owl:ObjectProperty rdf:about="https://w3id.org/def/vaeontology#satisfiesNorm">
        <rdfs:domain rdf:resource="https://w3id.org/def/vaeontology#Outcome"/>
        <rdfs:range rdf:resource="https://w3id.org/def/vaeontology#Norm"/>
        <rdfs:comment>Said of an Outcome satisfying a Norm.</rdfs:comment>
        <rdfs:label>satisfies norm</rdfs:label>
    </owl:ObjectProperty>
    


    <!-- https://w3id.org/def/vaeontology#satisfiesProperty -->

    <owl:ObjectProperty rdf:about="https://w3id.org/def/vaeontology#satisfiesProperty">
        <rdfs:subPropertyOf rdf:resource="http://www.ontologydesignpatterns.org/ont/dul/DUL.owl#isDescribedBy"/>
        <rdfs:domain rdf:resource="https://w3id.org/def/vaeontology#Outcome"/>
        <rdfs:range rdf:resource="https://w3id.org/def/vaeontology#VaeProperty"/>
        <rdfs:comment>Indicates that the Outcome satisfies the VaeProperty specified.</rdfs:comment>
        <rdfs:label>satisfies property</rdfs:label>
    </owl:ObjectProperty>
    


    <!-- https://w3id.org/def/vaeontology#shapesNorm -->

    <owl:ObjectProperty rdf:about="https://w3id.org/def/vaeontology#shapesNorm">
        <rdfs:domain rdf:resource="https://w3id.org/def/vaeontology#ValueConcept"/>
        <rdfs:range rdf:resource="https://w3id.org/def/vaeontology#Norm"/>
        <rdfs:comment>Said of a ValueConcept shaping a Norm.</rdfs:comment>
        <rdfs:label>shapes norm</rdfs:label>
    </owl:ObjectProperty>
    


    <!-- https://w3id.org/def/vaeontology#startsWithInputOutcome -->

    <owl:ObjectProperty rdf:about="https://w3id.org/def/vaeontology#startsWithInputOutcome">
        <rdfs:subPropertyOf rdf:resource="http://www.ontologydesignpatterns.org/ont/dul/DUL.owl#hasProperPart"/>
        <rdfs:subPropertyOf rdf:resource="https://w3id.org/def/vaeontology#hasInputOutcome"/>
        <rdfs:domain rdf:resource="https://w3id.org/def/vaeontology#Sequence"/>
        <rdfs:range rdf:resource="https://w3id.org/def/vaeontology#MultiInputOutcome"/>
        <rdfs:comment>Indicates that the vae:Sequence relation starts with a vae:MultiInputOutcome relation.</rdfs:comment>
        <rdfs:label>starts with InputOutcome</rdfs:label>
    </owl:ObjectProperty>
    


    <!-- https://w3id.org/def/vaeontology#superiorInComparison -->

    <owl:ObjectProperty rdf:about="https://w3id.org/def/vaeontology#superiorInComparison">
        <rdfs:subPropertyOf rdf:resource="https://w3id.org/def/vaeontology#hasInterpretation"/>
        <rdfs:domain rdf:resource="https://w3id.org/def/vaeontology#ValueConcept"/>
        <rdfs:range rdf:resource="https://w3id.org/def/vaeontology#ValueComparisonStatement"/>
        <rdfs:comment>Indicates in the ValueComparisonStatement the ValueConcept that is superior to some other inferior one (that is to be supplied in the same ValueComparisonStatement).</rdfs:comment>
        <rdfs:label>superior in comparison</rdfs:label>
    </owl:ObjectProperty>
    


    <!-- https://w3id.org/def/vaeontology#withNorm -->

    <owl:ObjectProperty rdf:about="https://w3id.org/def/vaeontology#withNorm">
        <rdfs:subPropertyOf rdf:resource="https://w3id.org/def/vaeontology#interpretationOn"/>
        <rdfs:domain rdf:resource="https://w3id.org/def/vaeontology#VaeStatement"/>
        <rdfs:range rdf:resource="https://w3id.org/def/vaeontology#Norm"/>
        <rdfs:comment>Indicates that the norm is being used in a VaeStatement as the evaluated characteristic, e.g. for an AwarenessStatement: &quot;The vae:Agent payerAgent is aware of the vae:Norm [norm]&quot;.</rdfs:comment>
        <rdfs:label>with norm</rdfs:label>
    </owl:ObjectProperty>
    


    <!-- https://w3id.org/def/vaeontology#withValue -->

    <owl:ObjectProperty rdf:about="https://w3id.org/def/vaeontology#withValue">
        <rdfs:subPropertyOf rdf:resource="https://w3id.org/def/vaeontology#interpretationOn"/>
        <rdfs:domain rdf:resource="https://w3id.org/def/vaeontology#VaeStatement"/>
        <rdfs:range rdf:resource="https://w3id.org/def/vaeontology#ValueConcept"/>
        <rdfs:comment>Indicates that the value concept is being used in a VaeStatement as the evaluated characteristic, e.g. for an AlignmentStatement: &quot;The vae:Outcome actOfPayingTaxes is aligned with the vae:ValueConcept [value concept] with a vae:GiniIndex of 0.9&quot;.</rdfs:comment>
        <rdfs:label>with value</rdfs:label>
    </owl:ObjectProperty>
    


    <!-- https://w3id.org/framester/schema/hasPerspective -->

    <owl:ObjectProperty rdf:about="https://w3id.org/framester/schema/hasPerspective">
        <owl:inverseOf rdf:resource="https://w3id.org/framester/schema/perspectiveOn"/>
    </owl:ObjectProperty>
    


    <!-- https://w3id.org/framester/schema/perspectiveOn -->

    <owl:ObjectProperty rdf:about="https://w3id.org/framester/schema/perspectiveOn"/>
    


    <!-- https://w3id.org/framester/schema/subsumedUnder -->

    <owl:ObjectProperty rdf:about="https://w3id.org/framester/schema/subsumedUnder">
        <owl:inverseOf rdf:resource="https://w3id.org/framester/schema/subsumes"/>
    </owl:ObjectProperty>
    


    <!-- https://w3id.org/framester/schema/subsumes -->

    <owl:ObjectProperty rdf:about="https://w3id.org/framester/schema/subsumes"/>
    


    <!-- https://w3id.org/spice/SON/SchwartzValues#attitude -->

    <owl:ObjectProperty rdf:about="https://w3id.org/spice/SON/SchwartzValues#attitude"/>
    


    <!-- https://w3id.org/spice/SON/SchwartzValues#focus -->

    <owl:ObjectProperty rdf:about="https://w3id.org/spice/SON/SchwartzValues#focus"/>
    


    <!-- https://w3id.org/spice/SON/SchwartzValues#opposingValueMotivation -->

    <owl:ObjectProperty rdf:about="https://w3id.org/spice/SON/SchwartzValues#opposingValueMotivation"/>
    


    <!-- https://w3id.org/spice/SON/SchwartzValues#valueMotivation -->

    <owl:ObjectProperty rdf:about="https://w3id.org/spice/SON/SchwartzValues#valueMotivation"/>
    


    <!-- 
    ///////////////////////////////////////////////////////////////////////////////////////
    //
    // Data properties
    //
    ///////////////////////////////////////////////////////////////////////////////////////
     -->

    


    <!-- http://www.ontologydesignpatterns.org/ont/dul/DUL.owl#hasDataValue -->

    <owl:DatatypeProperty rdf:about="http://www.ontologydesignpatterns.org/ont/dul/DUL.owl#hasDataValue">
        <rdfs:domain rdf:resource="http://www.ontologydesignpatterns.org/ont/dul/DUL.owl#Entity"/>
    </owl:DatatypeProperty>
    


    <!-- http://www.ontologydesignpatterns.org/ont/dul/DUL.owl#hasEventDate -->

    <owl:DatatypeProperty rdf:about="http://www.ontologydesignpatterns.org/ont/dul/DUL.owl#hasEventDate">
        <rdfs:domain rdf:resource="http://www.ontologydesignpatterns.org/ont/dul/DUL.owl#Event"/>
    </owl:DatatypeProperty>
    


    <!-- http://www.ontologydesignpatterns.org/ont/dul/DUL.owl#hasIntervalDate -->

    <owl:DatatypeProperty rdf:about="http://www.ontologydesignpatterns.org/ont/dul/DUL.owl#hasIntervalDate">
        <rdfs:domain rdf:resource="http://www.ontologydesignpatterns.org/ont/dul/DUL.owl#TimeInterval"/>
    </owl:DatatypeProperty>
    


    <!-- http://www.w3.org/1999/02/22-rdf-syntax-ns#value -->

    <owl:DatatypeProperty rdf:about="http://www.w3.org/1999/02/22-rdf-syntax-ns#value"/>
    


    <!-- https://w3id.org/def/vaeontology#degreeOfSatisfaction -->

    <owl:DatatypeProperty rdf:about="https://w3id.org/def/vaeontology#degreeOfSatisfaction">
        <rdfs:domain rdf:resource="https://w3id.org/def/vaeontology#TaxonomyProperty"/>
        <rdfs:range rdf:resource="http://www.w3.org/2001/XMLSchema#float"/>
        <rdfs:comment>States the degree of satisfaction of an instance of a property used in some ValueTaxonomy (PropertyTaxonomy).</rdfs:comment>
        <rdfs:label>degree of satisfaction</rdfs:label>
    </owl:DatatypeProperty>
    


    <!-- https://w3id.org/def/vaeontology#importanceValue -->

    <owl:DatatypeProperty rdf:about="https://w3id.org/def/vaeontology#importanceValue">
        <rdfs:domain rdf:resource="https://w3id.org/def/vaeontology#NodeImportance"/>
        <rdfs:range rdf:resource="http://www.w3.org/2001/XMLSchema#float"/>
        <rdfs:comment>Defines the importance of a ValueConcept that a ConceptNode or PropertyNode is about.</rdfs:comment>
        <rdfs:label>importance value</rdfs:label>
    </owl:DatatypeProperty>
    


    <!-- https://w3id.org/def/vaeontology#isActive -->

    <owl:DatatypeProperty rdf:about="https://w3id.org/def/vaeontology#isActive">
        <rdfs:domain rdf:resource="https://w3id.org/def/vaeontology#Context"/>
        <rdfs:range rdf:resource="http://www.w3.org/2001/XMLSchema#boolean"/>
        <rdfs:comment>Represents if the Context is active (actually influences any ValueObject).</rdfs:comment>
        <rdfs:label>is active</rdfs:label>
    </owl:DatatypeProperty>
    


    <!-- 
    ///////////////////////////////////////////////////////////////////////////////////////
    //
    // Classes
    //
    ///////////////////////////////////////////////////////////////////////////////////////
     -->

    


    <!-- http://dbpedia.org/resource/Value_(ethics) -->

    <owl:Class rdf:about="http://dbpedia.org/resource/Value_(ethics)">
        <owl:equivalentClass rdf:resource="http://www.ontologydesignpatterns.org/ont/values/valuecore_with_value_frames.owl#Value"/>
        <rdfs:subClassOf rdf:resource="https://w3id.org/def/vaeontology#ValueConcept"/>
    </owl:Class>
    


    <!-- http://schema.org/Action -->

    <owl:Class rdf:about="http://schema.org/Action"/>
    


    <!-- http://www.ontologydesignpatterns.org/ont/dul/DUL.owl#Action -->

    <owl:Class rdf:about="http://www.ontologydesignpatterns.org/ont/dul/DUL.owl#Action">
        <rdfs:subClassOf rdf:resource="http://www.ontologydesignpatterns.org/ont/dul/DUL.owl#Event"/>
        <rdfs:subClassOf>
            <owl:Restriction>
                <owl:onProperty rdf:resource="http://www.ontologydesignpatterns.org/ont/dul/DUL.owl#hasParticipant"/>
                <owl:someValuesFrom rdf:resource="http://www.ontologydesignpatterns.org/ont/dul/DUL.owl#Agent"/>
            </owl:Restriction>
        </rdfs:subClassOf>
        <rdfs:subClassOf>
            <owl:Restriction>
                <owl:onProperty rdf:resource="http://www.ontologydesignpatterns.org/ont/dul/DUL.owl#executesTask"/>
                <owl:minCardinality rdf:datatype="http://www.w3.org/2001/XMLSchema#nonNegativeInteger">1</owl:minCardinality>
            </owl:Restriction>
        </rdfs:subClassOf>
        <rdfs:comment>An Event with at least one Agent that isParticipantIn it, and that executes a Task that typically isDefinedIn a Plan, Workflow, Project, etc.</rdfs:comment>
        <rdfs:isDefinedBy rdf:resource="http://www.ontologydesignpatterns.org/ont/dul/DUL.owl"/>
        <rdfs:label xml:lang="en">Action</rdfs:label>
        <rdfs:label xml:lang="it">Azione</rdfs:label>
    </owl:Class>
    


    <!-- http://www.ontologydesignpatterns.org/ont/dul/DUL.owl#Agent -->

    <owl:Class rdf:about="http://www.ontologydesignpatterns.org/ont/dul/DUL.owl#Agent">
        <rdfs:subClassOf rdf:resource="http://www.ontologydesignpatterns.org/ont/dul/DUL.owl#Object"/>
        <rdfs:comment>Additional comment: a computational agent can be considered as a PhysicalAgent that realizes a certain class of algorithms (that can be considered as instances of InformationObject) that allow to obtain some behaviors that are considered typical of agents in general. For an ontology of computational objects based on DOLCE see e.g. http://www.loa-cnr.it/COS/COS.owl, and http://www.loa-cnr.it/KCO/KCO.owl.</rdfs:comment>
        <rdfs:comment>Any agentive Object , either physical (e.g. a whale, a robot, an oak), or social (e.g. a corporation, an institution, a community).</rdfs:comment>
        <rdfs:isDefinedBy rdf:resource="http://www.ontologydesignpatterns.org/ont/dul/DUL.owl"/>
        <rdfs:label>Agent</rdfs:label>
        <rdfs:label xml:lang="en">Agent</rdfs:label>
        <rdfs:label xml:lang="it">Agente</rdfs:label>
    </owl:Class>
    


    <!-- http://www.ontologydesignpatterns.org/ont/dul/DUL.owl#Collection -->

    <owl:Class rdf:about="http://www.ontologydesignpatterns.org/ont/dul/DUL.owl#Collection">
        <rdfs:subClassOf rdf:resource="http://www.ontologydesignpatterns.org/ont/dul/DUL.owl#SocialObject"/>
        <rdfs:subClassOf>
            <owl:Restriction>
                <owl:onProperty rdf:resource="http://www.ontologydesignpatterns.org/ont/dul/DUL.owl#hasPart"/>
                <owl:allValuesFrom rdf:resource="http://www.ontologydesignpatterns.org/ont/dul/DUL.owl#Collection"/>
            </owl:Restriction>
        </rdfs:subClassOf>
        <rdfs:comment>Any container for entities that share one or more common properties. E.g. &quot;stone objects&quot;, &quot;the nurses&quot;, &quot;the Louvre Aegyptian collection&quot;, all the elections for the Italian President of the Republic. 
A collection is not a logical class: a collection is a first-order entity, while a class is second-order.
A collection is neither an aggregate of its member entities (see e.g. ObjectAggregate class).</rdfs:comment>
        <rdfs:isDefinedBy rdf:resource="http://www.ontologydesignpatterns.org/ont/dul/DUL.owl"/>
        <rdfs:label xml:lang="en">Collection</rdfs:label>
        <rdfs:label xml:lang="it">Collezione</rdfs:label>
    </owl:Class>
    


    <!-- http://www.ontologydesignpatterns.org/ont/dul/DUL.owl#Description -->

    <owl:Class rdf:about="http://www.ontologydesignpatterns.org/ont/dul/DUL.owl#Description">
        <rdfs:subClassOf rdf:resource="http://www.ontologydesignpatterns.org/ont/dul/DUL.owl#SocialObject"/>
        <owl:disjointWith rdf:resource="http://www.ontologydesignpatterns.org/ont/dul/DUL.owl#Situation"/>
        <rdfs:comment>A Description is a SocialObject that represents a conceptualization. 
It can be thought also as a &apos;descriptive context&apos; that uses or defines concepts in order to create a view on a &apos;relational context&apos; (cf. Situation) out of a set of data or observations. 
For example, a Plan is a Description of some actions to be executed by agents in a certain way, with certain parameters; a Diagnosis is a Description that provides an interpretation for a set of observed entities, etc.
Descriptions &apos;define&apos; or &apos;use&apos; concepts, and can be &apos;satisfied&apos; by situations.</rdfs:comment>
        <rdfs:isDefinedBy rdf:resource="http://www.ontologydesignpatterns.org/ont/dul/DUL.owl"/>
        <rdfs:label xml:lang="en">Description</rdfs:label>
        <rdfs:label xml:lang="it">Descrizione</rdfs:label>
    </owl:Class>
    


    <!-- http://www.ontologydesignpatterns.org/ont/dul/DUL.owl#Entity -->

    <owl:Class rdf:about="http://www.ontologydesignpatterns.org/ont/dul/DUL.owl#Entity">
        <rdfs:comment>Anything: real, possible, or imaginary, which some modeller wants to talk about for some purpose.</rdfs:comment>
        <rdfs:isDefinedBy rdf:resource="http://www.ontologydesignpatterns.org/ont/dul/DUL.owl"/>
        <rdfs:label>Entity</rdfs:label>
        <rdfs:label xml:lang="en">Entity</rdfs:label>
        <rdfs:label xml:lang="it">Entità</rdfs:label>
    </owl:Class>
    


    <!-- http://www.ontologydesignpatterns.org/ont/dul/DUL.owl#Event -->

    <owl:Class rdf:about="http://www.ontologydesignpatterns.org/ont/dul/DUL.owl#Event">
        <rdfs:subClassOf rdf:resource="http://www.ontologydesignpatterns.org/ont/dul/DUL.owl#Entity"/>
        <rdfs:subClassOf>
            <owl:Restriction>
                <owl:onProperty rdf:resource="http://www.ontologydesignpatterns.org/ont/dul/DUL.owl#hasParticipant"/>
                <owl:someValuesFrom rdf:resource="http://www.ontologydesignpatterns.org/ont/dul/DUL.owl#Object"/>
            </owl:Restriction>
        </rdfs:subClassOf>
        <rdfs:subClassOf>
            <owl:Restriction>
                <owl:onProperty rdf:resource="http://www.ontologydesignpatterns.org/ont/dul/DUL.owl#hasTimeInterval"/>
                <owl:someValuesFrom rdf:resource="http://www.ontologydesignpatterns.org/ont/dul/DUL.owl#TimeInterval"/>
            </owl:Restriction>
        </rdfs:subClassOf>
        <owl:disjointWith rdf:resource="http://www.ontologydesignpatterns.org/ont/dul/DUL.owl#Object"/>
        <rdfs:comment>Any physical, social, or mental process, event, or state.

More theoretically, events can be classified in different ways, possibly based on &apos;aspect&apos; (e.g. stative, continuous, accomplishement, achievement, etc.), on &apos;agentivity&apos; (e.g. intentional, natural, etc.), or on &apos;typical participants&apos; (e.g. human, physical, abstract, food, etc.).
Here no special direction is taken, and the following explains why: events are related to observable situations, and they can have different views at a same time.
If a position has to be suggested here anyway, the participant-based classification of events seems the most stable and appropriate for many modelling problems.

(1) Alternative aspectual views

Consider a same event &apos;rock erosion in the Sinni valley&apos;: it can be conceptualized as an accomplishment (what has brought a certain state to occur), as an achievement (the state resulting from a previous accomplishment), as a punctual event (if we collapse the time interval of the erosion into a time point), or as a transition (something that has changed from a state to a different one). 
In the erosion case, we could therefore have good motivations to shift from one aspect to another: a) causation focus, b) effectual focus, c) historical condensation, d) transition (causality).

The different views refer to the same event, but are still different: how to live with this seeming paradox? 
A typical solution e.g. in linguistics (cf. Levin&apos;s aspectual classes) and in DOLCE Full (cf. WonderWeb D18 axiomatization) is to classify events based on aspectual differences. But this solution would create different identities for a same event, where the difference is only based on the modeller&apos;s attitude.
An alternative solution is suggested here, and exploits the notion of (observable) Situation; a Situation is a view, consistent with a Description, which can be observed of a set of entities. It can also be seen as a &apos;relational context&apos; created by an observer on the basis of a &apos;frame&apos;. Therefore, a Situation allows to create a context where each particular view can have a proper identity, while the Event preserves its own identity. 
For example, ErosionAsAccomplishment is a Situation where rock erosion is observed as a process leading to a certain achievement: the conditions (roles, parameters) that suggest such view are stated in a Description, which acts as a &apos;theory of accomplishments&apos;. Similarly, ErosionAsTransition is a Situation where rock erosion is observed as an event that has changed a state to another: the conditions for such interpretation are stated in a different Description, which acts as a &apos;theory of state transitions&apos;.
Consider that in no case the actual event is changed or enriched in parts by the aspectual view.

(2) Alternative intentionality views

Similarly to aspectual views, several intentionality views can be provided for a same Event. For example, one can investigate if an avalanche has been caused by immediate natural forces, or if there is any hint of an intentional effort to activate those natural forces.
Also in this case, the Event as such has not different identities, while the causal analysis generates situations with different identities, according to what Description is taken for interpreting the Event. 
On the other hand, if the possible actions of an Agent causing the starting of an avalanche are taken as parts of the Event, then this makes its identity change, because we are adding a part to it. 
Therefore, if intentionality is a criterion to classify events or not, this depends on if an ontology designer wants to consider causality as a relevant dimension for events&apos; identity.

(3) Alternative participant views

A slightly different case is when we consider the basic participants to an Event. In this case, the identity of the Event is affected by the participating objects, because it depends on them. 
For example, if snow, mountain slopes, wind, waves, etc. are considered as an avalanche basic participants, or if we also want to add water, human agents, etc., that makes the identity of an avalanche change.
Anyway, this approach to event classification is based on the designer&apos;s choices, and more accurately mirrors lexical or commonsense classifications (see. e.g. WordNet &apos;supersenses&apos; for verb synsets).

Ultimately, this discussion has no end, because realists will keep defending the idea that events in reality are not changed by the way we describe them, while constructivists will keep defending the idea that, whatever &apos;true reality&apos; is about, it can&apos;t be modelled without the theoretical burden of how we observe and describe it. 
Both positions are in principle valid, but, if taken too radically, they focus on issues that are only partly relevant to the aim of computational ontologies, which assist domain experts in representing a certain portion of reality according to their own assumptions and requirements. 

For this reason, in this ontology version of DOLCE, both events and situations are allowed, together with descriptions (the reason for the inclusion of the D&amp;S framewrok in DOLCE), in order to encode the modelling needs, independently from the position (if any) chosen by the model designer.</rdfs:comment>
        <rdfs:isDefinedBy rdf:resource="http://www.ontologydesignpatterns.org/ont/dul/DUL.owl"/>
        <rdfs:label>Event</rdfs:label>
        <rdfs:label xml:lang="en">Event</rdfs:label>
        <rdfs:label xml:lang="it">Evento</rdfs:label>
    </owl:Class>
    


    <!-- http://www.ontologydesignpatterns.org/ont/dul/DUL.owl#Norm -->

    <owl:Class rdf:about="http://www.ontologydesignpatterns.org/ont/dul/DUL.owl#Norm">
        <rdfs:subClassOf rdf:resource="http://www.ontologydesignpatterns.org/ont/dul/DUL.owl#Description"/>
        <rdfs:comment>A social norm.</rdfs:comment>
        <rdfs:isDefinedBy rdf:resource="http://www.ontologydesignpatterns.org/ont/dul/DUL.owl"/>
        <rdfs:label>Norm</rdfs:label>
        <rdfs:label xml:lang="en">Norm</rdfs:label>
        <rdfs:label xml:lang="it">Norma</rdfs:label>
    </owl:Class>
    


    <!-- http://www.ontologydesignpatterns.org/ont/dul/DUL.owl#Object -->

    <owl:Class rdf:about="http://www.ontologydesignpatterns.org/ont/dul/DUL.owl#Object">
        <rdfs:subClassOf rdf:resource="http://www.ontologydesignpatterns.org/ont/dul/DUL.owl#Entity"/>
        <rdfs:comment>Any physical, social, or mental object, or a substance. Following DOLCE Full, objects are always participating in some event (at least their own life), and are spatially located.</rdfs:comment>
        <rdfs:isDefinedBy rdf:resource="http://www.ontologydesignpatterns.org/ont/dul/DUL.owl"/>
        <rdfs:label xml:lang="en">Object</rdfs:label>
        <rdfs:label xml:lang="it">Oggetto</rdfs:label>
    </owl:Class>
    


    <!-- http://www.ontologydesignpatterns.org/ont/dul/DUL.owl#Person -->

    <owl:Class rdf:about="http://www.ontologydesignpatterns.org/ont/dul/DUL.owl#Person">
        <rdfs:subClassOf rdf:resource="http://www.ontologydesignpatterns.org/ont/dul/DUL.owl#Agent"/>
        <rdfs:comment>Persons in commonsense intuition, which does not apparently distinguish between either natural or social persons.</rdfs:comment>
        <rdfs:isDefinedBy rdf:resource="http://www.ontologydesignpatterns.org/ont/dul/DUL.owl"/>
        <rdfs:label xml:lang="en">Person</rdfs:label>
        <rdfs:label>Persona {it}</rdfs:label>
    </owl:Class>
    


    <!-- http://www.ontologydesignpatterns.org/ont/dul/DUL.owl#Process -->

    <owl:Class rdf:about="http://www.ontologydesignpatterns.org/ont/dul/DUL.owl#Process">
        <rdfs:subClassOf rdf:resource="http://www.ontologydesignpatterns.org/ont/dul/DUL.owl#Event"/>
    </owl:Class>
    


    <!-- http://www.ontologydesignpatterns.org/ont/dul/DUL.owl#Region -->

    <owl:Class rdf:about="http://www.ontologydesignpatterns.org/ont/dul/DUL.owl#Region">
        <rdfs:subClassOf rdf:resource="http://www.ontologydesignpatterns.org/ont/dul/DUL.owl#Entity"/>
        <rdfs:label>Region</rdfs:label>
    </owl:Class>
    


    <!-- http://www.ontologydesignpatterns.org/ont/dul/DUL.owl#Situation -->

    <owl:Class rdf:about="http://www.ontologydesignpatterns.org/ont/dul/DUL.owl#Situation">
        <rdfs:subClassOf rdf:resource="http://www.ontologydesignpatterns.org/ont/dul/DUL.owl#Entity"/>
        <rdfs:subClassOf>
            <owl:Restriction>
                <owl:onProperty rdf:resource="http://www.ontologydesignpatterns.org/ont/dul/DUL.owl#satisfies"/>
                <owl:someValuesFrom rdf:resource="http://www.ontologydesignpatterns.org/ont/dul/DUL.owl#Description"/>
            </owl:Restriction>
        </rdfs:subClassOf>
        <rdfs:comment>A view, consistent with (&apos;satisfying&apos;) a Description, on a set of entities. 
It can also be seen as a &apos;relational context&apos; created by an observer on the basis of a &apos;frame&apos; (i.e. a Description). 
For example, a PlanExecution is a context including some actions executed by agents according to certain parameters and expected tasks to be achieved from a Plan; a DiagnosedSituation is a context of observed entities that is interpreted on the basis of a Diagnosis, etc.
Situation is also able to represent reified n-ary relations, where isSettingFor is the top-level relation for all binary projections of the n-ary relation. 
If used in a transformation pattern for n-ary relations, the designer should take care of adding (some or all) OWL2 keys, corresponding to binary projections of the n-ary, to a subclass of Situation. Otherwise the &apos;identification constraint&apos; (Calvanese et al., IJCAI 2001) might be violated.</rdfs:comment>
        <rdfs:isDefinedBy rdf:resource="http://www.ontologydesignpatterns.org/ont/dul/DUL.owl"/>
        <rdfs:label xml:lang="en">Situation</rdfs:label>
        <rdfs:label xml:lang="it">Situazione</rdfs:label>
    </owl:Class>
    


    <!-- http://www.ontologydesignpatterns.org/ont/dul/DUL.owl#SocialObject -->

    <owl:Class rdf:about="http://www.ontologydesignpatterns.org/ont/dul/DUL.owl#SocialObject">
        <rdfs:subClassOf rdf:resource="http://www.ontologydesignpatterns.org/ont/dul/DUL.owl#Object"/>
        <rdfs:comment>Any Object that exists only within some communication Event, in which at least one PhysicalObject participates in. 
In other words, all objects that have been or are created in the process of social communication: for the sake of communication (InformationObject), for incorporating new individuals (SocialAgent, Place), for contextualizing or intepreting existing entities (Description, Concept), or for collecting existing entities (Collection).
Being dependent on communication, all social objects need to be expressed by some information object (information objects are self-expressing).</rdfs:comment>
        <rdfs:isDefinedBy rdf:resource="http://www.ontologydesignpatterns.org/ont/dul/DUL.owl"/>
        <rdfs:label xml:lang="it">Oggetto sociale</rdfs:label>
        <rdfs:label xml:lang="en">Social object</rdfs:label>
    </owl:Class>
    


    <!-- http://www.ontologydesignpatterns.org/ont/dul/DUL.owl#Theory -->

    <owl:Class rdf:about="http://www.ontologydesignpatterns.org/ont/dul/DUL.owl#Theory">
        <rdfs:subClassOf rdf:resource="http://www.ontologydesignpatterns.org/ont/dul/DUL.owl#Description"/>
        <rdfs:comment>A Theory is a Description that represents a set of assumptions for describing something, usually general. Scientific, philosophical, and commonsense theories can be included here.
This class can also be used to act as &apos;naturalized reifications&apos; of logical theories (of course, they will be necessarily incomplete in this case, because second-order entities are represented as first-order ones).</rdfs:comment>
        <rdfs:isDefinedBy rdf:resource="http://www.ontologydesignpatterns.org/ont/dul/DUL.owl"/>
        <rdfs:label xml:lang="it">Teoria</rdfs:label>
        <rdfs:label>Theory</rdfs:label>
        <rdfs:label xml:lang="en">Theory</rdfs:label>
    </owl:Class>
    


    <!-- http://www.ontologydesignpatterns.org/ont/dul/DUL.owl#TimeInterval -->

    <owl:Class rdf:about="http://www.ontologydesignpatterns.org/ont/dul/DUL.owl#TimeInterval">
        <rdfs:subClassOf rdf:resource="http://www.ontologydesignpatterns.org/ont/dul/DUL.owl#Region"/>
        <rdfs:comment>Any Region in a dimensional space that aims at representing time.</rdfs:comment>
        <rdfs:isDefinedBy rdf:resource="http://www.ontologydesignpatterns.org/ont/dul/DUL.owl"/>
        <rdfs:label xml:lang="it">Intervallo di tempo</rdfs:label>
        <rdfs:label xml:lang="en">Time interval</rdfs:label>
    </owl:Class>
    


    <!-- http://www.ontologydesignpatterns.org/ont/values/valuecore_with_value_frames.owl#Value -->

    <owl:Class rdf:about="http://www.ontologydesignpatterns.org/ont/values/valuecore_with_value_frames.owl#Value">
        <owl:equivalentClass rdf:resource="https://w3id.org/def/vaeontology#Value"/>
        <owl:equivalentClass rdf:resource="https://w3id.org/spice/SON/SchwartzValues#Value"/>
        <rdfs:subClassOf rdf:resource="https://w3id.org/def/vaeontology#Value"/>
        <rdfs:comment>Schwartz: The relative importance of multiple values guides action. Any attitude or behaviour typically has implications for more than one value. … The tradeoff among relevant, competing values guides attitudes and behaviors… Values influence action when they are relevant in the context (hence likely to be activated) and important to the actor.</rdfs:comment>
        <rdfs:comment>Schwartz: Values are beliefs linked inextricably to affect. When values are activated, they become infused with feeling.</rdfs:comment>
        <rdfs:comment>Schwartz: Values are ordered by importance relative to one another. People’s values form an ordered system of priorities that characterize them as individuals.</rdfs:comment>
        <rdfs:comment>Schwartz: Values refer to desirable goals that motivate action.</rdfs:comment>
        <rdfs:comment>Schwartz: Values serve as standards or criteria. Values guide the selection or evaluation of actions, policies, people, and events. People decide what is good or bad, justified or illegitimate, worth doing or avoiding, based on possible consequences for their cherished values. But the impact of values in everyday decisions is rarely conscious. Values enter awareness when the actions or judgments one is considering have conflicting implications for different values one cherishes.</rdfs:comment>
        <rdfs:comment>Schwartz: Values transcend specific actions and situations. … This feature distinguishes values from norms and attitudes that usually refer to specific actions, objects, or situations.</rdfs:comment>
        <rdfs:label>value</rdfs:label>
    </owl:Class>
    


    <!-- http://www.w3.org/ns/odrl/2/Action -->

    <owl:Class rdf:about="http://www.w3.org/ns/odrl/2/Action">
        <rdfs:subClassOf rdf:resource="http://schema.org/Action"/>
        <rdfs:isDefinedBy rdf:resource="http://www.w3.org/ns/odrl/2/"/>
        <rdfs:label>Action</rdfs:label>
        <rdfs:label xml:lang="en">Action</rdfs:label>
        <skos:definition xml:lang="en">An operation on an Asset.</skos:definition>
        <skos:note xml:lang="en">Actions may be allowed by Permissions, disallowed by Prohibitions, or made mandatory by Duties.</skos:note>
    </owl:Class>
    


    <!-- http://www.w3.org/ns/odrl/2/Asset -->

    <owl:Class rdf:about="http://www.w3.org/ns/odrl/2/Asset">
        <owl:disjointWith rdf:resource="http://www.w3.org/ns/odrl/2/Constraint"/>
        <rdfs:isDefinedBy rdf:resource="http://www.w3.org/ns/odrl/2/"/>
        <rdfs:label>Asset</rdfs:label>
        <rdfs:label xml:lang="en">Asset</rdfs:label>
        <skos:definition xml:lang="en">A resource or a collection of resources that are the subject of a Rule.</skos:definition>
        <skos:note xml:lang="en">The Asset entity can be any form of identifiable resource, such as data/information, content/media, applications, or services. Furthermore, it can be used to represent other Asset entities that are needed to undertake the Policy expression, such as with the Duty entity. To describe more details about the Asset, it is recommended to use Dublin Core [[dcterms]] elements or other content metadata.</skos:note>
    </owl:Class>
    


    <!-- http://www.w3.org/ns/odrl/2/Constraint -->

    <owl:Class rdf:about="http://www.w3.org/ns/odrl/2/Constraint">
        <rdfs:isDefinedBy rdf:resource="http://www.w3.org/ns/odrl/2/"/>
        <rdfs:label>Constraint</rdfs:label>
        <rdfs:label xml:lang="en">Constraint</rdfs:label>
        <skos:definition xml:lang="en">A boolean expression that refines the semantics of an Action and Party/Asset Collection or declare the conditions applicable to a Rule.</skos:definition>
    </owl:Class>
    


    <!-- http://www.w3.org/ns/odrl/2/LogicalConstraint -->

    <owl:Class rdf:about="http://www.w3.org/ns/odrl/2/LogicalConstraint"/>
    


    <!-- http://www.w3.org/ns/odrl/2/Operator -->

    <owl:Class rdf:about="http://www.w3.org/ns/odrl/2/Operator">
        <rdfs:isDefinedBy rdf:resource="http://www.w3.org/ns/odrl/2/"/>
        <rdfs:label>Operator</rdfs:label>
        <rdfs:label xml:lang="en">Operator</rdfs:label>
        <skos:definition xml:lang="en">Operator for constraint expression.</skos:definition>
        <skos:note xml:lang="en">Instances of the Operator class representing relational operators.</skos:note>
    </owl:Class>
    


    <!-- http://www.w3.org/ns/odrl/2/Party -->

    <owl:Class rdf:about="http://www.w3.org/ns/odrl/2/Party">
        <rdfs:isDefinedBy rdf:resource="http://www.w3.org/ns/odrl/2/"/>
        <rdfs:label>Party</rdfs:label>
        <rdfs:label xml:lang="en">Party</rdfs:label>
        <skos:definition xml:lang="en">An entity or a collection of entities that undertake Roles in a Rule.</skos:definition>
        <skos:note xml:lang="en">The Party entity could be a person, group of people, organisation, or agent. An agent is a person or thing that takes an active role or produces a specified effect. To describe more details about the Party, it is recommended to use W3C vCard Ontology [[vcard-rdf]] or FOAF Vocabulary [[foaf]].</skos:note>
    </owl:Class>
    


    <!-- http://www.w3.org/ns/odrl/2/Policy -->

    <owl:Class rdf:about="http://www.w3.org/ns/odrl/2/Policy">
        <rdfs:isDefinedBy rdf:resource="http://www.w3.org/ns/odrl/2/"/>
        <rdfs:label>Policy</rdfs:label>
        <rdfs:label xml:lang="en">Policy</rdfs:label>
        <skos:definition xml:lang="en">A non-empty group of Permissions and/or Prohibitions.</skos:definition>
        <skos:note xml:lang="en">A Policy may contain multiple Rules.</skos:note>
    </owl:Class>
    


    <!-- http://www.w3.org/ns/odrl/2/Rule -->

    <owl:Class rdf:about="http://www.w3.org/ns/odrl/2/Rule"/>
    


    <!-- https://w3id.org/def/vaeontology#Abidance -->

    <owl:Class rdf:about="https://w3id.org/def/vaeontology#Abidance">
        <rdfs:subClassOf rdf:resource="https://w3id.org/spice/SON/SchwartzValues#Conformity"/>
        <rdfs:comment>Abidance: acting according to certain accepted standards</rdfs:comment>
        <rdfs:comment>Term added automatically</rdfs:comment>
        <rdfs:label>Abidance</rdfs:label>
    </owl:Class>
    


    <!-- https://w3id.org/def/vaeontology#Accomplishment -->

    <owl:Class rdf:about="https://w3id.org/def/vaeontology#Accomplishment">
        <rdfs:subClassOf rdf:resource="https://w3id.org/spice/SON/SchwartzValues#Achievement"/>
        <rdfs:comment>Accomplishment: the action of accomplishing something</rdfs:comment>
        <rdfs:comment>Term added automatically</rdfs:comment>
        <rdfs:label>Accomplishment</rdfs:label>
    </owl:Class>
    


    <!-- https://w3id.org/def/vaeontology#Accord -->

    <owl:Class rdf:about="https://w3id.org/def/vaeontology#Accord">
        <rdfs:subClassOf rdf:resource="https://w3id.org/spice/SON/SchwartzValues#Conformity"/>
        <rdfs:comment>Accord: concurrence of opinion</rdfs:comment>
        <rdfs:comment>Term added automatically</rdfs:comment>
        <rdfs:label>Accord</rdfs:label>
    </owl:Class>
    


    <!-- https://w3id.org/def/vaeontology#Accordance -->

    <owl:Class rdf:about="https://w3id.org/def/vaeontology#Accordance">
        <rdfs:subClassOf rdf:resource="https://w3id.org/spice/SON/SchwartzValues#Conformity"/>
        <rdfs:comment>Accordance: concurrence of opinion</rdfs:comment>
        <rdfs:comment>Term added automatically</rdfs:comment>
        <rdfs:label>Accordance</rdfs:label>
    </owl:Class>
    


    <!-- https://w3id.org/def/vaeontology#ActingAgent -->

    <owl:Class rdf:about="https://w3id.org/def/vaeontology#ActingAgent">
        <rdfs:subClassOf rdf:resource="https://w3id.org/def/vaeontology#Agent"/>
        <rdfs:subClassOf>
            <owl:Restriction>
                <owl:onProperty rdf:resource="http://www.ontologydesignpatterns.org/ont/dul/DUL.owl#isParticipantIn"/>
                <owl:someValuesFrom rdf:resource="https://w3id.org/def/vaeontology#Action"/>
            </owl:Restriction>
        </rdfs:subClassOf>
        <rdfs:subClassOf>
            <owl:Restriction>
                <owl:onProperty rdf:resource="https://w3id.org/def/vaeontology#followsStrategy"/>
                <owl:someValuesFrom rdf:resource="https://w3id.org/def/vaeontology#Strategy"/>
            </owl:Restriction>
        </rdfs:subClassOf>
        <rdfs:subClassOf>
            <owl:Restriction>
                <owl:onProperty rdf:resource="https://w3id.org/def/vaeontology#makesAction"/>
                <owl:allValuesFrom rdf:resource="https://w3id.org/def/vaeontology#Action"/>
            </owl:Restriction>
        </rdfs:subClassOf>
        <rdfs:comment>An Agent that makes Actions and/or follows some Strategy</rdfs:comment>
        <rdfs:label>Acting Agent</rdfs:label>
    </owl:Class>
    


    <!-- https://w3id.org/def/vaeontology#Action -->

    <owl:Class rdf:about="https://w3id.org/def/vaeontology#Action">
        <rdfs:subClassOf rdf:resource="http://www.ontologydesignpatterns.org/ont/dul/DUL.owl#Action"/>
        <rdfs:subClassOf rdf:resource="https://w3id.org/def/vaeontology#Outcome"/>
        <rdfs:comment>An action that produces some effect in the world, made possible by some ActingAgent.</rdfs:comment>
        <rdfs:label>Action</rdfs:label>
        <rdfs:seeAlso rdf:resource="https://w3id.org/def/vaeontology#ActingAgent"/>
    </owl:Class>
    


    <!-- https://w3id.org/def/vaeontology#ActionOnState -->

    <owl:Class rdf:about="https://w3id.org/def/vaeontology#ActionOnState">
        <rdfs:subClassOf rdf:resource="https://w3id.org/def/vaeontology#Outcome"/>
        <rdfs:subClassOf>
            <owl:Restriction>
                <owl:onProperty rdf:resource="https://w3id.org/def/vaeontology#onState"/>
                <owl:someValuesFrom rdf:resource="https://w3id.org/def/vaeontology#State"/>
            </owl:Restriction>
        </rdfs:subClassOf>
        <rdfs:subClassOf>
            <owl:Restriction>
                <owl:onProperty rdf:resource="https://w3id.org/def/vaeontology#perform"/>
                <owl:someValuesFrom>
                    <owl:Class>
                        <owl:unionOf rdf:parseType="Collection">
                            <rdf:Description rdf:about="https://w3id.org/def/vaeontology#Action"/>
                            <rdf:Description rdf:about="https://w3id.org/def/vaeontology#Strategy"/>
                        </owl:unionOf>
                    </owl:Class>
                </owl:someValuesFrom>
            </owl:Restriction>
        </rdfs:subClassOf>
        <rdfs:comment>A policy that defines that, on some given State, an Action is to be made. These are the basic components of Strategies which followed by ActingAgents.</rdfs:comment>
        <rdfs:label>Action On State</rdfs:label>
    </owl:Class>
    


    <!-- https://w3id.org/def/vaeontology#Agent -->

    <owl:Class rdf:about="https://w3id.org/def/vaeontology#Agent">
        <rdfs:subClassOf rdf:resource="http://www.ontologydesignpatterns.org/ont/dul/DUL.owl#Agent"/>
        <rdfs:subClassOf rdf:resource="http://www.w3.org/ns/odrl/2/Party"/>
        <rdfs:subClassOf rdf:resource="https://w3id.org/def/vaeontology#VaeConditionedEntity"/>
        <rdfs:comment>An agent that takes part in a problem of interest, either by commiting to a ValueConcept or by participating in some Outcome.</rdfs:comment>
        <rdfs:label>Agent</rdfs:label>
    </owl:Class>
    


    <!-- https://w3id.org/def/vaeontology#AgentStatement -->

    <owl:Class rdf:about="https://w3id.org/def/vaeontology#AgentStatement">
        <owl:equivalentClass>
            <owl:Class>
                <owl:intersectionOf rdf:parseType="Collection">
                    <owl:Restriction>
                        <owl:onProperty rdf:resource="http://www.ontologydesignpatterns.org/ont/dul/DUL.owl#hasSetting"/>
                        <owl:someValuesFrom rdf:resource="https://w3id.org/def/vaeontology#Context"/>
                    </owl:Restriction>
                    <owl:Restriction>
                        <owl:onProperty rdf:resource="https://w3id.org/def/vaeontology#isProposedByAgent"/>
                        <owl:someValuesFrom rdf:resource="https://w3id.org/def/vaeontology#Agent"/>
                    </owl:Restriction>
                </owl:intersectionOf>
            </owl:Class>
        </owl:equivalentClass>
        <rdfs:subClassOf rdf:resource="http://www.ontologydesignpatterns.org/ont/dul/DUL.owl#Description"/>
        <rdfs:subClassOf rdf:resource="https://w3id.org/def/vaeontology#VaeEntity"/>
        <rdfs:comment>An AgentStatement is whatever statement proposed by an Agent in some context about the world.</rdfs:comment>
        <rdfs:label>Agent Statement</rdfs:label>
    </owl:Class>
    


    <!-- https://w3id.org/def/vaeontology#AggregationFunction -->

    <owl:Class rdf:about="https://w3id.org/def/vaeontology#AggregationFunction">
        <rdfs:subClassOf rdf:resource="https://w3id.org/def/vaeontology#QuantitativeVaeProperty"/>
        <rdfs:comment>An aggregation of some other VaeProperty over a set of Outcomes (or Sequence).</rdfs:comment>
        <rdfs:label>Aggregation Function</rdfs:label>
    </owl:Class>
    


    <!-- https://w3id.org/def/vaeontology#AlignmentSituation -->

    <owl:Class rdf:about="https://w3id.org/def/vaeontology#AlignmentSituation">
        <rdfs:subClassOf rdf:resource="https://w3id.org/def/vaeontology#VaeSituation"/>
        <rdfs:subClassOf>
            <owl:Restriction>
                <owl:onProperty rdf:resource="http://www.ontologydesignpatterns.org/ont/dul/DUL.owl#satisfies"/>
                <owl:someValuesFrom rdf:resource="https://w3id.org/def/vaeontology#AlignmentStatement"/>
            </owl:Restriction>
        </rdfs:subClassOf>
        <rdfs:comment>[Luc Steels: https://vale2023.iiia.csic.es/accepted-papers]  &quot;When norms properly reflect values we say that the norms are value-aligned.” + (previously) “The application of norms always implies situation-awareness first.”</rdfs:comment>
        <rdfs:comment>[Luc Steels: https://vale2023.iiia.csic.es/accepted-papers]  “… when the outcomes adequately abide by values - possibly because they satisfy entirely the (value-aligned) norms - we say that these outcomes are value-aligned.”</rdfs:comment>
        <rdfs:label>Alignment Statement</rdfs:label>
        <skos:note>References for the specific ways of certifying alignment: [Nieves Montes, Carles Sierra et al. (Gini Index - Semantics Functions, Preferences,  Promotion, Demotion, Optimally aligned norms) https://www.jair.org/index.php/jair/article/view/13487], [Lera Leri et al. (“Moral Value Interpretation”) https://www.iiia.csic.es/media/filer_public/06/0a/060aec7a-2db6-40d7-b3e6-67de4260a065/2022aamaspluralisticvaluealignment.pdf], [Andrés Holgado-Sánchez (Admissibility of sequences of outcomes) https://link.springer.com/chapter/10.1007/978-3-031-43264-4_27]</skos:note>
    </owl:Class>
    


    <!-- https://w3id.org/def/vaeontology#AlignmentStatement -->

    <owl:Class rdf:about="https://w3id.org/def/vaeontology#AlignmentStatement">
        <rdfs:subClassOf rdf:resource="https://w3id.org/def/vaeontology#VaeStatement"/>
        <rdfs:subClassOf>
            <owl:Class>
                <owl:unionOf rdf:parseType="Collection">
                    <owl:Restriction>
                        <owl:onProperty rdf:resource="https://w3id.org/def/vaeontology#onEntity"/>
                        <owl:someValuesFrom rdf:resource="https://w3id.org/def/vaeontology#Norm"/>
                    </owl:Restriction>
                    <owl:Restriction>
                        <owl:onProperty rdf:resource="https://w3id.org/def/vaeontology#onEntity"/>
                        <owl:someValuesFrom rdf:resource="https://w3id.org/def/vaeontology#Outcome"/>
                    </owl:Restriction>
                </owl:unionOf>
            </owl:Class>
        </rdfs:subClassOf>
        <rdfs:subClassOf>
            <owl:Class>
                <owl:complementOf>
                    <owl:Restriction>
                        <owl:onProperty rdf:resource="https://w3id.org/def/vaeontology#withNorm"/>
                        <owl:someValuesFrom rdf:resource="https://w3id.org/def/vaeontology#Norm"/>
                    </owl:Restriction>
                </owl:complementOf>
            </owl:Class>
        </rdfs:subClassOf>
        <rdfs:subClassOf>
            <owl:Restriction>
                <owl:onProperty rdf:resource="https://w3id.org/def/vaeontology#withValue"/>
                <owl:someValuesFrom rdf:resource="https://w3id.org/def/vaeontology#ValueConcept"/>
            </owl:Restriction>
        </rdfs:subClassOf>
        <owl:disjointWith rdf:resource="https://w3id.org/def/vaeontology#AwarenessStatement"/>
        <rdfs:comment>[Luc Steels: https://vale2023.iiia.csic.es/accepted-papers]  &quot;When norms properly reflect values we say that the norms are value-aligned.” + (previously) “The application of norms always implies situation-awareness first.”</rdfs:comment>
        <rdfs:comment>[Luc Steels: https://vale2023.iiia.csic.es/accepted-papers]  “… when the outcomes adequately abide by values - possibly because they satisfy entirely the (value-aligned) norms - we say that these outcomes are value-aligned.”</rdfs:comment>
        <rdfs:label>Alignment Statement</rdfs:label>
        <rdfs:seeAlso rdf:resource="https://w3id.org/def/vaeontology#AwarenessStatement"/>
        <skos:note>References for the specific ways of certifying alignment: [Nieves Montes, Carles Sierra et al. (Gini Index - Semantics Functions, Preferences,  Promotion, Demotion, Optimally aligned norms) https://www.jair.org/index.php/jair/article/view/13487], [Lera Leri et al. (“Moral Value Interpretation”) https://www.iiia.csic.es/media/filer_public/06/0a/060aec7a-2db6-40d7-b3e6-67de4260a065/2022aamaspluralisticvaluealignment.pdf], [Andrés Holgado-Sánchez (Admissibility of sequences of outcomes) https://link.springer.com/chapter/10.1007/978-3-031-43264-4_27]</skos:note>
    </owl:Class>
    


    <!-- https://w3id.org/def/vaeontology#Allowance -->

    <owl:Class rdf:about="https://w3id.org/def/vaeontology#Allowance">
        <rdfs:subClassOf rdf:resource="https://w3id.org/spice/SON/SchwartzValues#Tolerance"/>
        <rdfs:comment>Allowance: a permissible difference; allowing some freedom to move within limits</rdfs:comment>
        <rdfs:comment>Term added automatically</rdfs:comment>
        <rdfs:label>Allowance</rdfs:label>
    </owl:Class>
    


    <!-- https://w3id.org/def/vaeontology#ArgumentStatement -->

    <owl:Class rdf:about="https://w3id.org/def/vaeontology#ArgumentStatement">
        <rdfs:subClassOf rdf:resource="https://w3id.org/def/vaeontology#AgentStatement"/>
        <rdfs:subClassOf>
            <owl:Restriction>
                <owl:onProperty rdf:resource="https://w3id.org/def/vaeontology#hasClaim"/>
                <owl:someValuesFrom rdf:resource="https://w3id.org/def/vaeontology#VaeStatement"/>
            </owl:Restriction>
        </rdfs:subClassOf>
        <rdfs:subClassOf>
            <owl:Restriction>
                <owl:onProperty rdf:resource="https://w3id.org/def/vaeontology#isProposedByAgent"/>
                <owl:someValuesFrom rdf:resource="https://w3id.org/def/vaeontology#Agent"/>
            </owl:Restriction>
        </rdfs:subClassOf>
        <rdfs:subClassOf>
            <owl:Restriction>
                <owl:onProperty rdf:resource="https://w3id.org/def/vaeontology#hasPremise"/>
                <owl:allValuesFrom rdf:resource="https://w3id.org/def/vaeontology#VaeStatement"/>
            </owl:Restriction>
        </rdfs:subClassOf>
        <rdfs:subClassOf>
            <owl:Restriction>
                <owl:onProperty rdf:resource="https://w3id.org/def/vaeontology#isBasedOnCriterion"/>
                <owl:allValuesFrom rdf:resource="https://w3id.org/def/vaeontology#Criterion"/>
            </owl:Restriction>
        </rdfs:subClassOf>
        <rdfs:comment>An ArgumentStatement is a AgentStatment where a claim is made directly characterizing some value or norm related content (VaeStatement), justified by using other statements (premises) and based on some Criterion.</rdfs:comment>
        <rdfs:comment>[Luc Steels: https://vale2023.iiia.csic.es/accepted-papers]  “One of the big advantages of explicit representations is that outcomes can be explained by the system itself in terms of norms and values. For example, a user can ask why he is blocked on a social media platform and this is then explained in terms of which community rules he broke and possibly what values these rules reflect (i.e. why the norm was adopted)”.</rdfs:comment>
        <rdfs:label>Argument Statement</rdfs:label>
    </owl:Class>
    


    <!-- https://w3id.org/def/vaeontology#AwarenessSituation -->

    <owl:Class rdf:about="https://w3id.org/def/vaeontology#AwarenessSituation">
        <rdfs:subClassOf rdf:resource="https://w3id.org/def/vaeontology#VaeSituation"/>
        <rdfs:subClassOf>
            <owl:Restriction>
                <owl:onProperty rdf:resource="http://www.ontologydesignpatterns.org/ont/dul/DUL.owl#satisfies"/>
                <owl:someValuesFrom rdf:resource="https://w3id.org/def/vaeontology#AwarenessStatement"/>
            </owl:Restriction>
        </rdfs:subClassOf>
        <rdfs:comment>[Luc Steels: https://vale2023.iiia.csic.es/accepted-papers] “… a system can be given a formal representation of the norms and/or values that determine its behavior or the behavior it expects from its users. In this case we say that the system is norm and/or value-aware.”</rdfs:comment>
        <rdfs:label>Awareness Statement</rdfs:label>
    </owl:Class>
    


    <!-- https://w3id.org/def/vaeontology#AwarenessStatement -->

    <owl:Class rdf:about="https://w3id.org/def/vaeontology#AwarenessStatement">
        <rdfs:subClassOf rdf:resource="https://w3id.org/def/vaeontology#VaeStatement"/>
        <rdfs:subClassOf>
            <owl:Class>
                <owl:unionOf rdf:parseType="Collection">
                    <owl:Restriction>
                        <owl:onProperty rdf:resource="https://w3id.org/def/vaeontology#withNorm"/>
                        <owl:someValuesFrom rdf:resource="https://w3id.org/def/vaeontology#Norm"/>
                    </owl:Restriction>
                    <owl:Restriction>
                        <owl:onProperty rdf:resource="https://w3id.org/def/vaeontology#withValue"/>
                        <owl:someValuesFrom rdf:resource="https://w3id.org/def/vaeontology#ValueConcept"/>
                    </owl:Restriction>
                </owl:unionOf>
            </owl:Class>
        </rdfs:subClassOf>
        <rdfs:subClassOf>
            <owl:Restriction>
                <owl:onProperty rdf:resource="https://w3id.org/def/vaeontology#onEntity"/>
                <owl:someValuesFrom rdf:resource="https://w3id.org/def/vaeontology#Agent"/>
            </owl:Restriction>
        </rdfs:subClassOf>
        <rdfs:subClassOf>
            <owl:Restriction>
                <owl:onProperty rdf:resource="https://w3id.org/def/vaeontology#onEntity"/>
                <owl:allValuesFrom rdf:resource="https://w3id.org/def/vaeontology#Agent"/>
            </owl:Restriction>
        </rdfs:subClassOf>
        <rdfs:comment>[Luc Steels: https://vale2023.iiia.csic.es/accepted-papers] “… a system can be given a formal representation of the norms and/or values that determine its behavior or the behavior it expects from its users. In this case we say that the system is norm and/or value-aware.”</rdfs:comment>
        <rdfs:label>Awareness Statement</rdfs:label>
        <rdfs:seeAlso rdf:resource="https://w3id.org/def/vaeontology#AlignmentStatement"/>
    </owl:Class>
    


    <!-- https://w3id.org/def/vaeontology#BooleanVaeProperty -->

    <owl:Class rdf:about="https://w3id.org/def/vaeontology#BooleanVaeProperty">
        <rdfs:subClassOf rdf:resource="https://w3id.org/def/vaeontology#VaeProperty"/>
        <rdfs:comment>A VaeProperty taken boolean values.</rdfs:comment>
        <rdfs:label>Boolean Vae Property</rdfs:label>
    </owl:Class>
    


    <!-- https://w3id.org/def/vaeontology#Compliance -->

    <owl:Class rdf:about="https://w3id.org/def/vaeontology#Compliance">
        <rdfs:subClassOf rdf:resource="https://w3id.org/spice/SON/SchwartzValues#Conformity"/>
        <rdfs:comment>Compliance: acting according to certain accepted standards</rdfs:comment>
        <rdfs:comment>Term added automatically</rdfs:comment>
        <rdfs:label>Compliance</rdfs:label>
    </owl:Class>
    


    <!-- https://w3id.org/def/vaeontology#ConceptNode -->

    <owl:Class rdf:about="https://w3id.org/def/vaeontology#ConceptNode">
        <rdfs:subClassOf rdf:resource="https://w3id.org/def/vaeontology#VaePropertyStatement"/>
        <rdfs:subClassOf>
            <owl:Restriction>
                <owl:onProperty rdf:resource="https://w3id.org/def/vaeontology#isConceptNodeOf"/>
                <owl:someValuesFrom rdf:resource="https://w3id.org/def/vaeontology#ValueTaxonomyStatement"/>
            </owl:Restriction>
        </rdfs:subClassOf>
        <rdfs:subClassOf>
            <owl:Restriction>
                <owl:onProperty rdf:resource="https://w3id.org/def/vaeontology#hasImportance"/>
                <owl:qualifiedCardinality rdf:datatype="http://www.w3.org/2001/XMLSchema#nonNegativeInteger">1</owl:qualifiedCardinality>
                <owl:onClass rdf:resource="https://w3id.org/def/vaeontology#NodeImportance"/>
            </owl:Restriction>
        </rdfs:subClassOf>
        <owl:disjointWith rdf:resource="https://w3id.org/def/vaeontology#PropertyNode"/>
        <rdfs:comment>[Nardine Osman, Mark D’Inverno https://arxiv.org/abs/2305.02748]</rdfs:comment>
        <rdfs:label>Concept Node</rdfs:label>
        <bhv:bibRef>Osman, N., d’Inverno, M.: A computational framework of human values for ethical
ai (2023)</bhv:bibRef>
    </owl:Class>
    


    <!-- https://w3id.org/def/vaeontology#Conformance -->

    <owl:Class rdf:about="https://w3id.org/def/vaeontology#Conformance">
        <rdfs:subClassOf rdf:resource="https://w3id.org/spice/SON/SchwartzValues#Conformity"/>
        <rdfs:comment>Conformance: correspondence in form or appearance</rdfs:comment>
        <rdfs:comment>Term added automatically</rdfs:comment>
        <rdfs:label>Conformance</rdfs:label>
    </owl:Class>
    


    <!-- https://w3id.org/def/vaeontology#Conformation -->

    <owl:Class rdf:about="https://w3id.org/def/vaeontology#Conformation">
        <rdfs:subClassOf rdf:resource="https://w3id.org/spice/SON/SchwartzValues#Conformity"/>
        <rdfs:comment>Conformation: acting according to certain accepted standards</rdfs:comment>
        <rdfs:comment>Term added automatically</rdfs:comment>
        <rdfs:label>Conformation</rdfs:label>
    </owl:Class>
    


    <!-- https://w3id.org/def/vaeontology#Conformism -->

    <owl:Class rdf:about="https://w3id.org/def/vaeontology#Conformism">
        <rdfs:subClassOf rdf:resource="https://w3id.org/spice/SON/SchwartzValues#Conformity"/>
        <rdfs:comment>Conformism: orthodoxy in thoughts and belief</rdfs:comment>
        <rdfs:comment>Term added automatically</rdfs:comment>
        <rdfs:label>Conformism</rdfs:label>
    </owl:Class>
    


    <!-- https://w3id.org/def/vaeontology#Context -->

    <owl:Class rdf:about="https://w3id.org/def/vaeontology#Context">
        <rdfs:subClassOf rdf:resource="http://www.ontologydesignpatterns.org/ont/dul/DUL.owl#Situation"/>
        <rdfs:comment>A Context is any kind of entity that is underlying of specific events, situations, descriptions and agents. They can be used to describe, for example, the kind of problem or world where a system is deployed, contextualization of statements, etc.</rdfs:comment>
        <rdfs:label>Context</rdfs:label>
        <rdfs:seeAlso rdf:resource="https://w3id.org/def/vaeontology#VaeObject"/>
        <bhv:bibRef>Osman, N., d’Inverno, M.: A computational framework of human values for ethical
ai (2023)</bhv:bibRef>
        <bhv:bibRef>https://arxiv.org/abs/2305.02748</bhv:bibRef>
    </owl:Class>
    


    <!-- https://w3id.org/def/vaeontology#Criterion -->

    <owl:Class rdf:about="https://w3id.org/def/vaeontology#Criterion">
        <rdfs:subClassOf rdf:resource="http://www.ontologydesignpatterns.org/ont/dul/DUL.owl#Theory"/>
        <rdfs:subClassOf rdf:resource="http://www.w3.org/ns/odrl/2/Policy"/>
        <rdfs:subClassOf rdf:resource="https://w3id.org/def/vaeontology#AgentStatement"/>
        <rdfs:subClassOf>
            <owl:Class>
                <owl:unionOf rdf:parseType="Collection">
                    <owl:Restriction>
                        <owl:onProperty rdf:resource="http://www.w3.org/ns/odrl/2/action"/>
                        <owl:someValuesFrom>
                            <owl:Class>
                                <owl:intersectionOf rdf:parseType="Collection">
                                    <rdf:Description rdf:about="https://w3id.org/def/vaeontology#VaeStatement"/>
                                    <owl:Restriction>
                                        <owl:onProperty rdf:resource="https://w3id.org/def/vaeontology#withNorm"/>
                                        <owl:someValuesFrom rdf:resource="https://w3id.org/def/vaeontology#Norm"/>
                                    </owl:Restriction>
                                </owl:intersectionOf>
                            </owl:Class>
                        </owl:someValuesFrom>
                    </owl:Restriction>
                    <owl:Restriction>
                        <owl:onProperty rdf:resource="http://www.w3.org/ns/odrl/2/action"/>
                        <owl:someValuesFrom>
                            <owl:Class>
                                <owl:intersectionOf rdf:parseType="Collection">
                                    <rdf:Description rdf:about="https://w3id.org/def/vaeontology#VaeStatement"/>
                                    <owl:Restriction>
                                        <owl:onProperty rdf:resource="https://w3id.org/def/vaeontology#withValue"/>
                                        <owl:someValuesFrom rdf:resource="https://w3id.org/def/vaeontology#ValueConcept"/>
                                    </owl:Restriction>
                                </owl:intersectionOf>
                            </owl:Class>
                        </owl:someValuesFrom>
                    </owl:Restriction>
                </owl:unionOf>
            </owl:Class>
        </rdfs:subClassOf>
        <rdfs:subClassOf>
            <owl:Restriction>
                <owl:onProperty rdf:resource="http://www.w3.org/ns/odrl/2/action"/>
                <owl:someValuesFrom rdf:resource="https://w3id.org/def/vaeontology#VaeStatement"/>
            </owl:Restriction>
        </rdfs:subClassOf>
        <rdfs:subClassOf>
            <owl:Restriction>
                <owl:onProperty rdf:resource="http://www.w3.org/ns/odrl/2/assignee"/>
                <owl:someValuesFrom rdf:resource="https://w3id.org/def/vaeontology#Agent"/>
            </owl:Restriction>
        </rdfs:subClassOf>
        <rdfs:subClassOf>
            <owl:Restriction>
                <owl:onProperty rdf:resource="http://www.w3.org/ns/odrl/2/assigner"/>
                <owl:someValuesFrom rdf:resource="https://w3id.org/def/vaeontology#User"/>
            </owl:Restriction>
        </rdfs:subClassOf>
        <rdfs:subClassOf>
            <owl:Restriction>
                <owl:onProperty rdf:resource="https://w3id.org/def/vaeontology#interpretationOn"/>
                <owl:someValuesFrom rdf:resource="https://w3id.org/def/vaeontology#VaeConditioningEntity"/>
            </owl:Restriction>
        </rdfs:subClassOf>
        <rdfs:subClassOf>
            <owl:Restriction>
                <owl:onProperty rdf:resource="http://www.w3.org/ns/odrl/2/constraint"/>
                <owl:allValuesFrom rdf:resource="http://www.w3.org/ns/odrl/2/Constraint"/>
            </owl:Restriction>
        </rdfs:subClassOf>
        <rdfs:subClassOf>
            <owl:Restriction>
                <owl:onProperty rdf:resource="http://www.w3.org/ns/odrl/2/target"/>
                <owl:allValuesFrom rdf:resource="http://www.w3.org/ns/odrl/2/Asset"/>
            </owl:Restriction>
        </rdfs:subClassOf>
        <rdfs:comment>In ArgumentStatements, the fact that specific claims can follow from some premises must be based on some Criterion (this class) proposed by an authority (i.e. the system designer or the researcher) or evolved by the society in some way. 

Criteria link premises and claims and provide constraints for the premises to be true, for the claim to follow from the premises, from the context, etc.</rdfs:comment>
        <rdfs:label>Criterion</rdfs:label>
        <skos:note>[Luc Steels: https://vale2023.iiia.csic.es/accepted-papers]  “One of the big advantages of explicit representations is that outcomes can be explained by the system itself in terms of norms and values. For example, a user can ask why he is blocked on a social media platform and this is then explained in terms of which community rules he broke and possibly what values these rules reflect (i.e. why the norm was adopted)”. 

Criteria are those conditions that identify value-aligned or missaligned behaviour with values or norms in mind.</skos:note>
    </owl:Class>
    


    <!-- https://w3id.org/def/vaeontology#Custom -->

    <owl:Class rdf:about="https://w3id.org/def/vaeontology#Custom">
        <rdfs:subClassOf rdf:resource="https://w3id.org/spice/SON/SchwartzValues#Tradition"/>
        <rdfs:comment>Custom: a specific practice of long standing</rdfs:comment>
        <rdfs:comment>Term added automatically</rdfs:comment>
        <rdfs:label>Custom</rdfs:label>
    </owl:Class>
    


    <!-- https://w3id.org/def/vaeontology#Dependableness -->

    <owl:Class rdf:about="https://w3id.org/def/vaeontology#Dependableness">
        <rdfs:subClassOf rdf:resource="https://w3id.org/spice/SON/SchwartzValues#Dependability"/>
        <rdfs:comment>Dependableness: the quality of being dependable or reliable</rdfs:comment>
        <rdfs:comment>Term added automatically</rdfs:comment>
        <rdfs:label>Dependableness</rdfs:label>
    </owl:Class>
    


    <!-- https://w3id.org/def/vaeontology#Economic_value -->

    <owl:Class rdf:about="https://w3id.org/def/vaeontology#Economic_value">
        <rdfs:subClassOf rdf:resource="https://w3id.org/spice/SON/SchwartzValues#Value"/>
        <rdfs:comment>Economic_value: the amount (of money or goods or services) that is considered to be a fair equivalent for something else</rdfs:comment>
        <rdfs:comment>Term added automatically</rdfs:comment>
        <rdfs:label>Economic_value</rdfs:label>
    </owl:Class>
    


    <!-- https://w3id.org/def/vaeontology#Equality -->

    <owl:Class rdf:about="https://w3id.org/def/vaeontology#Equality">
        <rdfs:subClassOf rdf:resource="https://w3id.org/spice/SON/SchwartzValues#SelfTrascendence"/>
        <rdfs:comment>Equality is present in most of the VAE papers so far, as it is easy to formalize mathematically.</rdfs:comment>
        <rdfs:label>Equality</rdfs:label>
    </owl:Class>
    


    <!-- https://w3id.org/def/vaeontology#FinalInputOutcome -->

    <owl:Class rdf:about="https://w3id.org/def/vaeontology#FinalInputOutcome">
        <rdfs:subClassOf rdf:resource="https://w3id.org/def/vaeontology#MultiInputOutcome"/>
        <rdfs:subClassOf>
            <owl:Class>
                <owl:complementOf>
                    <owl:Restriction>
                        <owl:onProperty rdf:resource="https://w3id.org/def/vaeontology#nextInputOutcome"/>
                        <owl:someValuesFrom rdf:resource="https://w3id.org/def/vaeontology#MultiInputOutcome"/>
                    </owl:Restriction>
                </owl:complementOf>
            </owl:Class>
        </rdfs:subClassOf>
        <rdfs:comment>The final relation between inputs and outcomes of a Sequence.</rdfs:comment>
        <rdfs:label>Final Input Outcome</rdfs:label>
        <rdfs:seeAlso rdf:resource="https://w3id.org/def/vaeontology#Sequence"/>
        <rdfs:seeAlso>http://ontologydesignpatterns.org/wiki/Submissions:Sequence</rdfs:seeAlso>
    </owl:Class>
    


    <!-- https://w3id.org/def/vaeontology#Force -->

    <owl:Class rdf:about="https://w3id.org/def/vaeontology#Force">
        <rdfs:subClassOf rdf:resource="https://w3id.org/spice/SON/SchwartzValues#Power"/>
        <rdfs:comment>Force: one possessing or exercising power or influence or authority</rdfs:comment>
        <rdfs:comment>Term added automatically</rdfs:comment>
        <rdfs:label>Force</rdfs:label>
    </owl:Class>
    


    <!-- https://w3id.org/def/vaeontology#Generalization -->

    <owl:Class rdf:about="https://w3id.org/def/vaeontology#Generalization">
        <rdfs:subClassOf rdf:resource="https://w3id.org/def/vaeontology#ValueComparisonStatement"/>
        <owl:disjointWith rdf:resource="https://w3id.org/def/vaeontology#ImportanceRelation"/>
        <rdfs:comment>A comparison statement proposed by an Agent in which believes that some ValueConcept (superior) generalizes another one (inferior).</rdfs:comment>
        <rdfs:label>Generalization</rdfs:label>
        <rdfs:seeAlso rdf:resource="https://w3id.org/def/vaeontology#generalizesNode"/>
    </owl:Class>
    


    <!-- https://w3id.org/def/vaeontology#GiniIndex -->

    <owl:Class rdf:about="https://w3id.org/def/vaeontology#GiniIndex">
        <rdfs:subClassOf rdf:resource="https://w3id.org/def/vaeontology#SemanticsFunction"/>
        <rdfs:comment>The Gini Index can be used as a Semantics Function in State, as in the taxing problem from Montes and Sierra (see reference).</rdfs:comment>
        <rdfs:label>Gini Index</rdfs:label>
        <bhv:bibRef>Montes, N., Sierra, C.: Synthesis and properties of optimally value-aligned nor-
mative systems. Journal of Artificial Intelligence Research 74, 1739–1774 (2022).
https://doi.org/10.1613/jair.1.13487</bhv:bibRef>
    </owl:Class>
    


    <!-- https://w3id.org/def/vaeontology#Humbleness -->

    <owl:Class rdf:about="https://w3id.org/def/vaeontology#Humbleness">
        <rdfs:subClassOf rdf:resource="https://w3id.org/spice/SON/SchwartzValues#Humility"/>
        <rdfs:comment>Humbleness: a disposition to be humble; a lack of false pride</rdfs:comment>
        <rdfs:comment>Term added automatically</rdfs:comment>
        <rdfs:label>Humbleness</rdfs:label>
    </owl:Class>
    


    <!-- https://w3id.org/def/vaeontology#Imagination -->

    <owl:Class rdf:about="https://w3id.org/def/vaeontology#Imagination">
        <rdfs:subClassOf rdf:resource="https://w3id.org/spice/SON/SchwartzValues#Resources"/>
        <rdfs:comment>Imagination: the ability to deal resourcefully with unusual problems</rdfs:comment>
        <rdfs:comment>Term added automatically</rdfs:comment>
        <rdfs:label>Imagination</rdfs:label>
    </owl:Class>
    


    <!-- https://w3id.org/def/vaeontology#ImportanceRelation -->

    <owl:Class rdf:about="https://w3id.org/def/vaeontology#ImportanceRelation">
        <rdfs:subClassOf rdf:resource="https://w3id.org/def/vaeontology#ValueComparisonStatement"/>
        <rdfs:comment>&quot;Another important concept considered core in the social sciences is value priority, or how important a value is for someone.&quot;  [Nardine Osman, Mark D’Inverno https://arxiv.org/abs/2305.02748]</rdfs:comment>
        <rdfs:comment>A comparison statement proposed by an Agent in which believes that some ValueConcept (superior) is more important than another one (inferior).</rdfs:comment>
        <rdfs:label>Importance Relation</rdfs:label>
        <rdfs:seeAlso>http://hdl.handle.net/10261/197622</rdfs:seeAlso>
        <bhv:bibRef>Value Systems as a ranking between values: [Serramia et al. https://aamas.csc.liv.ac.uk/Proceedings/aamas2018/pdfs/p1294.pdf]</bhv:bibRef>
    </owl:Class>
    


    <!-- https://w3id.org/def/vaeontology#Leeway -->

    <owl:Class rdf:about="https://w3id.org/def/vaeontology#Leeway">
        <rdfs:subClassOf rdf:resource="https://w3id.org/spice/SON/SchwartzValues#Tolerance"/>
        <rdfs:comment>Leeway: a permissible difference; allowing some freedom to move within limits</rdfs:comment>
        <rdfs:comment>Term added automatically</rdfs:comment>
        <rdfs:label>Leeway</rdfs:label>
    </owl:Class>
    


    <!-- https://w3id.org/def/vaeontology#Margin -->

    <owl:Class rdf:about="https://w3id.org/def/vaeontology#Margin">
        <rdfs:subClassOf rdf:resource="https://w3id.org/spice/SON/SchwartzValues#Tolerance"/>
        <rdfs:comment>Margin: a permissible difference; allowing some freedom to move within limits</rdfs:comment>
        <rdfs:comment>Term added automatically</rdfs:comment>
        <rdfs:label>Margin</rdfs:label>
    </owl:Class>
    


    <!-- https://w3id.org/def/vaeontology#MultiInputOutcome -->

    <owl:Class rdf:about="https://w3id.org/def/vaeontology#MultiInputOutcome">
        <rdfs:subClassOf rdf:resource="https://w3id.org/def/vaeontology#Outcome"/>
        <rdfs:subClassOf>
            <owl:Restriction>
                <owl:onProperty rdf:resource="https://w3id.org/def/vaeontology#isStartOfSequence"/>
                <owl:someValuesFrom rdf:resource="https://w3id.org/def/vaeontology#Sequence"/>
            </owl:Restriction>
        </rdfs:subClassOf>
        <rdfs:comment>A relationship between a series of input dul:Events and a series of Outcomes that follow those. MultiInputOutcomes are the basic blocks to build Sequences, they follow the Sequence ODP.</rdfs:comment>
        <rdfs:label>Multi Input Outcome</rdfs:label>
        <rdfs:seeAlso rdf:resource="https://w3id.org/def/vaeontology#Sequence"/>
        <rdfs:seeAlso>http://ontologydesignpatterns.org/wiki/Submissions:Sequence</rdfs:seeAlso>
    </owl:Class>
    


    <!-- https://w3id.org/def/vaeontology#NodeImportance -->

    <owl:Class rdf:about="https://w3id.org/def/vaeontology#NodeImportance">
        <rdfs:subClassOf rdf:resource="https://w3id.org/def/vaeontology#QuantitativeVaeProperty"/>
        <rdfs:subClassOf rdf:resource="https://w3id.org/def/vaeontology#ValueProperty"/>
        <rdfs:subClassOf>
            <owl:Restriction>
                <owl:onProperty rdf:resource="https://w3id.org/def/vaeontology#isImportanceOf"/>
                <owl:someValuesFrom>
                    <owl:Class>
                        <owl:unionOf rdf:parseType="Collection">
                            <rdf:Description rdf:about="https://w3id.org/def/vaeontology#ConceptNode"/>
                            <rdf:Description rdf:about="https://w3id.org/def/vaeontology#PropertyNode"/>
                        </owl:unionOf>
                    </owl:Class>
                </owl:someValuesFrom>
            </owl:Restriction>
        </rdfs:subClassOf>
        <rdfs:comment>&quot;Another important concept considered core in the social sciences is value priority, or how important a value is for someone. We incorporate this concept by attaching a mea- sure of importance to each node of the taxonomy.&quot;  [Nardine Osman, Mark D’Inverno https://arxiv.org/abs/2305.02748]</rdfs:comment>
        <rdfs:label>Node Importance</rdfs:label>
        <rdfs:seeAlso rdf:resource="https://w3id.org/def/vaeontology#ImportanceRelation"/>
        <rdfs:seeAlso rdf:resource="https://w3id.org/def/vaeontology#ValueTaxonomy"/>
    </owl:Class>
    


    <!-- https://w3id.org/def/vaeontology#Norm -->

    <owl:Class rdf:about="https://w3id.org/def/vaeontology#Norm">
        <rdfs:subClassOf rdf:resource="http://www.ontologydesignpatterns.org/ont/dul/DUL.owl#Norm"/>
        <rdfs:subClassOf rdf:resource="http://www.w3.org/ns/odrl/2/Policy"/>
        <rdfs:subClassOf rdf:resource="https://w3id.org/def/vaeontology#VaeConditionedEntity"/>
        <rdfs:subClassOf rdf:resource="https://w3id.org/def/vaeontology#VaeConditioningEntity"/>
        <rdfs:subClassOf>
            <owl:Restriction>
                <owl:onProperty rdf:resource="http://www.w3.org/ns/odrl/2/action"/>
                <owl:someValuesFrom rdf:resource="https://w3id.org/def/vaeontology#Outcome"/>
            </owl:Restriction>
        </rdfs:subClassOf>
        <rdfs:subClassOf>
            <owl:Restriction>
                <owl:onProperty rdf:resource="http://www.w3.org/ns/odrl/2/assignee"/>
                <owl:someValuesFrom rdf:resource="https://w3id.org/def/vaeontology#Agent"/>
            </owl:Restriction>
        </rdfs:subClassOf>
        <rdfs:subClassOf>
            <owl:Restriction>
                <owl:onProperty rdf:resource="http://www.w3.org/ns/odrl/2/assigner"/>
                <owl:someValuesFrom rdf:resource="https://w3id.org/def/vaeontology#User"/>
            </owl:Restriction>
        </rdfs:subClassOf>
        <rdfs:subClassOf>
            <owl:Restriction>
                <owl:onProperty rdf:resource="http://www.w3.org/ns/odrl/2/target"/>
                <owl:someValuesFrom rdf:resource="https://w3id.org/def/vaeontology#System"/>
            </owl:Restriction>
        </rdfs:subClassOf>
        <rdfs:subClassOf>
            <owl:Restriction>
                <owl:onProperty rdf:resource="https://w3id.org/def/vaeontology#influencesOutcome"/>
                <owl:someValuesFrom rdf:resource="https://w3id.org/def/vaeontology#Outcome"/>
            </owl:Restriction>
        </rdfs:subClassOf>
        <rdfs:subClassOf>
            <owl:Restriction>
                <owl:onProperty rdf:resource="https://w3id.org/def/vaeontology#reflectsValue"/>
                <owl:someValuesFrom rdf:resource="https://w3id.org/def/vaeontology#ValueConcept"/>
            </owl:Restriction>
        </rdfs:subClassOf>
        <rdfs:subClassOf>
            <owl:Restriction>
                <owl:onProperty rdf:resource="http://www.w3.org/ns/odrl/2/constraint"/>
                <owl:allValuesFrom rdf:resource="http://www.w3.org/ns/odrl/2/Constraint"/>
            </owl:Restriction>
        </rdfs:subClassOf>
        <owl:disjointWith rdf:resource="https://w3id.org/def/vaeontology#ValueTaxonomyStatement"/>
        <rdfs:comment>&quot;Norms (...) establish boundaries, either soft or hard, on individual autonomy through a variety of mechanisms such as social pressure and expectations, constraints on actions, and sanctions for violation or rewards for compliance.&quot;</rdfs:comment>
        <rdfs:comment>[Luc Steels: https://vale2023.iiia.csic.es/accepted-papers] &quot;Explicit representations of norms are often called policies.&quot;</rdfs:comment>
        <rdfs:label>Norm</rdfs:label>
        <bhv:bibRef>Nieves Montes, Nardine Osman, and Carles Sierra, ‘Perspective-dependent value alignment of norms’ VALE workshop, ECAI 2023</bhv:bibRef>
    </owl:Class>
    


    <!-- https://w3id.org/def/vaeontology#OptimizedProperty -->

    <owl:Class rdf:about="https://w3id.org/def/vaeontology#OptimizedProperty">
        <owl:equivalentClass>
            <owl:Restriction>
                <owl:onProperty rdf:resource="https://w3id.org/def/vaeontology#isOptimizationOfProperty"/>
                <owl:someValuesFrom rdf:resource="https://w3id.org/def/vaeontology#VaeProperty"/>
            </owl:Restriction>
        </owl:equivalentClass>
        <rdfs:subClassOf rdf:resource="https://w3id.org/def/vaeontology#BooleanVaeProperty"/>
        <rdfs:subClassOf rdf:resource="https://w3id.org/def/vaeontology#QuantitativeVaeProperty"/>
        <rdfs:comment>Assertion that a property has being optimized over a set of possible outcomes, supplying the value achieved (e.g. an optimal (maximum) vae:GiniIndex value of 0.9 is vae:measuredOnOutcome vae:State, over some other possible states -the optimization domain could be represented somewhere else or with a custom property-).</rdfs:comment>
        <rdfs:label>Optimized Property</rdfs:label>
    </owl:Class>
    


    <!-- https://w3id.org/def/vaeontology#Ossification -->

    <owl:Class rdf:about="https://w3id.org/def/vaeontology#Ossification">
        <rdfs:subClassOf rdf:resource="https://w3id.org/spice/SON/SchwartzValues#Conformity"/>
        <rdfs:comment>Ossification: hardened conventionality</rdfs:comment>
        <rdfs:comment>Term added automatically</rdfs:comment>
        <rdfs:label>Ossification</rdfs:label>
    </owl:Class>
    


    <!-- https://w3id.org/def/vaeontology#Outcome -->

    <owl:Class rdf:about="https://w3id.org/def/vaeontology#Outcome">
        <rdfs:subClassOf rdf:resource="http://www.ontologydesignpatterns.org/ont/dul/DUL.owl#Event"/>
        <rdfs:subClassOf rdf:resource="https://w3id.org/def/vaeontology#VaeConditionedEntity"/>
        <rdfs:subClassOf>
            <owl:Restriction>
                <owl:onProperty rdf:resource="https://w3id.org/def/vaeontology#abidesByValue"/>
                <owl:allValuesFrom rdf:resource="https://w3id.org/def/vaeontology#ValueConcept"/>
            </owl:Restriction>
        </rdfs:subClassOf>
        <rdfs:subClassOf>
            <owl:Restriction>
                <owl:onProperty rdf:resource="https://w3id.org/def/vaeontology#satisfiesNorm"/>
                <owl:allValuesFrom rdf:resource="https://w3id.org/def/vaeontology#Norm"/>
            </owl:Restriction>
        </rdfs:subClassOf>
        <rdfs:subClassOf>
            <owl:Restriction>
                <owl:onProperty rdf:resource="https://w3id.org/def/vaeontology#satisfiesProperty"/>
                <owl:allValuesFrom rdf:resource="https://w3id.org/def/vaeontology#VaeProperty"/>
            </owl:Restriction>
        </rdfs:subClassOf>
        <rdfs:subClassOf>
            <owl:Restriction>
                <owl:onProperty rdf:resource="https://w3id.org/def/vaeontology#composedBySequence"/>
                <owl:maxQualifiedCardinality rdf:datatype="http://www.w3.org/2001/XMLSchema#nonNegativeInteger">1</owl:maxQualifiedCardinality>
                <owl:onClass rdf:resource="https://w3id.org/def/vaeontology#Sequence"/>
            </owl:Restriction>
        </rdfs:subClassOf>
        <rdfs:comment>Outcomes include the effect of the behavior of a system or of a user using a system [Luc Steels: https://vale2023.iiia.csic.es/accepted-papers].</rdfs:comment>
        <rdfs:label>Outcome</rdfs:label>
    </owl:Class>
    


    <!-- https://w3id.org/def/vaeontology#Permissiveness -->

    <owl:Class rdf:about="https://w3id.org/def/vaeontology#Permissiveness">
        <rdfs:subClassOf rdf:resource="https://w3id.org/spice/SON/SchwartzValues#Tolerance"/>
        <rdfs:comment>Permissiveness: a disposition to allow freedom of choice and behavior</rdfs:comment>
        <rdfs:comment>Term added automatically</rdfs:comment>
        <rdfs:label>Permissiveness</rdfs:label>
    </owl:Class>
    


    <!-- https://w3id.org/def/vaeontology#Prise -->

    <owl:Class rdf:about="https://w3id.org/def/vaeontology#Prise">
        <rdfs:subClassOf rdf:resource="https://w3id.org/spice/SON/SchwartzValues#Value"/>
        <rdfs:comment>Prise: regard highly; think much of</rdfs:comment>
        <rdfs:comment>Term added automatically</rdfs:comment>
        <rdfs:label>Prise</rdfs:label>
    </owl:Class>
    


    <!-- https://w3id.org/def/vaeontology#Prize -->

    <owl:Class rdf:about="https://w3id.org/def/vaeontology#Prize">
        <rdfs:subClassOf rdf:resource="https://w3id.org/spice/SON/SchwartzValues#Value"/>
        <rdfs:comment>Prize: hold dear</rdfs:comment>
        <rdfs:comment>Term added automatically</rdfs:comment>
        <rdfs:label>Prize</rdfs:label>
    </owl:Class>
    


    <!-- https://w3id.org/def/vaeontology#PromotionDemotion -->

    <owl:Class rdf:about="https://w3id.org/def/vaeontology#PromotionDemotion">
        <rdfs:subClassOf rdf:resource="https://w3id.org/def/vaeontology#QualitativeVaeProperty"/>
        <rdfs:subClassOf rdf:resource="https://w3id.org/def/vaeontology#ValueProperty"/>
        <rdfs:comment>A QualitativeVaeProperty and a ValueProperty that can represent Promotion, Demotion or Neutrality of an Outcome towards some Value.</rdfs:comment>
        <rdfs:label>Promotion Demotion</rdfs:label>
    </owl:Class>
    


    <!-- https://w3id.org/def/vaeontology#PropertyNode -->

    <owl:Class rdf:about="https://w3id.org/def/vaeontology#PropertyNode">
        <rdfs:subClassOf rdf:resource="https://w3id.org/def/vaeontology#VaePropertyStatement"/>
        <rdfs:subClassOf>
            <owl:Restriction>
                <owl:onProperty rdf:resource="https://w3id.org/def/vaeontology#hasPropertyTaxonomy"/>
                <owl:someValuesFrom rdf:resource="https://w3id.org/def/vaeontology#TaxonomyProperty"/>
            </owl:Restriction>
        </rdfs:subClassOf>
        <rdfs:subClassOf>
            <owl:Restriction>
                <owl:onProperty rdf:resource="https://w3id.org/def/vaeontology#isPropertyNodeOf"/>
                <owl:someValuesFrom rdf:resource="https://w3id.org/def/vaeontology#ValueTaxonomyStatement"/>
            </owl:Restriction>
        </rdfs:subClassOf>
        <rdfs:subClassOf>
            <owl:Restriction>
                <owl:onProperty rdf:resource="https://w3id.org/def/vaeontology#hasImportance"/>
                <owl:qualifiedCardinality rdf:datatype="http://www.w3.org/2001/XMLSchema#nonNegativeInteger">1</owl:qualifiedCardinality>
                <owl:onClass rdf:resource="https://w3id.org/def/vaeontology#NodeImportance"/>
            </owl:Restriction>
        </rdfs:subClassOf>
        <rdfs:comment>[Nardine Osman, Mark D’Inverno https://arxiv.org/abs/2305.02748]</rdfs:comment>
        <rdfs:label>Property Node</rdfs:label>
        <bhv:bibRef>Osman, N., d’Inverno, M.: A computational framework of human values for ethical
ai (2023)</bhv:bibRef>
    </owl:Class>
    


    <!-- https://w3id.org/def/vaeontology#QualitativeVaeProperty -->

    <owl:Class rdf:about="https://w3id.org/def/vaeontology#QualitativeVaeProperty">
        <rdfs:subClassOf rdf:resource="https://w3id.org/def/vaeontology#VaeProperty"/>
        <rdfs:comment>A VaeProperty that represent a qualitative consideration on an Outcome with respect to a Value or Norm.</rdfs:comment>
        <rdfs:label>Qualitative Vae Property</rdfs:label>
    </owl:Class>
    


    <!-- https://w3id.org/def/vaeontology#QuantitativePromotionDemotion -->

    <owl:Class rdf:about="https://w3id.org/def/vaeontology#QuantitativePromotionDemotion">
        <rdfs:subClassOf rdf:resource="https://w3id.org/def/vaeontology#PromotionDemotion"/>
        <rdfs:subClassOf rdf:resource="https://w3id.org/def/vaeontology#QuantitativeVaeProperty"/>
        <rdfs:comment>A quantitative version of PromotionDemotion that specifies some degre of Promotion/Demotion/Neutrality.</rdfs:comment>
        <rdfs:label>Quantitative Promotion Demotion</rdfs:label>
    </owl:Class>
    


    <!-- https://w3id.org/def/vaeontology#QuantitativeVaeProperty -->

    <owl:Class rdf:about="https://w3id.org/def/vaeontology#QuantitativeVaeProperty">
        <rdfs:subClassOf rdf:resource="https://w3id.org/def/vaeontology#VaeProperty"/>
        <rdfs:subClassOf>
            <owl:Restriction>
                <owl:onProperty rdf:resource="http://www.w3.org/1999/02/22-rdf-syntax-ns#value"/>
                <owl:someValuesFrom rdf:resource="http://www.w3.org/2002/07/owl#real"/>
            </owl:Restriction>
        </rdfs:subClassOf>
        <rdfs:comment>A VaeProperty that is represented by some numeric value.</rdfs:comment>
        <rdfs:label>Quantitative Vae Property</rdfs:label>
    </owl:Class>
    


    <!-- https://w3id.org/def/vaeontology#Reliability -->

    <owl:Class rdf:about="https://w3id.org/def/vaeontology#Reliability">
        <rdfs:subClassOf rdf:resource="https://w3id.org/spice/SON/SchwartzValues#Dependability"/>
        <rdfs:comment>Reliability: the quality of being dependable or reliable</rdfs:comment>
        <rdfs:comment>Term added automatically</rdfs:comment>
        <rdfs:label>Reliability</rdfs:label>
    </owl:Class>
    


    <!-- https://w3id.org/def/vaeontology#Reliableness -->

    <owl:Class rdf:about="https://w3id.org/def/vaeontology#Reliableness">
        <rdfs:subClassOf rdf:resource="https://w3id.org/spice/SON/SchwartzValues#Dependability"/>
        <rdfs:comment>Reliableness: the quality of being dependable or reliable</rdfs:comment>
        <rdfs:comment>Term added automatically</rdfs:comment>
        <rdfs:label>Reliableness</rdfs:label>
    </owl:Class>
    


    <!-- https://w3id.org/def/vaeontology#Resourcefulness -->

    <owl:Class rdf:about="https://w3id.org/def/vaeontology#Resourcefulness">
        <rdfs:subClassOf rdf:resource="https://w3id.org/spice/SON/SchwartzValues#Resources"/>
        <rdfs:comment>Resourcefulness: the ability to deal resourcefully with unusual problems</rdfs:comment>
        <rdfs:comment>Term added automatically</rdfs:comment>
        <rdfs:label>Resourcefulness</rdfs:label>
    </owl:Class>
    


    <!-- https://w3id.org/def/vaeontology#SemanticsFunction -->

    <owl:Class rdf:about="https://w3id.org/def/vaeontology#SemanticsFunction">
        <rdfs:subClassOf rdf:resource="https://w3id.org/def/vaeontology#QuantitativeVaeProperty"/>
        <rdfs:subClassOf rdf:resource="https://w3id.org/def/vaeontology#ValueProperty"/>
        <rdfs:comment>&quot;To express the relationship between an abstract value and the meaning it takes in a particular context, we say that an explicit goal g grounds the semantics of value v in context C&quot; [Nieves Montes, Carles Sierra et al. https://www.jair.org/index.php/jair/article/view/13487]</rdfs:comment>
        <rdfs:label>Semantics Function</rdfs:label>
        <bhv:bibRef>Montes, N., Sierra, C.: Synthesis and properties of optimally value-aligned nor-
mative systems. Journal of Artificial Intelligence Research 74, 1739–1774 (2022).
https://doi.org/10.1613/jair.1.13487</bhv:bibRef>
    </owl:Class>
    


    <!-- https://w3id.org/def/vaeontology#Sequence -->

    <owl:Class rdf:about="https://w3id.org/def/vaeontology#Sequence">
        <rdfs:subClassOf rdf:resource="http://www.ontologydesignpatterns.org/ont/dul/DUL.owl#Process"/>
        <rdfs:subClassOf rdf:resource="https://w3id.org/def/vaeontology#Outcome"/>
        <rdfs:subClassOf>
            <owl:Restriction>
                <owl:onProperty rdf:resource="https://w3id.org/def/vaeontology#startsWithInputOutcome"/>
                <owl:qualifiedCardinality rdf:datatype="http://www.w3.org/2001/XMLSchema#nonNegativeInteger">1</owl:qualifiedCardinality>
                <owl:onClass rdf:resource="https://w3id.org/def/vaeontology#MultiInputOutcome"/>
            </owl:Restriction>
        </rdfs:subClassOf>
        <rdfs:comment>A Sequence of Outcomes. In general, allows representing sequences of input dul:Events and their related Outcomes (e.g. series of states -&gt; actions, newstates -&gt; actions, etc). It follows the Sequence ODP.</rdfs:comment>
        <rdfs:label>Sequence</rdfs:label>
        <rdfs:seeAlso>http://ontologydesignpatterns.org/wiki/Submissions:Sequence</rdfs:seeAlso>
    </owl:Class>
    


    <!-- https://w3id.org/def/vaeontology#SoundArgument -->

    <owl:Class rdf:about="https://w3id.org/def/vaeontology#SoundArgument">
        <rdfs:subClassOf rdf:resource="http://www.w3.org/ns/odrl/2/Operator"/>
        <rdfs:comment>Any operator used in a Constraint for a Criterion, between premises and claims contrasting if the argument is sound.</rdfs:comment>
        <rdfs:label>Sound Argument</rdfs:label>
    </owl:Class>
    


    <!-- https://w3id.org/def/vaeontology#State -->

    <owl:Class rdf:about="https://w3id.org/def/vaeontology#State">
        <rdfs:subClassOf rdf:resource="https://w3id.org/def/vaeontology#Outcome"/>
        <rdfs:comment>A representation of the State of an Agent.</rdfs:comment>
        <rdfs:label>State</rdfs:label>
    </owl:Class>
    


    <!-- https://w3id.org/def/vaeontology#Strategy -->

    <owl:Class rdf:about="https://w3id.org/def/vaeontology#Strategy">
        <rdfs:subClassOf rdf:resource="https://w3id.org/def/vaeontology#Outcome"/>
        <rdfs:comment>A mapping between States and Actions that an ActingAgent follows and regulate its behaviour in the world.</rdfs:comment>
        <rdfs:label>Strategy</rdfs:label>
    </owl:Class>
    


    <!-- https://w3id.org/def/vaeontology#System -->

    <owl:Class rdf:about="https://w3id.org/def/vaeontology#System">
        <rdfs:subClassOf rdf:resource="http://www.ontologydesignpatterns.org/ont/dul/DUL.owl#Collection"/>
        <rdfs:subClassOf rdf:resource="https://w3id.org/def/vaeontology#Agent"/>
        <rdfs:subClassOf>
            <owl:Restriction>
                <owl:onProperty rdf:resource="https://w3id.org/def/vaeontology#hasTrace"/>
                <owl:maxQualifiedCardinality rdf:datatype="http://www.w3.org/2001/XMLSchema#nonNegativeInteger">1</owl:maxQualifiedCardinality>
                <owl:onClass rdf:resource="https://w3id.org/def/vaeontology#Sequence"/>
            </owl:Restriction>
        </rdfs:subClassOf>
        <owl:disjointWith rdf:resource="https://w3id.org/def/vaeontology#User"/>
        <rdfs:comment>A system is the organization of a set of Agents modelling some complex joint behaviour or for solving a task. A system has a trace, a Sequence of the inputs and the corresponding Outcomes performed (e.g.) by the system or the agents on it.</rdfs:comment>
        <rdfs:label>System</rdfs:label>
    </owl:Class>
    


    <!-- https://w3id.org/def/vaeontology#TaxonomyAlignment -->

    <owl:Class rdf:about="https://w3id.org/def/vaeontology#TaxonomyAlignment">
        <rdfs:subClassOf rdf:resource="https://w3id.org/def/vaeontology#QuantitativeVaeProperty"/>
        <rdfs:subClassOf rdf:resource="https://w3id.org/def/vaeontology#ValueProperty"/>
        <rdfs:subClassOf>
            <owl:Restriction>
                <owl:onProperty rdf:resource="https://w3id.org/def/vaeontology#isAlignmentOfTaxonomy"/>
                <owl:someValuesFrom rdf:resource="https://w3id.org/def/vaeontology#ValueTaxonomyStatement"/>
            </owl:Restriction>
        </rdfs:subClassOf>
        <rdfs:comment>&quot;We argue that the property-based nodes of a value taxonomy introduce the foundations for linking abstract value concepts to concrete computational constructs that can help formally assess the alignment of behaviour with those values. The value alignment of an entity’s behaviour becomes the degree of satisfaction of the property-based value nodes of the relevant taxonomy that this behaviour brings about.&quot;</rdfs:comment>
        <rdfs:label>Taxonomy Alignment</rdfs:label>
        <rdfs:seeAlso rdf:resource="https://w3id.org/def/vaeontology#ValueTaxonomy"/>
        <bhv:bibRef>Osman, N., d’Inverno, M.: A computational framework of human values for ethical
ai (2023)</bhv:bibRef>
    </owl:Class>
    


    <!-- https://w3id.org/def/vaeontology#TaxonomyProperty -->

    <owl:Class rdf:about="https://w3id.org/def/vaeontology#TaxonomyProperty">
        <rdfs:subClassOf rdf:resource="https://w3id.org/def/vaeontology#QuantitativeVaeProperty"/>
        <rdfs:subClassOf rdf:resource="https://w3id.org/def/vaeontology#ValueProperty"/>
        <rdfs:comment>[Nardine Osman, Mark D’Inverno https://arxiv.org/abs/2305.02748]</rdfs:comment>
        <rdfs:label>Property Taxonomy</rdfs:label>
    </owl:Class>
    


    <!-- https://w3id.org/def/vaeontology#TextualVaeProperty -->

    <owl:Class rdf:about="https://w3id.org/def/vaeontology#TextualVaeProperty">
        <rdfs:subClassOf rdf:resource="https://w3id.org/def/vaeontology#VaeProperty"/>
        <rdfs:comment>A VaeProperty expressed in natural language.</rdfs:comment>
        <rdfs:label>Textual Vae Property</rdfs:label>
    </owl:Class>
    


    <!-- https://w3id.org/def/vaeontology#Treasure -->

    <owl:Class rdf:about="https://w3id.org/def/vaeontology#Treasure">
        <rdfs:subClassOf rdf:resource="https://w3id.org/spice/SON/SchwartzValues#Value"/>
        <rdfs:comment>Term added automatically</rdfs:comment>
        <rdfs:comment>Treasure: hold dear</rdfs:comment>
        <rdfs:label>Treasure</rdfs:label>
    </owl:Class>
    


    <!-- https://w3id.org/def/vaeontology#User -->

    <owl:Class rdf:about="https://w3id.org/def/vaeontology#User">
        <rdfs:subClassOf rdf:resource="http://www.ontologydesignpatterns.org/ont/dul/DUL.owl#Person"/>
        <rdfs:subClassOf rdf:resource="https://w3id.org/def/vaeontology#Agent"/>
        <rdfs:subClassOf>
            <owl:Restriction>
                <owl:onProperty rdf:resource="https://w3id.org/def/vaeontology#isUserOfSystem"/>
                <owl:someValuesFrom rdf:resource="https://w3id.org/def/vaeontology#System"/>
            </owl:Restriction>
        </rdfs:subClassOf>
        <rdfs:comment>A User is a human agent that can take part in a system (or model it, supervise it, interact with it...)</rdfs:comment>
        <rdfs:label>User</rdfs:label>
    </owl:Class>
    


    <!-- https://w3id.org/def/vaeontology#VaeConditionedEntity -->

    <owl:Class rdf:about="https://w3id.org/def/vaeontology#VaeConditionedEntity">
        <rdfs:subClassOf rdf:resource="https://w3id.org/def/vaeontology#VaeStatementEntity"/>
    </owl:Class>
    


    <!-- https://w3id.org/def/vaeontology#VaeConditioningEntity -->

    <owl:Class rdf:about="https://w3id.org/def/vaeontology#VaeConditioningEntity">
        <rdfs:subClassOf rdf:resource="https://w3id.org/def/vaeontology#VaeStatementEntity"/>
    </owl:Class>
    


    <!-- https://w3id.org/def/vaeontology#VaeEntity -->

    <owl:Class rdf:about="https://w3id.org/def/vaeontology#VaeEntity">
        <rdfs:subClassOf rdf:resource="http://www.ontologydesignpatterns.org/ont/dul/DUL.owl#Entity"/>
        <rdfs:subClassOf>
            <owl:Restriction>
                <owl:onProperty rdf:resource="http://www.ontologydesignpatterns.org/ont/dul/DUL.owl#hasSetting"/>
                <owl:someValuesFrom rdf:resource="https://w3id.org/def/vaeontology#Context"/>
            </owl:Restriction>
        </rdfs:subClassOf>
        <rdfs:comment>Any kind of object from the VAE domain that is contextualized.</rdfs:comment>
        <rdfs:label>Vae Object</rdfs:label>
        <rdfs:seeAlso rdf:resource="https://w3id.org/def/vaeontology#Context"/>
    </owl:Class>
    


    <!-- https://w3id.org/def/vaeontology#VaeProperty -->

    <owl:Class rdf:about="https://w3id.org/def/vaeontology#VaeProperty">
        <rdfs:subClassOf rdf:resource="http://www.ontologydesignpatterns.org/ont/dul/DUL.owl#Description"/>
        <rdfs:subClassOf rdf:resource="https://w3id.org/def/vaeontology#VaeStatementEntity"/>
        <rdfs:subClassOf>
            <owl:Restriction>
                <owl:onProperty rdf:resource="https://w3id.org/def/vaeontology#measuredOnOutcome"/>
                <owl:someValuesFrom rdf:resource="https://w3id.org/def/vaeontology#Outcome"/>
            </owl:Restriction>
        </rdfs:subClassOf>
        <rdfs:subClassOf>
            <owl:Restriction>
                <owl:onProperty rdf:resource="https://w3id.org/def/vaeontology#propertyExpressedAt"/>
                <owl:allValuesFrom rdf:resource="https://w3id.org/def/vaeontology#VaePropertyStatement"/>
            </owl:Restriction>
        </rdfs:subClassOf>
        <rdfs:subClassOf>
            <owl:Restriction>
                <owl:onProperty rdf:resource="https://w3id.org/def/vaeontology#relationWith"/>
                <owl:allValuesFrom rdf:resource="https://w3id.org/def/vaeontology#VaeConditioningEntity"/>
            </owl:Restriction>
        </rdfs:subClassOf>
        <rdfs:comment>Any property measured on an Outcome, useful to describe some aspect that is related to a Norm or a Value</rdfs:comment>
        <rdfs:label>Vae Property</rdfs:label>
    </owl:Class>
    


    <!-- https://w3id.org/def/vaeontology#VaePropertyStatement -->

    <owl:Class rdf:about="https://w3id.org/def/vaeontology#VaePropertyStatement">
        <rdfs:subClassOf rdf:resource="https://w3id.org/def/vaeontology#AgentStatement"/>
        <rdfs:subClassOf>
            <owl:Restriction>
                <owl:onProperty rdf:resource="https://w3id.org/def/vaeontology#expressesProperty"/>
                <owl:someValuesFrom rdf:resource="https://w3id.org/def/vaeontology#VaeProperty"/>
            </owl:Restriction>
        </rdfs:subClassOf>
        <rdfs:comment>An AgentStatement where the agent expresses some VaeProperty of an Outcome.</rdfs:comment>
        <rdfs:label>Vae Property Statement</rdfs:label>
    </owl:Class>
    


    <!-- https://w3id.org/def/vaeontology#VaeSituation -->

    <owl:Class rdf:about="https://w3id.org/def/vaeontology#VaeSituation">
        <rdfs:subClassOf rdf:resource="http://www.w3.org/ns/odrl/2/Asset"/>
        <rdfs:subClassOf rdf:resource="https://w3id.org/def/vaeontology#VaeEntity"/>
        <rdfs:subClassOf rdf:resource="https://w3id.org/framester/schema/FrameOccurrence"/>
        <rdfs:subClassOf>
            <owl:Restriction>
                <owl:onProperty rdf:resource="http://www.ontologydesignpatterns.org/ont/dul/DUL.owl#satisfies"/>
                <owl:someValuesFrom rdf:resource="https://w3id.org/def/vaeontology#VaeStatement"/>
            </owl:Restriction>
        </rdfs:subClassOf>
        <rdfs:subClassOf>
            <owl:Restriction>
                <owl:onProperty rdf:resource="http://www.ontologydesignpatterns.org/ont/dul/DUL.owl#satisfies"/>
                <owl:someValuesFrom rdf:resource="https://w3id.org/def/vaeontology#ValueConcept"/>
            </owl:Restriction>
        </rdfs:subClassOf>
        <owl:disjointWith rdf:resource="https://w3id.org/def/vaeontology#VaeStatement"/>
        <rdfs:comment>Any kind of VaePropertyStatement proposed by an agent in which they express that a complex notion of understanding, preservation or respect with a ValueConcept/Norm is present on entity (Agent or Outcome or Norm) based on some VaeProperty(s) seen.</rdfs:comment>
        <rdfs:label>Vae Statement</rdfs:label>
    </owl:Class>
    


    <!-- https://w3id.org/def/vaeontology#VaeStatement -->

    <owl:Class rdf:about="https://w3id.org/def/vaeontology#VaeStatement">
        <rdfs:subClassOf rdf:resource="http://www.w3.org/ns/odrl/2/Action"/>
        <rdfs:subClassOf rdf:resource="http://www.w3.org/ns/odrl/2/Asset"/>
        <rdfs:subClassOf rdf:resource="https://w3id.org/def/vaeontology#VaePropertyStatement"/>
        <rdfs:subClassOf>
            <owl:Class>
                <owl:unionOf rdf:parseType="Collection">
                    <owl:Restriction>
                        <owl:onProperty rdf:resource="https://w3id.org/def/vaeontology#interpretationOn"/>
                        <owl:someValuesFrom rdf:resource="https://w3id.org/def/vaeontology#Norm"/>
                    </owl:Restriction>
                    <owl:Restriction>
                        <owl:onProperty rdf:resource="https://w3id.org/def/vaeontology#interpretationOn"/>
                        <owl:someValuesFrom rdf:resource="https://w3id.org/def/vaeontology#Value"/>
                    </owl:Restriction>
                </owl:unionOf>
            </owl:Class>
        </rdfs:subClassOf>
        <rdfs:subClassOf>
            <owl:Restriction>
                <owl:onProperty rdf:resource="https://w3id.org/def/vaeontology#onEntity"/>
                <owl:someValuesFrom rdf:resource="https://w3id.org/def/vaeontology#VaeConditionedEntity"/>
            </owl:Restriction>
        </rdfs:subClassOf>
        <rdfs:subClassOf>
            <owl:Restriction>
                <owl:onProperty rdf:resource="http://www.ontologydesignpatterns.org/ont/dul/DUL.owl#isSatisfiedBy"/>
                <owl:allValuesFrom rdf:resource="https://w3id.org/def/vaeontology#VaeSituation"/>
            </owl:Restriction>
        </rdfs:subClassOf>
        <rdfs:comment>Any kind of VaePropertyStatement proposed by an agent in which they express that a complex notion of understanding, preservation or respect with a ValueConcept/Norm is present on entity (Agent or Outcome or Norm) based on some VaeProperty(s) seen.</rdfs:comment>
        <rdfs:label>Vae Statement</rdfs:label>
    </owl:Class>
    


    <!-- https://w3id.org/def/vaeontology#VaeStatementEntity -->

    <owl:Class rdf:about="https://w3id.org/def/vaeontology#VaeStatementEntity">
        <rdfs:subClassOf rdf:resource="https://w3id.org/def/vaeontology#VaeEntity"/>
    </owl:Class>
    


    <!-- https://w3id.org/def/vaeontology#Value -->

    <owl:Class rdf:about="https://w3id.org/def/vaeontology#Value">
        <owl:equivalentClass rdf:resource="https://w3id.org/spice/SON/SchwartzValues#Value"/>
        <rdfs:subClassOf rdf:resource="https://w3id.org/def/vaeontology#ValueConcept"/>
        <rdfs:comment>&quot;Values are very general, abstract guiding principles that individuals and groups utilise to generate judgements on a variety of constructs, such as actions, strategies, conventions and policies&quot;</rdfs:comment>
        <rdfs:label>Value</rdfs:label>
        <bhv:bibRef>Nieves Montes, Nardine Osman, and Carles Sierra, ‘Perspective-dependent value alignment of norms’ VALE workshop, ECAI 2023</bhv:bibRef>
    </owl:Class>
    


    <!-- https://w3id.org/def/vaeontology#ValueComparisonStatement -->

    <owl:Class rdf:about="https://w3id.org/def/vaeontology#ValueComparisonStatement">
        <rdfs:subClassOf rdf:resource="https://w3id.org/def/vaeontology#VaePropertyStatement"/>
        <rdfs:subClassOf>
            <owl:Class>
                <owl:intersectionOf rdf:parseType="Collection">
                    <owl:Restriction>
                        <owl:onProperty rdf:resource="https://w3id.org/def/vaeontology#comparisonHasInferior"/>
                        <owl:someValuesFrom rdf:resource="https://w3id.org/def/vaeontology#ValueConcept"/>
                    </owl:Restriction>
                    <owl:Restriction>
                        <owl:onProperty rdf:resource="https://w3id.org/def/vaeontology#comparisonHasSuperior"/>
                        <owl:someValuesFrom rdf:resource="https://w3id.org/def/vaeontology#ValueConcept"/>
                    </owl:Restriction>
                </owl:intersectionOf>
            </owl:Class>
        </rdfs:subClassOf>
        <rdfs:comment>Any kind of comparison proposed by an Agent (or that the Agent believes in) between two instances of ValueConcepts, under some context.</rdfs:comment>
        <rdfs:label>Value Comparison Statement</rdfs:label>
    </owl:Class>
    


    <!-- https://w3id.org/def/vaeontology#ValueConcept -->

    <owl:Class rdf:about="https://w3id.org/def/vaeontology#ValueConcept">
        <rdfs:subClassOf rdf:resource="https://w3id.org/def/vaeontology#VaeConditioningEntity"/>
        <rdfs:subClassOf rdf:resource="https://w3id.org/framester/schema/ConceptualFrame"/>
        <rdfs:subClassOf>
            <owl:Restriction>
                <owl:onProperty rdf:resource="https://w3id.org/def/vaeontology#shapesNorm"/>
                <owl:someValuesFrom rdf:resource="https://w3id.org/def/vaeontology#Norm"/>
            </owl:Restriction>
        </rdfs:subClassOf>
        <rdfs:comment>Any abstraction of Value, something that is considered as such even if not present in any specific theory.</rdfs:comment>
        <rdfs:label>Value Concept</rdfs:label>
        <rdfs:seeAlso rdf:resource="http://www.ontologydesignpatterns.org/ont/values/valuecore#Value"/>
    </owl:Class>
    


    <!-- https://w3id.org/def/vaeontology#ValueDefinition -->

    <owl:Class rdf:about="https://w3id.org/def/vaeontology#ValueDefinition">
        <rdfs:subClassOf rdf:resource="https://w3id.org/def/vaeontology#AgentStatement"/>
        <rdfs:subClassOf>
            <owl:Restriction>
                <owl:onProperty rdf:resource="https://w3id.org/framester/schema/perspectiveOn"/>
                <owl:someValuesFrom rdf:resource="https://w3id.org/def/vaeontology#ValueConcept"/>
            </owl:Restriction>
        </rdfs:subClassOf>
        <rdfs:comment>A context-dependent grounded definition of a value.</rdfs:comment>
        <rdfs:label>Value Definition</rdfs:label>
    </owl:Class>
    


    <!-- https://w3id.org/def/vaeontology#ValueProperty -->

    <owl:Class rdf:about="https://w3id.org/def/vaeontology#ValueProperty">
        <rdfs:subClassOf rdf:resource="https://w3id.org/def/vaeontology#VaeProperty"/>
        <rdfs:subClassOf>
            <owl:Restriction>
                <owl:onProperty rdf:resource="https://w3id.org/def/vaeontology#relationWith"/>
                <owl:allValuesFrom rdf:resource="https://w3id.org/def/vaeontology#ValueConcept"/>
            </owl:Restriction>
        </rdfs:subClassOf>
        <rdfs:comment>A VaeProperty specifying something about a ValueConcept.</rdfs:comment>
        <rdfs:label>Value Property</rdfs:label>
    </owl:Class>
    


    <!-- https://w3id.org/def/vaeontology#ValueTaxonomyStatement -->

    <owl:Class rdf:about="https://w3id.org/def/vaeontology#ValueTaxonomyStatement">
        <rdfs:subClassOf rdf:resource="https://w3id.org/def/vaeontology#VaePropertyStatement"/>
        <rdfs:subClassOf>
            <owl:Class>
                <owl:intersectionOf rdf:parseType="Collection">
                    <owl:Restriction>
                        <owl:onProperty rdf:resource="https://w3id.org/def/vaeontology#hasPropertyNode"/>
                        <owl:someValuesFrom rdf:resource="https://w3id.org/def/vaeontology#PropertyNode"/>
                    </owl:Restriction>
                    <owl:Restriction>
                        <owl:onProperty rdf:resource="https://w3id.org/def/vaeontology#hasConceptNode"/>
                        <owl:allValuesFrom rdf:resource="https://w3id.org/def/vaeontology#ConceptNode"/>
                    </owl:Restriction>
                    <owl:Restriction>
                        <owl:onProperty rdf:resource="https://w3id.org/def/vaeontology#hasRootNode"/>
                        <owl:qualifiedCardinality rdf:datatype="http://www.w3.org/2001/XMLSchema#nonNegativeInteger">1</owl:qualifiedCardinality>
                        <owl:onClass rdf:resource="https://w3id.org/def/vaeontology#ConceptNode"/>
                    </owl:Restriction>
                </owl:intersectionOf>
            </owl:Class>
        </rdfs:subClassOf>
        <rdfs:comment>[Nardine Osman, Mark D’Inverno https://arxiv.org/abs/2305.02748]</rdfs:comment>
        <rdfs:label>Value Taxonomy</rdfs:label>
        <rdfs:seeAlso rdf:resource="https://w3id.org/def/vaeontology#TaxonomyAlignment"/>
        <bhv:bibRef>Osman, N., d’Inverno, M.: A computational framework of human values for ethical
ai (2023)</bhv:bibRef>
    </owl:Class>
    


    <!-- https://w3id.org/framester/schema/ConceptualFrame -->

    <owl:Class rdf:about="https://w3id.org/framester/schema/ConceptualFrame">
        <rdfs:subClassOf rdf:resource="http://www.ontologydesignpatterns.org/ont/dul/DUL.owl#Description"/>
    </owl:Class>
    


    <!-- https://w3id.org/framester/schema/FrameOccurrence -->

    <owl:Class rdf:about="https://w3id.org/framester/schema/FrameOccurrence">
        <rdfs:subClassOf rdf:resource="http://www.ontologydesignpatterns.org/ont/dul/DUL.owl#Situation"/>
    </owl:Class>
    


    <!-- https://w3id.org/spice/SON/SchwartzValues#Achievement -->

    <owl:Class rdf:about="https://w3id.org/spice/SON/SchwartzValues#Achievement">
        <rdfs:subClassOf rdf:resource="https://w3id.org/def/vaeontology#Value"/>
        <rdfs:subClassOf rdf:resource="https://w3id.org/spice/SON/SchwartzValues#SelfEnhancement"/>
        <rdfs:label>Achievement</rdfs:label>
    </owl:Class>
    


    <!-- https://w3id.org/spice/SON/SchwartzValues#Action -->

    <owl:Class rdf:about="https://w3id.org/spice/SON/SchwartzValues#Action">
        <rdfs:subClassOf rdf:resource="https://w3id.org/spice/SON/SchwartzValues#SelfDirection"/>
        <owl:disjointWith rdf:resource="https://w3id.org/spice/SON/SchwartzValues#Thought"/>
        <bhv:bibRef>&quot;The freedom to determine one&apos;s own actions.&quot;

Giménez, August Corrons, and Lluís Garay Tamajón. &quot;Analysis of the third-order structuring of Shalom Schwartz’s theory of basic human values.&quot; Heliyon 5.6 (2019): e01797.</bhv:bibRef>
    </owl:Class>
    


    <!-- https://w3id.org/spice/SON/SchwartzValues#Benevolence -->

    <owl:Class rdf:about="https://w3id.org/spice/SON/SchwartzValues#Benevolence">
        <rdfs:subClassOf rdf:resource="https://w3id.org/def/vaeontology#Value"/>
        <rdfs:subClassOf rdf:resource="https://w3id.org/spice/SON/SchwartzValues#SelfTrascendence"/>
        <owl:disjointWith rdf:resource="https://w3id.org/spice/SON/SchwartzValues#Humility"/>
        <rdfs:label>Benevolence</rdfs:label>
    </owl:Class>
    


    <!-- https://w3id.org/spice/SON/SchwartzValues#Caring -->

    <owl:Class rdf:about="https://w3id.org/spice/SON/SchwartzValues#Caring">
        <rdfs:subClassOf rdf:resource="https://w3id.org/spice/SON/SchwartzValues#Benevolence"/>
        <owl:disjointWith rdf:resource="https://w3id.org/spice/SON/SchwartzValues#Dependability"/>
        <bhv:bibRef>&quot;Devotion to the wellbeing of group members.&quot;

Giménez, August Corrons, and Lluís Garay Tamajón. &quot;Analysis of the third-order structuring of Shalom Schwartz’s theory of basic human values.&quot; Heliyon 5.6 (2019): e01797.</bhv:bibRef>
    </owl:Class>
    


    <!-- https://w3id.org/spice/SON/SchwartzValues#Concern -->

    <owl:Class rdf:about="https://w3id.org/spice/SON/SchwartzValues#Concern">
        <rdfs:subClassOf rdf:resource="https://w3id.org/spice/SON/SchwartzValues#Universalism"/>
        <bhv:bibRef>&quot;Commitment to equality, justice and protection for all.&quot;

Giménez, August Corrons, and Lluís Garay Tamajón. &quot;Analysis of the third-order structuring of Shalom Schwartz’s theory of basic human values.&quot; Heliyon 5.6 (2019): e01797.</bhv:bibRef>
    </owl:Class>
    


    <!-- https://w3id.org/spice/SON/SchwartzValues#Conformity -->

    <owl:Class rdf:about="https://w3id.org/spice/SON/SchwartzValues#Conformity">
        <rdfs:subClassOf rdf:resource="https://w3id.org/spice/SON/SchwartzValues#Conservation"/>
        <bhv:bibRef>&quot;Control of one&apos;s own impulses and behaviour, in line with social norms and expectations.&quot;

Giménez, August Corrons, and Lluís Garay Tamajón. &quot;Analysis of the third-order structuring of Shalom Schwartz’s theory of basic human values.&quot; Heliyon 5.6 (2019): e01797.</bhv:bibRef>
    </owl:Class>
    


    <!-- https://w3id.org/spice/SON/SchwartzValues#Conservation -->

    <owl:Class rdf:about="https://w3id.org/spice/SON/SchwartzValues#Conservation">
        <owl:equivalentClass>
            <owl:Class>
                <owl:intersectionOf rdf:parseType="Collection">
                    <owl:Class>
                        <owl:unionOf rdf:parseType="Collection">
                            <owl:Restriction>
                                <owl:onProperty rdf:resource="https://w3id.org/spice/SON/SchwartzValues#focus"/>
                                <owl:someValuesFrom rdf:resource="https://w3id.org/spice/SON/SchwartzValues#PersonalFocus"/>
                            </owl:Restriction>
                            <owl:Restriction>
                                <owl:onProperty rdf:resource="https://w3id.org/spice/SON/SchwartzValues#focus"/>
                                <owl:someValuesFrom rdf:resource="https://w3id.org/spice/SON/SchwartzValues#SocialFocus"/>
                            </owl:Restriction>
                        </owl:unionOf>
                    </owl:Class>
                    <owl:Restriction>
                        <owl:onProperty rdf:resource="https://w3id.org/spice/SON/SchwartzValues#attitude"/>
                        <owl:allValuesFrom rdf:resource="https://w3id.org/spice/SON/SchwartzValues#SelfProtectionAndAnxietyAvoidance"/>
                    </owl:Restriction>
                    <owl:Restriction>
                        <owl:onProperty rdf:resource="https://w3id.org/spice/SON/SchwartzValues#valueMotivation"/>
                        <owl:allValuesFrom rdf:resource="https://w3id.org/spice/SON/SchwartzValues#Conservation"/>
                    </owl:Restriction>
                </owl:intersectionOf>
            </owl:Class>
        </owl:equivalentClass>
        <owl:equivalentClass>
            <owl:Restriction>
                <owl:onProperty rdf:resource="https://w3id.org/spice/SON/SchwartzValues#opposingValueMotivation"/>
                <owl:someValuesFrom rdf:resource="https://w3id.org/spice/SON/SchwartzValues#OpennessToChange"/>
            </owl:Restriction>
        </owl:equivalentClass>
        <rdfs:subClassOf rdf:resource="https://w3id.org/def/vaeontology#ValueConcept"/>
    </owl:Class>
    


    <!-- https://w3id.org/spice/SON/SchwartzValues#Dependability -->

    <owl:Class rdf:about="https://w3id.org/spice/SON/SchwartzValues#Dependability">
        <rdfs:subClassOf rdf:resource="https://w3id.org/spice/SON/SchwartzValues#Benevolence"/>
        <bhv:bibRef>&quot;Being a reliable and trustworthy member of the in-group.&quot;

Giménez, August Corrons, and Lluís Garay Tamajón. &quot;Analysis of the third-order structuring of Shalom Schwartz’s theory of basic human values.&quot; Heliyon 5.6 (2019): e01797.</bhv:bibRef>
    </owl:Class>
    


    <!-- https://w3id.org/spice/SON/SchwartzValues#Dominance -->

    <owl:Class rdf:about="https://w3id.org/spice/SON/SchwartzValues#Dominance">
        <rdfs:subClassOf rdf:resource="https://w3id.org/spice/SON/SchwartzValues#Power"/>
        <owl:disjointWith rdf:resource="https://w3id.org/spice/SON/SchwartzValues#Resources"/>
        <bhv:bibRef>&quot;Power through exercising control over others.&quot;

Giménez, August Corrons, and Lluís Garay Tamajón. &quot;Analysis of the third-order structuring of Shalom Schwartz’s theory of basic human values.&quot; Heliyon 5.6 (2019): e01797.</bhv:bibRef>
    </owl:Class>
    


    <!-- https://w3id.org/spice/SON/SchwartzValues#Face -->

    <owl:Class rdf:about="https://w3id.org/spice/SON/SchwartzValues#Face">
        <rdfs:subClassOf rdf:resource="https://w3id.org/spice/SON/SchwartzValues#Conservation"/>
        <rdfs:subClassOf rdf:resource="https://w3id.org/spice/SON/SchwartzValues#SelfEnhancement"/>
        <bhv:bibRef>&quot;Security and power via the keeping up of one&apos;s own public image and avoidance of humiliation.&quot;

Giménez, August Corrons, and Lluís Garay Tamajón. &quot;Analysis of the third-order structuring of Shalom Schwartz’s theory of basic human values.&quot; Heliyon 5.6 (2019): e01797.</bhv:bibRef>
    </owl:Class>
    


    <!-- https://w3id.org/spice/SON/SchwartzValues#Focus -->

    <owl:Class rdf:about="https://w3id.org/spice/SON/SchwartzValues#Focus">
        <rdfs:subClassOf rdf:resource="https://w3id.org/def/vaeontology#ValueConcept"/>
    </owl:Class>
    


    <!-- https://w3id.org/spice/SON/SchwartzValues#GrowthAndAnxietyFree -->

    <owl:Class rdf:about="https://w3id.org/spice/SON/SchwartzValues#GrowthAndAnxietyFree">
        <rdfs:subClassOf rdf:resource="https://w3id.org/def/vaeontology#ValueConcept"/>
    </owl:Class>
    


    <!-- https://w3id.org/spice/SON/SchwartzValues#Hedonism -->

    <owl:Class rdf:about="https://w3id.org/spice/SON/SchwartzValues#Hedonism">
        <rdfs:subClassOf rdf:resource="https://w3id.org/spice/SON/SchwartzValues#OpennessToChange"/>
        <rdfs:subClassOf rdf:resource="https://w3id.org/spice/SON/SchwartzValues#SelfEnhancement"/>
        <bhv:bibRef>&quot;The search for pleasure and sensuous gratification or satisfaction for oneself.&quot;

Giménez, August Corrons, and Lluís Garay Tamajón. &quot;Analysis of the third-order structuring of Shalom Schwartz’s theory of basic human values.&quot; Heliyon 5.6 (2019): e01797.</bhv:bibRef>
    </owl:Class>
    


    <!-- https://w3id.org/spice/SON/SchwartzValues#Humility -->

    <owl:Class rdf:about="https://w3id.org/spice/SON/SchwartzValues#Humility">
        <owl:equivalentClass>
            <owl:Class>
                <owl:intersectionOf rdf:parseType="Collection">
                    <owl:Class>
                        <owl:unionOf rdf:parseType="Collection">
                            <owl:Restriction>
                                <owl:onProperty rdf:resource="https://w3id.org/spice/SON/SchwartzValues#attitude"/>
                                <owl:someValuesFrom rdf:resource="https://w3id.org/spice/SON/SchwartzValues#GrowthAndAnxietyFree"/>
                            </owl:Restriction>
                            <owl:Restriction>
                                <owl:onProperty rdf:resource="https://w3id.org/spice/SON/SchwartzValues#attitude"/>
                                <owl:someValuesFrom rdf:resource="https://w3id.org/spice/SON/SchwartzValues#SelfProtectionAndAnxietyAvoidance"/>
                            </owl:Restriction>
                        </owl:unionOf>
                    </owl:Class>
                    <owl:Class>
                        <owl:complementOf>
                            <owl:Restriction>
                                <owl:onProperty rdf:resource="https://w3id.org/spice/SON/SchwartzValues#focus"/>
                                <owl:someValuesFrom rdf:resource="https://w3id.org/spice/SON/SchwartzValues#PersonalFocus"/>
                            </owl:Restriction>
                        </owl:complementOf>
                    </owl:Class>
                    <owl:Restriction>
                        <owl:onProperty rdf:resource="https://w3id.org/spice/SON/SchwartzValues#focus"/>
                        <owl:allValuesFrom rdf:resource="https://w3id.org/spice/SON/SchwartzValues#SocialFocus"/>
                    </owl:Restriction>
                </owl:intersectionOf>
            </owl:Class>
        </owl:equivalentClass>
        <rdfs:subClassOf rdf:resource="https://w3id.org/spice/SON/SchwartzValues#Conservation"/>
        <rdfs:subClassOf rdf:resource="https://w3id.org/spice/SON/SchwartzValues#SelfTrascendence"/>
        <owl:disjointWith rdf:resource="https://w3id.org/spice/SON/SchwartzValues#Universalism"/>
        <bhv:bibRef>&quot;Acknowledgement of one&apos;s insignificance in the grand scheme of things.&quot;

Giménez, August Corrons, and Lluís Garay Tamajón. &quot;Analysis of the third-order structuring of Shalom Schwartz’s theory of basic human values.&quot; Heliyon 5.6 (2019): e01797.</bhv:bibRef>
    </owl:Class>
    


    <!-- https://w3id.org/spice/SON/SchwartzValues#Nature -->

    <owl:Class rdf:about="https://w3id.org/spice/SON/SchwartzValues#Nature">
        <rdfs:subClassOf rdf:resource="https://w3id.org/spice/SON/SchwartzValues#Universalism"/>
        <bhv:bibRef>&quot;Preservation of the natural environment.&quot;

Giménez, August Corrons, and Lluís Garay Tamajón. &quot;Analysis of the third-order structuring of Shalom Schwartz’s theory of basic human values.&quot; Heliyon 5.6 (2019): e01797.</bhv:bibRef>
    </owl:Class>
    


    <!-- https://w3id.org/spice/SON/SchwartzValues#OpennessToChange -->

    <owl:Class rdf:about="https://w3id.org/spice/SON/SchwartzValues#OpennessToChange">
        <owl:equivalentClass>
            <owl:Class>
                <owl:intersectionOf rdf:parseType="Collection">
                    <owl:Restriction>
                        <owl:onProperty rdf:resource="https://w3id.org/spice/SON/SchwartzValues#attitude"/>
                        <owl:allValuesFrom rdf:resource="https://w3id.org/spice/SON/SchwartzValues#GrowthAndAnxietyFree"/>
                    </owl:Restriction>
                    <owl:Restriction>
                        <owl:onProperty rdf:resource="https://w3id.org/spice/SON/SchwartzValues#focus"/>
                        <owl:allValuesFrom rdf:resource="https://w3id.org/spice/SON/SchwartzValues#PersonalFocus"/>
                    </owl:Restriction>
                    <owl:Restriction>
                        <owl:onProperty rdf:resource="https://w3id.org/spice/SON/SchwartzValues#valueMotivation"/>
                        <owl:allValuesFrom rdf:resource="https://w3id.org/spice/SON/SchwartzValues#OpennessToChange"/>
                    </owl:Restriction>
                </owl:intersectionOf>
            </owl:Class>
        </owl:equivalentClass>
        <owl:equivalentClass>
            <owl:Restriction>
                <owl:onProperty rdf:resource="https://w3id.org/spice/SON/SchwartzValues#opposingValueMotivation"/>
                <owl:someValuesFrom rdf:resource="https://w3id.org/spice/SON/SchwartzValues#Conservation"/>
            </owl:Restriction>
        </owl:equivalentClass>
        <rdfs:subClassOf rdf:resource="https://w3id.org/def/vaeontology#ValueConcept"/>
        <rdfs:label>Openness To Change</rdfs:label>
    </owl:Class>
    


    <!-- https://w3id.org/spice/SON/SchwartzValues#PanCulturalBaselineForValuesPriority -->

    <owl:Class rdf:about="https://w3id.org/spice/SON/SchwartzValues#PanCulturalBaselineForValuesPriority">
        <rdfs:subClassOf rdf:resource="https://w3id.org/def/vaeontology#ValueConcept"/>
        <bhv:bibRef>&quot;Individuals differ substantially in the importance they attribute to the ten values. At the societal level, however, consensus regarding the hierarchical order of the values is surprisingly high.&quot;

Basic Human Values: Theory, Measurement, and Applications - S.H. Shwartz (2006)</bhv:bibRef>
    </owl:Class>
    


    <!-- https://w3id.org/spice/SON/SchwartzValues#Personal -->

    <owl:Class rdf:about="https://w3id.org/spice/SON/SchwartzValues#Personal">
        <owl:equivalentClass>
            <owl:Class>
                <owl:intersectionOf rdf:parseType="Collection">
                    <owl:Class>
                        <owl:complementOf>
                            <owl:Restriction>
                                <owl:onProperty rdf:resource="https://w3id.org/spice/SON/SchwartzValues#attitude"/>
                                <owl:someValuesFrom rdf:resource="https://w3id.org/spice/SON/SchwartzValues#GrowthAndAnxietyFree"/>
                            </owl:Restriction>
                        </owl:complementOf>
                    </owl:Class>
                    <owl:Restriction>
                        <owl:onProperty rdf:resource="https://w3id.org/spice/SON/SchwartzValues#attitude"/>
                        <owl:allValuesFrom rdf:resource="https://w3id.org/spice/SON/SchwartzValues#SelfProtectionAndAnxietyAvoidance"/>
                    </owl:Restriction>
                    <owl:Restriction>
                        <owl:onProperty rdf:resource="https://w3id.org/spice/SON/SchwartzValues#focus"/>
                        <owl:allValuesFrom rdf:resource="https://w3id.org/spice/SON/SchwartzValues#PersonalFocus"/>
                    </owl:Restriction>
                    <owl:Restriction>
                        <owl:onProperty rdf:resource="https://w3id.org/spice/SON/SchwartzValues#valueMotivation"/>
                        <owl:allValuesFrom rdf:resource="https://w3id.org/spice/SON/SchwartzValues#Conservation"/>
                    </owl:Restriction>
                </owl:intersectionOf>
            </owl:Class>
        </owl:equivalentClass>
        <rdfs:subClassOf rdf:resource="https://w3id.org/spice/SON/SchwartzValues#Security"/>
        <owl:disjointWith rdf:resource="https://w3id.org/spice/SON/SchwartzValues#Societal"/>
        <bhv:bibRef>&quot;Safety in one&apos;s own immediate environment.&quot;

Giménez, August Corrons, and Lluís Garay Tamajón. &quot;Analysis of the third-order structuring of Shalom Schwartz’s theory of basic human values.&quot; Heliyon 5.6 (2019): e01797.</bhv:bibRef>
    </owl:Class>
    


    <!-- https://w3id.org/spice/SON/SchwartzValues#PersonalFocus -->

    <owl:Class rdf:about="https://w3id.org/spice/SON/SchwartzValues#PersonalFocus">
        <rdfs:subClassOf rdf:resource="https://w3id.org/spice/SON/SchwartzValues#Focus"/>
        <rdfs:comment>Focus on personal issues and self.</rdfs:comment>
        <bhv:bibRef>Giménez, August Corrons, and Lluís Garay Tamajón. &quot;Analysis of the third-order structuring of Shalom Schwartz’s theory of basic human values.&quot; Heliyon 5.6 (2019): e01797.</bhv:bibRef>
    </owl:Class>
    


    <!-- https://w3id.org/spice/SON/SchwartzValues#Power -->

    <owl:Class rdf:about="https://w3id.org/spice/SON/SchwartzValues#Power">
        <rdfs:subClassOf rdf:resource="https://w3id.org/def/vaeontology#Value"/>
        <rdfs:subClassOf rdf:resource="https://w3id.org/spice/SON/SchwartzValues#SelfEnhancement"/>
        <rdfs:label>Power</rdfs:label>
    </owl:Class>
    


    <!-- https://w3id.org/spice/SON/SchwartzValues#Resources -->

    <owl:Class rdf:about="https://w3id.org/spice/SON/SchwartzValues#Resources">
        <rdfs:subClassOf rdf:resource="https://w3id.org/spice/SON/SchwartzValues#Power"/>
        <bhv:bibRef>&quot;Power through control of material and social resources.&quot;

Giménez, August Corrons, and Lluís Garay Tamajón. &quot;Analysis of the third-order structuring of Shalom Schwartz’s theory of basic human values.&quot; Heliyon 5.6 (2019): e01797.</bhv:bibRef>
    </owl:Class>
    


    <!-- https://w3id.org/spice/SON/SchwartzValues#Security -->

    <owl:Class rdf:about="https://w3id.org/spice/SON/SchwartzValues#Security">
        <rdfs:subClassOf rdf:resource="https://w3id.org/spice/SON/SchwartzValues#Conservation"/>
        <bhv:bibRef>&quot;Personal wellbeing and that of in-persons and in-groups, as well as the stability of society and oneself.&quot;

Giménez, August Corrons, and Lluís Garay Tamajón. &quot;Analysis of the third-order structuring of Shalom Schwartz’s theory of basic human values.&quot; Heliyon 5.6 (2019): e01797.</bhv:bibRef>
    </owl:Class>
    


    <!-- https://w3id.org/spice/SON/SchwartzValues#SelfDirection -->

    <owl:Class rdf:about="https://w3id.org/spice/SON/SchwartzValues#SelfDirection">
        <rdfs:subClassOf rdf:resource="https://w3id.org/spice/SON/SchwartzValues#OpennessToChange"/>
        <bhv:bibRef>&quot;Independence of thought, action and opinion.&quot;

Giménez, August Corrons, and Lluís Garay Tamajón. &quot;Analysis of the third-order structuring of Shalom Schwartz’s theory of basic human values.&quot; Heliyon 5.6 (2019): e01797.</bhv:bibRef>
    </owl:Class>
    


    <!-- https://w3id.org/spice/SON/SchwartzValues#SelfEnhancement -->

    <owl:Class rdf:about="https://w3id.org/spice/SON/SchwartzValues#SelfEnhancement">
        <owl:equivalentClass>
            <owl:Class>
                <owl:intersectionOf rdf:parseType="Collection">
                    <owl:Class>
                        <owl:unionOf rdf:parseType="Collection">
                            <owl:Restriction>
                                <owl:onProperty rdf:resource="https://w3id.org/spice/SON/SchwartzValues#attitude"/>
                                <owl:someValuesFrom rdf:resource="https://w3id.org/spice/SON/SchwartzValues#GrowthAndAnxietyFree"/>
                            </owl:Restriction>
                            <owl:Restriction>
                                <owl:onProperty rdf:resource="https://w3id.org/spice/SON/SchwartzValues#attitude"/>
                                <owl:someValuesFrom rdf:resource="https://w3id.org/spice/SON/SchwartzValues#SelfProtectionAndAnxietyAvoidance"/>
                            </owl:Restriction>
                        </owl:unionOf>
                    </owl:Class>
                    <owl:Restriction>
                        <owl:onProperty rdf:resource="https://w3id.org/spice/SON/SchwartzValues#focus"/>
                        <owl:allValuesFrom rdf:resource="https://w3id.org/spice/SON/SchwartzValues#PersonalFocus"/>
                    </owl:Restriction>
                    <owl:Restriction>
                        <owl:onProperty rdf:resource="https://w3id.org/spice/SON/SchwartzValues#valueMotivation"/>
                        <owl:allValuesFrom rdf:resource="https://w3id.org/spice/SON/SchwartzValues#SelfEnhancement"/>
                    </owl:Restriction>
                </owl:intersectionOf>
            </owl:Class>
        </owl:equivalentClass>
        <owl:equivalentClass>
            <owl:Restriction>
                <owl:onProperty rdf:resource="https://w3id.org/spice/SON/SchwartzValues#opposingValueMotivation"/>
                <owl:someValuesFrom rdf:resource="https://w3id.org/spice/SON/SchwartzValues#SelfTrascendence"/>
            </owl:Restriction>
        </owl:equivalentClass>
        <rdfs:subClassOf rdf:resource="https://w3id.org/def/vaeontology#ValueConcept"/>
        <rdfs:label>Self Enhancement</rdfs:label>
    </owl:Class>
    


    <!-- https://w3id.org/spice/SON/SchwartzValues#SelfProtectionAndAnxietyAvoidance -->

    <owl:Class rdf:about="https://w3id.org/spice/SON/SchwartzValues#SelfProtectionAndAnxietyAvoidance">
        <rdfs:subClassOf rdf:resource="https://w3id.org/def/vaeontology#ValueConcept"/>
        <rdfs:comment>The attitude to which can be ascribed some values motivations: Self Protection and Anxiety Avoidance is a reactive attitude.</rdfs:comment>
        <bhv:bibRef>Giménez, August Corrons, and Lluís Garay Tamajón. &quot;Analysis of the third-order structuring of Shalom Schwartz’s theory of basic human values.&quot; Heliyon 5.6 (2019): e01797.</bhv:bibRef>
    </owl:Class>
    


    <!-- https://w3id.org/spice/SON/SchwartzValues#SelfTrascendence -->

    <owl:Class rdf:about="https://w3id.org/spice/SON/SchwartzValues#SelfTrascendence">
        <owl:equivalentClass>
            <owl:Class>
                <owl:intersectionOf rdf:parseType="Collection">
                    <owl:Restriction>
                        <owl:onProperty rdf:resource="https://w3id.org/spice/SON/SchwartzValues#attitude"/>
                        <owl:allValuesFrom rdf:resource="https://w3id.org/spice/SON/SchwartzValues#GrowthAndAnxietyFree"/>
                    </owl:Restriction>
                    <owl:Restriction>
                        <owl:onProperty rdf:resource="https://w3id.org/spice/SON/SchwartzValues#focus"/>
                        <owl:allValuesFrom rdf:resource="https://w3id.org/spice/SON/SchwartzValues#SocialFocus"/>
                    </owl:Restriction>
                    <owl:Restriction>
                        <owl:onProperty rdf:resource="https://w3id.org/spice/SON/SchwartzValues#valueMotivation"/>
                        <owl:allValuesFrom rdf:resource="https://w3id.org/spice/SON/SchwartzValues#SelfTrascendence"/>
                    </owl:Restriction>
                </owl:intersectionOf>
            </owl:Class>
        </owl:equivalentClass>
        <owl:equivalentClass>
            <owl:Restriction>
                <owl:onProperty rdf:resource="https://w3id.org/spice/SON/SchwartzValues#opposingValueMotivation"/>
                <owl:someValuesFrom rdf:resource="https://w3id.org/spice/SON/SchwartzValues#SelfEnhancement"/>
            </owl:Restriction>
        </owl:equivalentClass>
        <rdfs:subClassOf rdf:resource="https://w3id.org/def/vaeontology#ValueConcept"/>
        <rdfs:label>Self Trascendence</rdfs:label>
    </owl:Class>
    


    <!-- https://w3id.org/spice/SON/SchwartzValues#SocialFocus -->

    <owl:Class rdf:about="https://w3id.org/spice/SON/SchwartzValues#SocialFocus">
        <rdfs:subClassOf rdf:resource="https://w3id.org/spice/SON/SchwartzValues#Focus"/>
        <rdfs:comment>Focus on social issues and others, or self as a member of a social community.</rdfs:comment>
        <bhv:bibRef>Giménez, August Corrons, and Lluís Garay Tamajón. &quot;Analysis of the third-order structuring of Shalom Schwartz’s theory of basic human values.&quot; Heliyon 5.6 (2019): e01797.</bhv:bibRef>
    </owl:Class>
    


    <!-- https://w3id.org/spice/SON/SchwartzValues#Societal -->

    <owl:Class rdf:about="https://w3id.org/spice/SON/SchwartzValues#Societal">
        <owl:equivalentClass>
            <owl:Class>
                <owl:intersectionOf rdf:parseType="Collection">
                    <owl:Class>
                        <owl:complementOf>
                            <owl:Restriction>
                                <owl:onProperty rdf:resource="https://w3id.org/spice/SON/SchwartzValues#attitude"/>
                                <owl:someValuesFrom rdf:resource="https://w3id.org/spice/SON/SchwartzValues#GrowthAndAnxietyFree"/>
                            </owl:Restriction>
                        </owl:complementOf>
                    </owl:Class>
                    <owl:Restriction>
                        <owl:onProperty rdf:resource="https://w3id.org/spice/SON/SchwartzValues#attitude"/>
                        <owl:allValuesFrom rdf:resource="https://w3id.org/spice/SON/SchwartzValues#SelfProtectionAndAnxietyAvoidance"/>
                    </owl:Restriction>
                    <owl:Restriction>
                        <owl:onProperty rdf:resource="https://w3id.org/spice/SON/SchwartzValues#focus"/>
                        <owl:allValuesFrom rdf:resource="https://w3id.org/spice/SON/SchwartzValues#SocialFocus"/>
                    </owl:Restriction>
                    <owl:Restriction>
                        <owl:onProperty rdf:resource="https://w3id.org/spice/SON/SchwartzValues#valueMotivation"/>
                        <owl:allValuesFrom rdf:resource="https://w3id.org/spice/SON/SchwartzValues#Conservation"/>
                    </owl:Restriction>
                </owl:intersectionOf>
            </owl:Class>
        </owl:equivalentClass>
        <rdfs:subClassOf rdf:resource="https://w3id.org/spice/SON/SchwartzValues#Security"/>
        <bhv:bibRef>&quot;Security and stability in wider society.&quot;

Giménez, August Corrons, and Lluís Garay Tamajón. &quot;Analysis of the third-order structuring of Shalom Schwartz’s theory of basic human values.&quot; Heliyon 5.6 (2019): e01797.</bhv:bibRef>
    </owl:Class>
    


    <!-- https://w3id.org/spice/SON/SchwartzValues#Stimulation -->

    <owl:Class rdf:about="https://w3id.org/spice/SON/SchwartzValues#Stimulation">
        <rdfs:subClassOf rdf:resource="https://w3id.org/def/vaeontology#Value"/>
        <rdfs:subClassOf rdf:resource="https://w3id.org/spice/SON/SchwartzValues#OpennessToChange"/>
        <rdfs:label>Stimulation</rdfs:label>
    </owl:Class>
    


    <!-- https://w3id.org/spice/SON/SchwartzValues#Thought -->

    <owl:Class rdf:about="https://w3id.org/spice/SON/SchwartzValues#Thought">
        <rdfs:subClassOf rdf:resource="https://w3id.org/spice/SON/SchwartzValues#SelfDirection"/>
        <bhv:bibRef>&quot;The freedom to cultivate one&apos;s own ideas and skills.&quot;

Giménez, August Corrons, and Lluís Garay Tamajón. &quot;Analysis of the third-order structuring of Shalom Schwartz’s theory of basic human values.&quot; Heliyon 5.6 (2019): e01797.</bhv:bibRef>
    </owl:Class>
    


    <!-- https://w3id.org/spice/SON/SchwartzValues#Tolerance -->

    <owl:Class rdf:about="https://w3id.org/spice/SON/SchwartzValues#Tolerance">
        <rdfs:subClassOf rdf:resource="https://w3id.org/spice/SON/SchwartzValues#Universalism"/>
        <bhv:bibRef>&quot;Acceptance and understanding of those different from oneself.&quot;

Giménez, August Corrons, and Lluís Garay Tamajón. &quot;Analysis of the third-order structuring of Shalom Schwartz’s theory of basic human values.&quot; Heliyon 5.6 (2019): e01797.</bhv:bibRef>
    </owl:Class>
    


    <!-- https://w3id.org/spice/SON/SchwartzValues#Tradition -->

    <owl:Class rdf:about="https://w3id.org/spice/SON/SchwartzValues#Tradition">
        <rdfs:subClassOf rdf:resource="https://w3id.org/spice/SON/SchwartzValues#Conservation"/>
        <bhv:bibRef>&quot;Respect for, commitment to and acceptation of the ideals and customs imposed by culture or religion.&quot;

Giménez, August Corrons, and Lluís Garay Tamajón. &quot;Analysis of the third-order structuring of Shalom Schwartz’s theory of basic human values.&quot; Heliyon 5.6 (2019): e01797.</bhv:bibRef>
    </owl:Class>
    


    <!-- https://w3id.org/spice/SON/SchwartzValues#Universalism -->

    <owl:Class rdf:about="https://w3id.org/spice/SON/SchwartzValues#Universalism">
        <rdfs:subClassOf rdf:resource="https://w3id.org/def/vaeontology#Value"/>
        <rdfs:subClassOf rdf:resource="https://w3id.org/spice/SON/SchwartzValues#SelfTrascendence"/>
        <rdfs:label>Universalism</rdfs:label>
    </owl:Class>
    


    <!-- https://w3id.org/spice/SON/SchwartzValues#Value -->

    <owl:Class rdf:about="https://w3id.org/spice/SON/SchwartzValues#Value">
        <rdfs:subClassOf rdf:resource="https://w3id.org/def/vaeontology#Value"/>
        <rdfs:subClassOf rdf:resource="https://w3id.org/def/vaeontology#ValueConcept"/>
        <rdfs:label>Value</rdfs:label>
    </owl:Class>
    


    <!-- 
    ///////////////////////////////////////////////////////////////////////////////////////
    //
    // Individuals
    //
    ///////////////////////////////////////////////////////////////////////////////////////
     -->

    


    <!-- https://w3id.org/def/vaeontology#achievementTax -->

    <owl:NamedIndividual rdf:about="https://w3id.org/def/vaeontology#achievementTax">
        <rdf:type rdf:resource="https://w3id.org/spice/SON/SchwartzValues#Achievement"/>
    </owl:NamedIndividual>
    


    <!-- https://w3id.org/def/vaeontology#actOfPayingMiniumumTaxes -->

    <owl:NamedIndividual rdf:about="https://w3id.org/def/vaeontology#actOfPayingMiniumumTaxes">
        <rdf:type rdf:resource="https://w3id.org/def/vaeontology#Action"/>
        <dul:hasSetting rdf:resource="https://w3id.org/def/vaeontology#taxProblemContext"/>
    </owl:NamedIndividual>
    


    <!-- https://w3id.org/def/vaeontology#actOfPayingTaxes -->

    <owl:NamedIndividual rdf:about="https://w3id.org/def/vaeontology#actOfPayingTaxes">
        <rdf:type rdf:resource="https://w3id.org/def/vaeontology#Action"/>
    </owl:NamedIndividual>
    


    <!-- https://w3id.org/def/vaeontology#aggregationSum -->

    <owl:NamedIndividual rdf:about="https://w3id.org/def/vaeontology#aggregationSum">
        <rdf:type rdf:resource="https://w3id.org/def/vaeontology#AggregationFunction"/>
        <measuredOnOutcome rdf:resource="https://w3id.org/def/vaeontology#state1"/>
        <measuredOnOutcome rdf:resource="https://w3id.org/def/vaeontology#state2"/>
        <rdf:value rdf:datatype="http://www.w3.org/2001/XMLSchema#decimal">0.87</rdf:value>
    </owl:NamedIndividual>
    


    <!-- https://w3id.org/def/vaeontology#alignClaim -->

    <owl:NamedIndividual rdf:about="https://w3id.org/def/vaeontology#alignClaim">
        <rdf:type rdf:resource="https://w3id.org/def/vaeontology#AlignmentStatement"/>
        <dul:hasSetting rdf:resource="https://w3id.org/def/vaeontology#taxProblemContext"/>
        <onEntity rdf:resource="https://w3id.org/def/vaeontology#state2"/>
        <withValue rdf:resource="https://w3id.org/def/vaeontology#benevolenceTax"/>
    </owl:NamedIndividual>
    


    <!-- https://w3id.org/def/vaeontology#alignPremise -->

    <owl:NamedIndividual rdf:about="https://w3id.org/def/vaeontology#alignPremise">
        <rdf:type rdf:resource="https://w3id.org/def/vaeontology#AlignmentStatement"/>
        <dul:hasSetting rdf:resource="https://w3id.org/def/vaeontology#taxProblemContext"/>
        <expressesProperty rdf:resource="https://w3id.org/def/vaeontology#giniIndex0_9"/>
        <expressesProperty rdf:resource="https://w3id.org/def/vaeontology#giniIndexSatisfiedThreshold0_7"/>
        <onEntity rdf:resource="https://w3id.org/def/vaeontology#state2"/>
        <withValue rdf:resource="https://w3id.org/def/vaeontology#equalityTax"/>
    </owl:NamedIndividual>
    


    <!-- https://w3id.org/def/vaeontology#alignmentSituationWithbenevolence -->

    <owl:NamedIndividual rdf:about="https://w3id.org/def/vaeontology#alignmentSituationWithbenevolence">
        <rdf:type rdf:resource="https://w3id.org/def/vaeontology#AlignmentSituation"/>
        <dul:satisfies rdf:resource="https://w3id.org/def/vaeontology#alignClaim"/>
        <dul:satisfies rdf:resource="https://w3id.org/def/vaeontology#benevolenceTax"/>
    </owl:NamedIndividual>
    


    <!-- https://w3id.org/def/vaeontology#argumentAlign -->

    <owl:NamedIndividual rdf:about="https://w3id.org/def/vaeontology#argumentAlign">
        <rdf:type rdf:resource="https://w3id.org/def/vaeontology#ArgumentStatement"/>
        <dul:hasSetting rdf:resource="https://w3id.org/def/vaeontology#taxProblemContext"/>
        <hasClaim rdf:resource="https://w3id.org/def/vaeontology#alignClaim"/>
        <hasPremise rdf:resource="https://w3id.org/def/vaeontology#alignPremise"/>
        <isBasedOnCriterion rdf:resource="https://w3id.org/def/vaeontology#criterionAlign"/>
    </owl:NamedIndividual>
    


    <!-- https://w3id.org/def/vaeontology#benevolenceDef -->

    <owl:NamedIndividual rdf:about="https://w3id.org/def/vaeontology#benevolenceDef">
        <rdf:type rdf:resource="https://w3id.org/def/vaeontology#ValueDefinition"/>
        <dul:hasSetting rdf:resource="https://w3id.org/def/vaeontology#taxProblemContext"/>
        <dul:defines rdf:resource="https://w3id.org/def/vaeontology#benevolenceTax"/>
    </owl:NamedIndividual>
    


    <!-- https://w3id.org/def/vaeontology#benevolenceNode -->

    <owl:NamedIndividual rdf:about="https://w3id.org/def/vaeontology#benevolenceNode">
        <rdf:type rdf:resource="https://w3id.org/def/vaeontology#ConceptNode"/>
        <hasImportance rdf:resource="https://w3id.org/def/vaeontology#benvolenceNodeImportance"/>
        <directlyGeneralizes rdf:resource="https://w3id.org/def/vaeontology#equalityNode"/>
    </owl:NamedIndividual>
    


    <!-- https://w3id.org/def/vaeontology#benevolenceTax -->

    <owl:NamedIndividual rdf:about="https://w3id.org/def/vaeontology#benevolenceTax">
        <rdf:type rdf:resource="https://w3id.org/spice/SON/SchwartzValues#Benevolence"/>
        <shapesNorm rdf:resource="https://w3id.org/def/vaeontology#payTaxes"/>
    </owl:NamedIndividual>
    


    <!-- https://w3id.org/def/vaeontology#benvolenceNodeImportance -->

    <owl:NamedIndividual rdf:about="https://w3id.org/def/vaeontology#benvolenceNodeImportance">
        <rdf:type rdf:resource="https://w3id.org/def/vaeontology#NodeImportance"/>
        <dul:describes rdf:resource="https://w3id.org/def/vaeontology#benevolenceTax"/>
        <importanceValue rdf:datatype="http://www.w3.org/2001/XMLSchema#float">0.8</importanceValue>
    </owl:NamedIndividual>
    


    <!-- https://w3id.org/def/vaeontology#constraintAlign -->

    <owl:NamedIndividual rdf:about="https://w3id.org/def/vaeontology#constraintAlign">
        <rdf:type rdf:resource="http://www.w3.org/ns/odrl/2/Constraint"/>
        <odrl:leftOperand rdf:resource="https://w3id.org/def/vaeontology#alignPremise"/>
        <odrl:operator rdf:resource="https://w3id.org/def/vaeontology#logicalImplication"/>
        <odrl:operator rdf:resource="https://w3id.org/def/vaeontology#sameContext"/>
        <odrl:rightOperand rdf:resource="https://w3id.org/def/vaeontology#alignClaim"/>
    </owl:NamedIndividual>
    


    <!-- https://w3id.org/def/vaeontology#correctNaming -->

    <owl:NamedIndividual rdf:about="https://w3id.org/def/vaeontology#correctNaming">
        <rdf:type rdf:resource="https://w3id.org/def/vaeontology#SoundArgument"/>
    </owl:NamedIndividual>
    


    <!-- https://w3id.org/def/vaeontology#criterionAlign -->

    <owl:NamedIndividual rdf:about="https://w3id.org/def/vaeontology#criterionAlign">
        <rdf:type rdf:resource="https://w3id.org/def/vaeontology#Criterion"/>
        <dul:describes rdf:resource="https://w3id.org/def/vaeontology#benevolenceTax"/>
        <odrl:action rdf:resource="https://w3id.org/def/vaeontology#alignClaim"/>
        <odrl:constraint rdf:resource="https://w3id.org/def/vaeontology#constraintAlign"/>
        <odrl:target rdf:resource="https://w3id.org/def/vaeontology#alignPremise"/>
    </owl:NamedIndividual>
    


    <!-- https://w3id.org/def/vaeontology#equalityNode -->

    <owl:NamedIndividual rdf:about="https://w3id.org/def/vaeontology#equalityNode">
        <rdf:type rdf:resource="https://w3id.org/def/vaeontology#ConceptNode"/>
        <hasImportance rdf:resource="https://w3id.org/def/vaeontology#equalityNodeImportance"/>
        <directlyGeneralizes rdf:resource="https://w3id.org/def/vaeontology#giniPropertyNode"/>
    </owl:NamedIndividual>
    


    <!-- https://w3id.org/def/vaeontology#equalityNodeImportance -->

    <owl:NamedIndividual rdf:about="https://w3id.org/def/vaeontology#equalityNodeImportance">
        <rdf:type rdf:resource="https://w3id.org/def/vaeontology#NodeImportance"/>
        <dul:describes rdf:resource="https://w3id.org/def/vaeontology#equalityTax"/>
        <importanceValue rdf:datatype="http://www.w3.org/2001/XMLSchema#float">0.8</importanceValue>
    </owl:NamedIndividual>
    


    <!-- https://w3id.org/def/vaeontology#equalityTax -->

    <owl:NamedIndividual rdf:about="https://w3id.org/def/vaeontology#equalityTax">
        <rdf:type rdf:resource="https://w3id.org/def/vaeontology#Equality"/>
        <dul:hasSetting rdf:resource="https://w3id.org/def/vaeontology#taxProblemContext"/>
    </owl:NamedIndividual>
    


    <!-- https://w3id.org/def/vaeontology#evaderAgent -->

    <owl:NamedIndividual rdf:about="https://w3id.org/def/vaeontology#evaderAgent">
        <rdf:type rdf:resource="https://w3id.org/def/vaeontology#ActingAgent"/>
        <dul:hasSetting rdf:resource="https://w3id.org/def/vaeontology#taxProblemContext"/>
        <followsStrategy rdf:resource="https://w3id.org/def/vaeontology#evaderStrategy"/>
        <makesAction rdf:resource="https://w3id.org/def/vaeontology#actOfPayingMiniumumTaxes"/>
    </owl:NamedIndividual>
    


    <!-- https://w3id.org/def/vaeontology#evaderStrategy -->

    <owl:NamedIndividual rdf:about="https://w3id.org/def/vaeontology#evaderStrategy">
        <rdf:type rdf:resource="https://w3id.org/def/vaeontology#Strategy"/>
    </owl:NamedIndividual>
    


    <!-- https://w3id.org/def/vaeontology#generalizationRelationTaxPayer -->

    <owl:NamedIndividual rdf:about="https://w3id.org/def/vaeontology#generalizationRelationTaxPayer">
        <rdf:type rdf:resource="https://w3id.org/def/vaeontology#Generalization"/>
        <comparisonHasInferior rdf:resource="https://w3id.org/def/vaeontology#equalityTax"/>
        <comparisonHasSuperior rdf:resource="https://w3id.org/def/vaeontology#benevolenceTax"/>
        <isProposedByAgent rdf:resource="https://w3id.org/def/vaeontology#payerAgent"/>
    </owl:NamedIndividual>
    


    <!-- https://w3id.org/def/vaeontology#giniIndex0_3 -->

    <owl:NamedIndividual rdf:about="https://w3id.org/def/vaeontology#giniIndex0_3">
        <rdf:type rdf:resource="https://w3id.org/def/vaeontology#GiniIndex"/>
        <dul:describes rdf:resource="https://w3id.org/def/vaeontology#equalityTax"/>
        <measuredOnOutcome rdf:resource="https://w3id.org/def/vaeontology#state1"/>
    </owl:NamedIndividual>
    


    <!-- https://w3id.org/def/vaeontology#giniIndex0_9 -->

    <owl:NamedIndividual rdf:about="https://w3id.org/def/vaeontology#giniIndex0_9">
        <rdf:type rdf:resource="https://w3id.org/def/vaeontology#GiniIndex"/>
        <dul:describes rdf:resource="https://w3id.org/def/vaeontology#equalityTax"/>
        <measuredOnOutcome rdf:resource="https://w3id.org/def/vaeontology#state2"/>
    </owl:NamedIndividual>
    


    <!-- https://w3id.org/def/vaeontology#giniIndexProp -->

    <owl:NamedIndividual rdf:about="https://w3id.org/def/vaeontology#giniIndexProp">
        <rdf:type rdf:resource="https://w3id.org/def/vaeontology#TaxonomyProperty"/>
        <degreeOfSatisfaction rdf:datatype="http://www.w3.org/2001/XMLSchema#float">1.0</degreeOfSatisfaction>
    </owl:NamedIndividual>
    


    <!-- https://w3id.org/def/vaeontology#giniIndexSatisfiedThreshold0_7 -->

    <owl:NamedIndividual rdf:about="https://w3id.org/def/vaeontology#giniIndexSatisfiedThreshold0_7">
        <rdf:type rdf:resource="https://w3id.org/def/vaeontology#BooleanVaeProperty"/>
        <rdf:type rdf:resource="https://w3id.org/def/vaeontology#ValueProperty"/>
        <dul:describes rdf:resource="https://w3id.org/def/vaeontology#equalityTax"/>
    </owl:NamedIndividual>
    


    <!-- https://w3id.org/def/vaeontology#giniPropertyNode -->

    <owl:NamedIndividual rdf:about="https://w3id.org/def/vaeontology#giniPropertyNode">
        <rdf:type rdf:resource="https://w3id.org/def/vaeontology#PropertyNode"/>
        <hasPropertyTaxonomy rdf:resource="https://w3id.org/def/vaeontology#giniIndexProp"/>
    </owl:NamedIndividual>
    


    <!-- https://w3id.org/def/vaeontology#importanceRelationTaxPayer -->

    <owl:NamedIndividual rdf:about="https://w3id.org/def/vaeontology#importanceRelationTaxPayer">
        <rdf:type rdf:resource="https://w3id.org/def/vaeontology#ImportanceRelation"/>
        <comparisonHasInferior rdf:resource="https://w3id.org/def/vaeontology#achievementTax"/>
        <comparisonHasSuperior rdf:resource="https://w3id.org/def/vaeontology#benevolenceTax"/>
        <isProposedByAgent rdf:resource="https://w3id.org/def/vaeontology#payerAgent"/>
    </owl:NamedIndividual>
    


    <!-- https://w3id.org/def/vaeontology#logicalImplication -->

    <owl:NamedIndividual rdf:about="https://w3id.org/def/vaeontology#logicalImplication">
        <rdf:type rdf:resource="https://w3id.org/def/vaeontology#SoundArgument"/>
    </owl:NamedIndividual>
    


    <!-- https://w3id.org/def/vaeontology#multiInputOutcome1 -->

    <owl:NamedIndividual rdf:about="https://w3id.org/def/vaeontology#multiInputOutcome1">
        <rdf:type rdf:resource="https://w3id.org/def/vaeontology#MultiInputOutcome"/>
        <hasInput rdf:resource="https://w3id.org/def/vaeontology#state1"/>
        <hasOutcome rdf:resource="https://w3id.org/def/vaeontology#actOfPayingMiniumumTaxes"/>
        <hasOutcome rdf:resource="https://w3id.org/def/vaeontology#actOfPayingTaxes"/>
        <hasOutcome rdf:resource="https://w3id.org/def/vaeontology#state2"/>
        <nextInputOutcome rdf:resource="https://w3id.org/def/vaeontology#multiInputOutcome2"/>
    </owl:NamedIndividual>
    


    <!-- https://w3id.org/def/vaeontology#multiInputOutcome2 -->

    <owl:NamedIndividual rdf:about="https://w3id.org/def/vaeontology#multiInputOutcome2">
        <rdf:type rdf:resource="https://w3id.org/def/vaeontology#FinalInputOutcome"/>
        <hasInput rdf:resource="https://w3id.org/def/vaeontology#state2"/>
        <hasOutcome rdf:resource="https://w3id.org/def/vaeontology#actOfPayingTaxes"/>
    </owl:NamedIndividual>
    


    <!-- https://w3id.org/def/vaeontology#payMinimumTaxes -->

    <owl:NamedIndividual rdf:about="https://w3id.org/def/vaeontology#payMinimumTaxes">
        <rdf:type rdf:resource="https://w3id.org/def/vaeontology#Norm"/>
        <odrl:action rdf:resource="https://w3id.org/def/vaeontology#actOfPayingMiniumumTaxes"/>
        <odrl:assignee rdf:resource="https://w3id.org/def/vaeontology#evaderAgent"/>
        <odrl:assignee rdf:resource="https://w3id.org/def/vaeontology#payerAgent"/>
        <odrl:assigner rdf:resource="https://w3id.org/def/vaeontology#problemModeller"/>
    </owl:NamedIndividual>
    


    <!-- https://w3id.org/def/vaeontology#payTaxes -->

    <owl:NamedIndividual rdf:about="https://w3id.org/def/vaeontology#payTaxes">
        <rdf:type rdf:resource="https://w3id.org/def/vaeontology#Norm"/>
        <odrl:action rdf:resource="https://w3id.org/def/vaeontology#actOfPayingTaxes"/>
        <odrl:assignee rdf:resource="https://w3id.org/def/vaeontology#evaderAgent"/>
        <odrl:assigner rdf:resource="https://w3id.org/def/vaeontology#problemModeller"/>
    </owl:NamedIndividual>
    


    <!-- https://w3id.org/def/vaeontology#payerAgent -->

    <owl:NamedIndividual rdf:about="https://w3id.org/def/vaeontology#payerAgent">
        <rdf:type rdf:resource="https://w3id.org/def/vaeontology#ActingAgent"/>
        <dul:hasSetting rdf:resource="https://w3id.org/def/vaeontology#taxProblemContext"/>
        <followsStrategy rdf:resource="https://w3id.org/def/vaeontology#payerStrategy"/>
        <makesAction rdf:resource="https://w3id.org/def/vaeontology#actOfPayingTaxes"/>
        <proposesStatement rdf:resource="https://w3id.org/def/vaeontology#alignClaim"/>
        <proposesStatement rdf:resource="https://w3id.org/def/vaeontology#alignPremise"/>
        <proposesStatement rdf:resource="https://w3id.org/def/vaeontology#argumentAlign"/>
        <proposesStatement rdf:resource="https://w3id.org/def/vaeontology#importanceRelationTaxPayer"/>
        <vcvf:commitsTo rdf:resource="https://w3id.org/def/vaeontology#benevolenceTax"/>
    </owl:NamedIndividual>
    


    <!-- https://w3id.org/def/vaeontology#payerStrategy -->

    <owl:NamedIndividual rdf:about="https://w3id.org/def/vaeontology#payerStrategy">
        <rdf:type rdf:resource="https://w3id.org/def/vaeontology#Strategy"/>
    </owl:NamedIndividual>
    


    <!-- https://w3id.org/def/vaeontology#payerTaxonomy -->

    <owl:NamedIndividual rdf:about="https://w3id.org/def/vaeontology#payerTaxonomy">
        <rdf:type rdf:resource="https://w3id.org/def/vaeontology#ValueTaxonomyStatement"/>
        <hasConceptNode rdf:resource="https://w3id.org/def/vaeontology#benevolenceNode"/>
        <hasConceptNode rdf:resource="https://w3id.org/def/vaeontology#equalityNode"/>
        <hasRootNode rdf:resource="https://w3id.org/def/vaeontology#benevolenceNode"/>
        <hasTaxonomyAlignment rdf:resource="https://w3id.org/def/vaeontology#taxonomAlignment"/>
    </owl:NamedIndividual>
    


    <!-- https://w3id.org/def/vaeontology#positiveBenevolenceAlignment -->

    <owl:NamedIndividual rdf:about="https://w3id.org/def/vaeontology#positiveBenevolenceAlignment">
        <rdf:type rdf:resource="https://w3id.org/def/vaeontology#PromotionDemotion"/>
        <dul:describes rdf:resource="https://w3id.org/def/vaeontology#benevolenceTax"/>
    </owl:NamedIndividual>
    


    <!-- https://w3id.org/def/vaeontology#problemModeller -->

    <owl:NamedIndividual rdf:about="https://w3id.org/def/vaeontology#problemModeller">
        <rdf:type rdf:resource="https://w3id.org/def/vaeontology#User"/>
        <isUserOfSystem rdf:resource="https://w3id.org/def/vaeontology#taxSystem"/>
    </owl:NamedIndividual>
    


    <!-- https://w3id.org/def/vaeontology#sameContext -->

    <owl:NamedIndividual rdf:about="https://w3id.org/def/vaeontology#sameContext">
        <rdf:type rdf:resource="https://w3id.org/def/vaeontology#SoundArgument"/>
    </owl:NamedIndividual>
    


    <!-- https://w3id.org/def/vaeontology#sequenceOfOutcomes -->

    <owl:NamedIndividual rdf:about="https://w3id.org/def/vaeontology#sequenceOfOutcomes">
        <rdf:type rdf:resource="https://w3id.org/def/vaeontology#Sequence"/>
        <dul:hasSetting rdf:resource="https://w3id.org/def/vaeontology#taxProblemContext"/>
        <startsWithInputOutcome rdf:resource="https://w3id.org/def/vaeontology#multiInputOutcome1"/>
    </owl:NamedIndividual>
    


    <!-- https://w3id.org/def/vaeontology#state1 -->

    <owl:NamedIndividual rdf:about="https://w3id.org/def/vaeontology#state1">
        <rdf:type rdf:resource="https://w3id.org/def/vaeontology#State"/>
        <satisfiesProperty rdf:resource="https://w3id.org/def/vaeontology#aggregationSum"/>
    </owl:NamedIndividual>
    


    <!-- https://w3id.org/def/vaeontology#state2 -->

    <owl:NamedIndividual rdf:about="https://w3id.org/def/vaeontology#state2">
        <rdf:type rdf:resource="https://w3id.org/def/vaeontology#State"/>
        <satisfiesProperty rdf:resource="https://w3id.org/def/vaeontology#aggregationSum"/>
    </owl:NamedIndividual>
    


    <!-- https://w3id.org/def/vaeontology#taxProblemContext -->

    <owl:NamedIndividual rdf:about="https://w3id.org/def/vaeontology#taxProblemContext">
        <rdf:type rdf:resource="https://w3id.org/def/vaeontology#Context"/>
        <rdfs:comment>This context is of a problem on taxing</rdfs:comment>
    </owl:NamedIndividual>
    


    <!-- https://w3id.org/def/vaeontology#taxSystem -->

    <owl:NamedIndividual rdf:about="https://w3id.org/def/vaeontology#taxSystem">
        <rdf:type rdf:resource="https://w3id.org/def/vaeontology#System"/>
        <dul:hasSetting rdf:resource="https://w3id.org/def/vaeontology#taxProblemContext"/>
        <hasAgent rdf:resource="https://w3id.org/def/vaeontology#evaderAgent"/>
        <hasAgent rdf:resource="https://w3id.org/def/vaeontology#payerAgent"/>
        <hasState rdf:resource="https://w3id.org/def/vaeontology#state1"/>
        <hasState rdf:resource="https://w3id.org/def/vaeontology#state2"/>
        <hasTrace rdf:resource="https://w3id.org/def/vaeontology#sequenceOfOutcomes"/>
        <hasUser rdf:resource="https://w3id.org/def/vaeontology#problemModeller"/>
    </owl:NamedIndividual>
    


    <!-- https://w3id.org/def/vaeontology#taxonomAlignment -->

    <owl:NamedIndividual rdf:about="https://w3id.org/def/vaeontology#taxonomAlignment">
        <rdf:type rdf:resource="https://w3id.org/def/vaeontology#TaxonomyAlignment"/>
    </owl:NamedIndividual>
    


    <!-- 
    ///////////////////////////////////////////////////////////////////////////////////////
    //
    // General axioms
    //
    ///////////////////////////////////////////////////////////////////////////////////////
     -->

    <rdf:Description>
        <rdf:type rdf:resource="http://www.w3.org/2002/07/owl#AllDisjointClasses"/>
        <owl:members rdf:parseType="Collection">
            <rdf:Description rdf:about="http://www.ontologydesignpatterns.org/ont/dul/DUL.owl#Event"/>
            <rdf:Description rdf:about="https://w3id.org/def/vaeontology#Agent"/>
            <rdf:Description rdf:about="https://w3id.org/def/vaeontology#Norm"/>
        </owl:members>
    </rdf:Description>
    <rdf:Description>
        <rdf:type rdf:resource="http://www.w3.org/2002/07/owl#AllDisjointClasses"/>
        <owl:members rdf:parseType="Collection">
            <rdf:Description rdf:about="http://www.ontologydesignpatterns.org/ont/dul/DUL.owl#Norm"/>
            <rdf:Description rdf:about="http://www.ontologydesignpatterns.org/ont/dul/DUL.owl#Theory"/>
            <rdf:Description rdf:about="https://w3id.org/def/vaeontology#VaeProperty"/>
            <rdf:Description rdf:about="https://w3id.org/framester/schema/ConceptualFrame"/>
        </owl:members>
    </rdf:Description>
    <rdf:Description>
        <rdf:type rdf:resource="http://www.w3.org/2002/07/owl#AllDisjointClasses"/>
        <owl:members rdf:parseType="Collection">
            <rdf:Description rdf:about="https://w3id.org/def/vaeontology#Action"/>
            <rdf:Description rdf:about="https://w3id.org/def/vaeontology#ActionOnState"/>
            <rdf:Description rdf:about="https://w3id.org/def/vaeontology#MultiInputOutcome"/>
            <rdf:Description rdf:about="https://w3id.org/def/vaeontology#Sequence"/>
            <rdf:Description rdf:about="https://w3id.org/def/vaeontology#State"/>
            <rdf:Description rdf:about="https://w3id.org/def/vaeontology#Strategy"/>
        </owl:members>
    </rdf:Description>
    <rdf:Description>
        <rdf:type rdf:resource="http://www.w3.org/2002/07/owl#AllDisjointClasses"/>
        <owl:members rdf:parseType="Collection">
            <rdf:Description rdf:about="https://w3id.org/def/vaeontology#Agent"/>
            <rdf:Description rdf:about="https://w3id.org/def/vaeontology#Norm"/>
            <rdf:Description rdf:about="https://w3id.org/def/vaeontology#Outcome"/>
            <rdf:Description rdf:about="https://w3id.org/def/vaeontology#VaeProperty"/>
            <rdf:Description rdf:about="https://w3id.org/def/vaeontology#ValueConcept"/>
        </owl:members>
    </rdf:Description>
    <rdf:Description>
        <rdf:type rdf:resource="http://www.w3.org/2002/07/owl#AllDisjointClasses"/>
        <owl:members rdf:parseType="Collection">
            <rdf:Description rdf:about="https://w3id.org/def/vaeontology#AgentStatement"/>
            <rdf:Description rdf:about="https://w3id.org/def/vaeontology#VaeSituation"/>
            <rdf:Description rdf:about="https://w3id.org/def/vaeontology#VaeStatementEntity"/>
        </owl:members>
    </rdf:Description>
    <rdf:Description>
        <rdf:type rdf:resource="http://www.w3.org/2002/07/owl#AllDisjointClasses"/>
        <owl:members rdf:parseType="Collection">
            <rdf:Description rdf:about="https://w3id.org/def/vaeontology#ArgumentStatement"/>
            <rdf:Description rdf:about="https://w3id.org/def/vaeontology#Criterion"/>
            <rdf:Description rdf:about="https://w3id.org/def/vaeontology#ValueComparisonStatement"/>
            <rdf:Description rdf:about="https://w3id.org/def/vaeontology#ValueDefinition"/>
            <rdf:Description rdf:about="https://w3id.org/def/vaeontology#ValueTaxonomyStatement"/>
        </owl:members>
    </rdf:Description>
    <rdf:Description>
        <rdf:type rdf:resource="http://www.w3.org/2002/07/owl#AllDisjointClasses"/>
        <owl:members rdf:parseType="Collection">
            <rdf:Description rdf:about="https://w3id.org/spice/SON/SchwartzValues#Achievement"/>
            <rdf:Description rdf:about="https://w3id.org/spice/SON/SchwartzValues#Face"/>
            <rdf:Description rdf:about="https://w3id.org/spice/SON/SchwartzValues#Hedonism"/>
        </owl:members>
    </rdf:Description>
    <rdf:Description>
        <rdf:type rdf:resource="http://www.w3.org/2002/07/owl#AllDisjointClasses"/>
        <owl:members rdf:parseType="Collection">
            <rdf:Description rdf:about="https://w3id.org/spice/SON/SchwartzValues#Concern"/>
            <rdf:Description rdf:about="https://w3id.org/spice/SON/SchwartzValues#Nature"/>
            <rdf:Description rdf:about="https://w3id.org/spice/SON/SchwartzValues#Tolerance"/>
        </owl:members>
    </rdf:Description>
    <rdf:Description>
        <rdf:type rdf:resource="http://www.w3.org/2002/07/owl#AllDisjointClasses"/>
        <owl:members rdf:parseType="Collection">
            <rdf:Description rdf:about="https://w3id.org/spice/SON/SchwartzValues#Conformity"/>
            <rdf:Description rdf:about="https://w3id.org/spice/SON/SchwartzValues#Face"/>
            <rdf:Description rdf:about="https://w3id.org/spice/SON/SchwartzValues#Humility"/>
            <rdf:Description rdf:about="https://w3id.org/spice/SON/SchwartzValues#Security"/>
        </owl:members>
    </rdf:Description>
    <rdf:Description>
        <rdf:type rdf:resource="http://www.w3.org/2002/07/owl#AllDisjointClasses"/>
        <owl:members rdf:parseType="Collection">
            <rdf:Description rdf:about="https://w3id.org/spice/SON/SchwartzValues#Conformity"/>
            <rdf:Description rdf:about="https://w3id.org/spice/SON/SchwartzValues#Face"/>
            <rdf:Description rdf:about="https://w3id.org/spice/SON/SchwartzValues#Humility"/>
            <rdf:Description rdf:about="https://w3id.org/spice/SON/SchwartzValues#Tradition"/>
        </owl:members>
    </rdf:Description>
    <rdf:Description>
        <rdf:type rdf:resource="http://www.w3.org/2002/07/owl#AllDisjointClasses"/>
        <owl:members rdf:parseType="Collection">
            <rdf:Description rdf:about="https://w3id.org/spice/SON/SchwartzValues#Face"/>
            <rdf:Description rdf:about="https://w3id.org/spice/SON/SchwartzValues#Hedonism"/>
            <rdf:Description rdf:about="https://w3id.org/spice/SON/SchwartzValues#Power"/>
        </owl:members>
    </rdf:Description>
    <rdf:Description>
        <rdf:type rdf:resource="http://www.w3.org/2002/07/owl#AllDisjointClasses"/>
        <owl:members rdf:parseType="Collection">
            <rdf:Description rdf:about="https://w3id.org/spice/SON/SchwartzValues#Hedonism"/>
            <rdf:Description rdf:about="https://w3id.org/spice/SON/SchwartzValues#SelfDirection"/>
            <rdf:Description rdf:about="https://w3id.org/spice/SON/SchwartzValues#Stimulation"/>
        </owl:members>
    </rdf:Description>
</rdf:RDF>



<!-- Generated by the OWL API (version 4.5.26.2023-07-17T20:34:13Z) https://github.com/owlcs/owlapi -->

